@prefix rdfs: <http://www.w3.org/2000/01/rdf-schema#> .
@prefix owl:  <http://www.w3.org/2002/07/owl#> .
@prefix xsd:  <http://www.w3.org/2001/XMLSchema#> .
@prefix qa:   <https://www.statnett.no/Talk2PowerSystem/qa#> .
@prefix dct:  <http://purl.org/dc/terms/> .

qa: {

#################################################################
# Ontology Definition
#################################################################

qa: a owl:Ontology ;
    rdfs:label "Talk2PowerSystem Q&A Dataset Ontology"@en ;
    rdfs:comment "Ontology describing templates and paraphrases for the Q&A dataset in the Talk2PowerSystem project."@en ;
    dct:creator <https://graphwise.ai> ;
    dct:created "2025-11-14"^^xsd:date ;
    dct:modified "2025-11-14"^^xsd:date ;
    owl:versionInfo "1.0.0"^^xsd:string ;
    dct:license <https://creativecommons.org/licenses/by-sa/4.0> .

#################################################################
# Classes
#################################################################

qa:Template a owl:Class ;
    rdfs:label "Template"@en ;
    rdfs:comment "A query template that defines a general question pattern."@en ;
    rdfs:isDefinedBy qa: .

qa:Paraphrase a owl:Class ;
    rdfs:label "Paraphrase"@en ;
    rdfs:comment "A paraphrase instance representing a natural language question."@en ;
    rdfs:isDefinedBy qa: .

#################################################################
# Object Properties
#################################################################

qa:paraphrase a owl:ObjectProperty ;
    rdfs:label "paraphrase"@en ;
    rdfs:comment "Links a template to one of its paraphrases."@en ;
    rdfs:domain qa:Template ;
    rdfs:range qa:Paraphrase ;
    rdfs:isDefinedBy qa: .

#################################################################
# Data Properties
#################################################################

qa:question a owl:DatatypeProperty ;
    rdfs:label "question"@en ;
    rdfs:comment "The natural language question corresponding to the paraphrase."@en ;
    rdfs:domain qa:Paraphrase ;
    rdfs:range xsd:string ;
    rdfs:isDefinedBy qa: .

qa:querySparql a owl:DatatypeProperty ;
    rdfs:label "SPARQL query"@en ;
    rdfs:comment "The SPARQL query corresponding to the template."@en ;
    rdfs:domain qa:Template ;
    rdfs:range xsd:string ;
    rdfs:isDefinedBy qa: .

}
