@prefix adms: <http://www.w3.org/ns/adms#> .
@prefix alstom: <http://www.alstom.com/grid/CIM-schema-cim15-extension#> .
@prefix cdpsm: <http://iec.ch/TC57/CIM/CDPSM/SchemaExtension/2/0#> .
@prefix cim15: <http://iec.ch/TC57/2010/CIM-schema-cim15#> .
@prefix cim16: <http://iec.ch/TC57/2013/CIM-schema-cim16#> .
@prefix cim17: <http://iec.ch/TC57/CIM100#> .
@prefix cim: <https://cim.ucaiug.io/ns#> .
@prefix cimr: <https://cim.ucaiug.io/rules#> .
@prefix cims: <http://iec.ch/TC57/1999/rdf-schema-extensions-19990926#> .
@prefix dc: <http://purl.org/dc/elements/1.1/> .
@prefix dcat: <http://www.w3.org/ns/dcat#> .
@prefix dct: <http://purl.org/dc/terms/> .
@prefix entsoe_prof: <http://entsoe.eu/Secretariat/ProfileExtension/1#> .
@prefix entsoe_sch: <http://entsoe.eu/CIM/SchemaExtension/3/1#> .
@prefix eu1: <http://iec.ch/TC57/CIM100-European#> .
@prefix eu: <https://cim.ucaiug.io/ns/eu#> .
@prefix eu_ext: <http://iec.ch/TC57/CIM100-EuropeanExtension/1/0#> .
@prefix form: <https://form.statnett.no/voc/form-ksd-extensions#> .
@prefix form_ann: <https://form.statnett.no/schema/annotation#> .
@prefix geo: <http://www.opengis.net/ont/geosparql#> .
@prefix iec61968: <http://iec.ch/TC57/Inf/61968#> .
@prefix md: <http://iec.ch/TC57/61970-552/ModelDescription/1#> .
@prefix nc-no: <https://cim4.eu/ns/nc-no#> .
@prefix nc1: <http://entsoe.eu/ns/nc#> .
@prefix nc: <https://cim4.eu/ns/nc#> .
@prefix nek: <http://NEK.no/NK57/CIM/CIM100-Extension/1/0#> .
@prefix onto: <http://www.ontotext.com/> .
@prefix owl: <http://www.w3.org/2002/07/owl#> .
@prefix prefix: <http://qudt.org/vocab/prefix/> .
@prefix prov: <http://www.w3.org/ns/prov#> .
@prefix psys: <http://proton.semanticweb.org/protonsys#> .
@prefix pti: <http://www.pti-us.com/PTI_CIM-schema-cim16#> .
@prefix qkdv: <http://qudt.org/vocab/dimensionvector/> .
@prefix quantitykind: <http://qudt.org/vocab/quantitykind/> .
@prefix qudt: <http://qudt.org/schema/qudt/> .
@prefix rdf: <http://www.w3.org/1999/02/22-rdf-syntax-ns#> .
@prefix rdfs: <http://www.w3.org/2000/01/rdf-schema#> .
@prefix sh: <http://www.w3.org/ns/shacl#> .
@prefix skos: <http://www.w3.org/2004/02/skos/core#> .
@prefix so: <http://www.ontotext.com/semantic-object#> .
@prefix statnett: <http://www.statnett.no/CIM-schema-cim15-extension#> .
@prefix uml1: <http://langdale.com.au/2005/UML#> .
@prefix uml: <http://iec.ch/TC57/NonStandard/UML#> .
@prefix unit: <http://qudt.org/vocab/unit/> .
@prefix xsd: <http://www.w3.org/2001/XMLSchema#> .
@prefix rdf4j: <http://rdf4j.org/schema/rdf4j#> .
@prefix sesame: <http://www.openrdf.org/schema/sesame#> .
@prefix fn: <http://www.w3.org/2005/xpath-functions#> .

cims:pragmatics a owl:DatatypeProperty;
  rdfs:comment "Specific SPARQL guidance and important practical information for an LLM. Applies to Classes and Properties.";
  rdfs:range xsd:string;
  rdfs:label "LLM Pragmatics" .

dct:accessRights a owl:ObjectProperty, owl:FunctionalProperty;
  rdfs:comment """Information about who access the resource or an indication of its security status. Access Rights may include information regarding access or restrictions based on privacy, security, or other policies.
[CIM context:
Reference to the confidentiality level that shall be applied when handling this model.]."""@en;
  rdfs:domain dcat:Dataset;
  rdfs:range dcat:Dataset;
  rdfs:label "accessRights";
  cims:multiplicity cims:M:0..1 .

dct:conformsTo a owl:ObjectProperty;
  rdfs:comment "An established standard to which the described resource conforms. [CIM context: An IRI describing the profile that governs this model. It uniquely identifies the profile and its version. Multiple instances of the property describe all standards or specifications to which the model and the document representing this model conform to. A document would normally conform to profile definitions, the constraints that relate to the profile and/or the set of business specific constrains. A reference to a"@en;
  rdfs:domain dcat:Dataset;
  rdfs:range dcat:Dataset;
  rdfs:label "conformsTo";
  cims:multiplicity cims:M:0..n .

dct:description a owl:FunctionalProperty, owl:DatatypeProperty;
  rdfs:comment """A free-text account of the resource.
Description may include but is not limited to: an abstract, a table of contents, a graphical representation, or a free-text account of the resource."""@en,
    "A free-text account of the item."@en;
  rdfs:range xsd:string;
  rdfs:label "description";
  cims:multiplicity cims:M:0..1 .

dct:identifier a owl:FunctionalProperty, owl:DatatypeProperty;
  rdfs:comment "A unique identifier of the resource being described or cataloged. The identifier might be used as part of the IRI of the resource, but still having it represented explicitly is useful. The identifier is a text string which is assigned to the resource to provide an unambiguous reference within a particular context. [CIM context: A unique identifier of the model which is serialised in the document where the header is located. The identifier is persistent for a given version of the model and shall change"@en,
    "An unambiguous reference to the resource within a given context. Recommended practice is to identify the resource by means of a string conforming to an identification system. Examples include International Standard Book Number (ISBN), Digital Object Identifier (DOI), and Uniform Resource Name (URN). Persistent identifiers should be provided as HTTP URIs. [CIM context: A unique identifier of the model which is serialised in the document where the header is located. The identifier is persistent for"@en;
  rdfs:domain dcat:Dataset;
  rdfs:range xsd:string;
  rdfs:label "identifier";
  cims:multiplicity cims:M:0..1 .

dct:issued a owl:FunctionalProperty, owl:DatatypeProperty;
  rdfs:comment """Date of formal issuance of the resource.
Recommended practice is to describe the date, date/time, or period of time as recommended for the property Date, of which this is a subproperty.
[CIM context:
Reference to the date that the complete data set was made valid/available.]."""@en,
    """The date of listing (i.e., formal recording) of the corresponding dataset or service in the catalog.
[CIM context:
Reference to the date that the complete data set was made valid/available.]."""@en;
  rdfs:domain dcat:Dataset;
  rdfs:range xsd:dateTime;
  rdfs:label "issued";
  cims:multiplicity cims:M:0..1 .

dct:license a owl:ObjectProperty, owl:FunctionalProperty;
  rdfs:comment """A legal document giving official permission to do something with the resource. Recommended practice is to identify the license document with a URI. If this is not possible or feasible, a literal value that identifies the license may be provided.
[CIM context:
Reference to the license under which the data is made available. If no license holder is defined, then the original data provider holds the license.]."""@en;
  rdfs:domain dcat:Dataset;
  rdfs:range dcat:Dataset;
  rdfs:label "license";
  cims:multiplicity cims:M:0..1 .

dct:publisher a owl:ObjectProperty, owl:FunctionalProperty;
  rdfs:comment """An entity responsible for making the resource available.
[CIM context: 
The agent that is publishing the dataset on the given platform.]"""@en;
  rdfs:label "publisher";
  cims:multiplicity cims:M:0..1 .

dct:references a owl:ObjectProperty;
  rdfs:comment """A related resource that is referenced, cited, or otherwise pointed to by the described resource[.
[CIM context: 
The referenced resource that is being complemented in this dataset, e.g. SSH is referencing EQ.]"""@en;
  rdfs:domain dcat:Dataset;
  rdfs:range dcat:Dataset;
  rdfs:label "references";
  cims:multiplicity cims:M:0..n .

dct:rights a owl:FunctionalProperty, owl:DatatypeProperty;
  rdfs:comment "A statement that concerns all rights not addressed with dct:license or dct:accessRights, such as copyright statements."@en;
  rdfs:domain dcat:Dataset;
  rdfs:range xsd:string;
  rdfs:label "rights";
  cims:multiplicity cims:M:0..1 .

dct:rightsHolder a owl:FunctionalProperty, owl:DatatypeProperty;
  rdfs:comment """Information about rights held in and over the resource.
Typically, rights information includes a statement about various property rights associated with the resource, including intellectual property rights. Recommended practice is to refer to a rights statement with a URI. If this is not possible or feasible, a literal value (name, label, or short text) may be provided."""@en,
    "Information about rights held in and over the resource. Typically, rights information includes a statement about various property rights associated with the resource, including intellectual property rights. Recommended practice is to refer to a rights statement with a URI. If this is not possible or feasible, a literal value (name, label, or short text) may be provided."@en;
  rdfs:domain dcat:Dataset;
  rdfs:range xsd:string;
  rdfs:label "rightsHolder";
  cims:multiplicity cims:M:0..1 .

dct:spatial a owl:ObjectProperty, owl:FunctionalProperty;
  rdfs:comment """The geographical area covered by the dataset.
[CIM context: 
The responsibility area that multiple model can describe, also referred to frame.]"""@en;
  rdfs:domain dcat:Dataset;
  rdfs:range dcat:Dataset;
  rdfs:label "spatial";
  cims:multiplicity cims:M:0..1 .

dct:title a owl:FunctionalProperty, owl:DatatypeProperty;
  rdfs:comment """A name given to the resource.
[CIM context: 
The human readable name of the dataset that can form the instance file name.]"""@en,
    """A name given to the resource
[CIM context: 

The human readable name of the dataset that can form the instance file name.]"""@en;
  rdfs:domain dcat:Dataset;
  rdfs:range xsd:string;
  rdfs:label "title";
  cims:multiplicity cims:M:0..1 .

dct:type a owl:ObjectProperty, owl:FunctionalProperty;
  rdfs:comment "The nature or genre of the resource. Recommended practice is to use a controlled vocabulary such as the DCMI Type Vocabulary [DCMI-TYPE]. To describe the file format, physical medium, or dimensions of the resource, use the property Format."@en;
  rdfs:domain dcat:Dataset;
  rdfs:range dcat:Dataset;
  rdfs:label "type";
  cims:multiplicity cims:M:0..1 .

qudt:CurrencyUnit a rdfs:Class, sh:NodeShape;
  rdfs:subClassOf qudt:DimensionlessUnit;
  dct:description """
  Currency Units have their own subclass of unit because:
   (a) they have additional properties such as 'country' and
   (b) their URIs do not conform to the same rules as other units.
  """^^rdf:HTML;
  rdfs:label "Currency Unit" .

qudt:DecimalPrefix a rdfs:Class, sh:NodeShape;
  rdfs:subClassOf qudt:Prefix;
  dct:description """
  A <em>Decimal Prefix</em> is a prefix for multiples of units that are powers of 10.
  """;
  rdfs:label "Decimal Prefix" .

qudt:DerivedUnit a rdfs:Class, sh:NodeShape;
  rdfs:subClassOf qudt:Unit;
  dct:description """
  <p>A <em>Derived Unit</em> is a type specification for units that are derived from other units.
  </p>"""^^rdf:HTML;
  rdfs:label "Derived Unit" .

qudt:Prefix a rdfs:Class, sh:NodeShape;
  rdfs:subClassOf qudt:Concept, qudt:Verifiable;
  rdfs:label "Prefix" .

qudt:QuantityKind a rdfs:Class, sh:NodeShape;
  rdfs:subClassOf qudt:Verifiable, qudt:AbstractQuantityKind;
  dct:description """
  <p>A <em>Quantity Kind</em> is any observable property that can be  measured and quantified numerically. 
  Familiar examples include physical properties such as length, mass, time, force, energy, power, electric charge, etc. 
  Less familiar examples include currency, interest rate, price to earning ratio, and information capacity.
  </p>"""^^rdf:HTML;
  rdfs:label "Quantity Kind" .

qudt:QuantityKindDimensionVector_CGS a rdfs:Class, sh:NodeShape;
  rdfs:subClassOf qudt:QuantityKindDimensionVector;
  dct:description "A <em>CGS Dimension Vector</em> is used to specify the dimensions for a C.G.S. quantity kind."^^rdf:HTML;
  rdfs:label "CGS Dimension vector" .

qudt:QuantityKindDimensionVector_ISO a rdfs:Class, sh:NodeShape;
  rdfs:subClassOf qudt:QuantityKindDimensionVector;
  rdfs:label "ISO Dimension vector" .

qudt:QuantityKindDimensionVector_Imperial a rdfs:Class, sh:NodeShape;
  rdfs:subClassOf qudt:QuantityKindDimensionVector;
  rdfs:label "Imperial dimension vector" .

qudt:QuantityKindDimensionVector_SI a rdfs:Class, sh:NodeShape;
  rdfs:subClassOf qudt:QuantityKindDimensionVector;
  rdfs:label "Quantity Kind Dimension vector (SI)" .

qudt:SystemOfUnits a rdfs:Class, sh:NodeShape;
  rdfs:subClassOf qudt:Concept, qudt:Verifiable;
  dct:description """
  <p>A <em>System of Units</em> is a set of units which are chosen as the reference scales for some set of quantity kinds together with the definitions of each unit. 
  Units may be defined by experimental observation or by proportion to another unit not included in the system. 
  If the unit system is explicitly associated with a quantity kind system, then the unit system must define at least one unit for each quantity kind.
  </p>"""^^rdf:HTML;
  rdfs:label "System of Units" .

qudt:Unit a rdfs:Class, sh:NodeShape;
  rdfs:subClassOf qudt:Concept, qudt:Verifiable;
  dct:description """
  A unit of measure, or unit, is a particular quantity value that has been chosen as a scale for measuring other quantities the same kind (more generally of equivalent dimension). 
  For example, the meter is a quantity of length that has been rigorously defined and standardized by the BIPM (International Board of Weights and Measures). 
  Any measurement of the length can be expressed as a number multiplied by the unit meter. 
  More formally, the value of a physical quantity Q with respect to a unit (U) is expressed as the scalar multiple of a real number (n) and U, as  $Q = nU$.
  """^^qudt:LatexString;
  rdfs:label "Unit" .

unit:CCY_EUR-PER-MegaW-HR a qudt:Unit;
  rdfs:label "Euro per Megawatt Hour", "Euro per Megawatt Hour"@en;
  qudt:hasQuantityKind quantitykind:CostPerEnergy;
  qudt:conversionMultiplier 0.000000000277777777777777777777777777778;
  qudt:conversionMultiplierSN 2.777777777777777777777777777777778E-10;
  qudt:hasDimensionVector qkdv:A0E0L-2I0M-1H0T2D0;
  qudt:hasFactorUnit _:node11, _:node12, _:node13;
  qudt:plainTextDescription "Unit for measuring the cost of electricity.";
  qudt:symbol "€/(MW·h)" .

unit:CCY_NOK-PER-MegaW-HR a qudt:Unit;
  rdfs:label "Norwegian Krone per Megawatt Hour", "Norwegian Krone per Megawatt Hour"@en;
  qudt:hasQuantityKind quantitykind:CostPerEnergy;
  qudt:conversionMultiplier 0.000000000277777777777777777777777777778;
  qudt:conversionMultiplierSN 2.777777777777777777777777777777778E-10;
  qudt:hasDimensionVector qkdv:A0E0L-2I0M-1H0T2D0;
  qudt:hasFactorUnit _:node8, _:node9, _:node10;
  qudt:plainTextDescription "Unit for measuring the cost of electricity.";
  qudt:symbol "NOK/(MW·h)" .

unit:MegaW a qudt:Unit;
  dct:description "1,000,000-fold of the derived unit watt";
  rdfs:label "Megawatt", "Megawatt"@en;
  qudt:hasQuantityKind quantitykind:ElectricPower, quantitykind:Power;
  qudt:conversionMultiplier 1000000.0;
  qudt:conversionMultiplierSN 1.0E6;
  qudt:hasDimensionVector qkdv:A0E0L2I0M1H0T-3D0;
  qudt:symbol "MW";
  qudt:prefix prefix:Mega;
  qudt:uneceCommonCode "MAW";
  qudt:scalingOf unit:W .

adms:versionNotes a owl:FunctionalProperty, owl:DatatypeProperty;
  rdfs:comment "A description of changes between this version and the previous version of the resource."@en;
  rdfs:domain dcat:Dataset;
  rdfs:range xsd:string;
  rdfs:label "versionNotes";
  cims:multiplicity cims:M:0..1 .

dcat:Dataset a owl:Class;
  rdfs:comment "A collection of data, published or curated by a single source, and available for access or download in one or more representations."@en;
  rdfs:label "Dataset" .

dcat:endDate a owl:FunctionalProperty, owl:DatatypeProperty;
  rdfs:comment """This property contains the end of the period.
[CIM context:
The end date and time of the validity period of the model that it is serialized in the document where the header is located. It is only used in relation to the startDate property which indicates the beginning of the validity period of the model.]."""@en;
  rdfs:domain dcat:Dataset;
  rdfs:range xsd:dateTimeStamp;
  rdfs:label "endDate";
  cims:multiplicity cims:M:0..1 .

dcat:hasVersion a owl:ObjectProperty, owl:InverseFunctionalProperty;
  rdfs:comment """This resource is a version of a non-versioned or abstract resource.
This property is intended for relating a versioned resource to a non-versioned or abstract resource.

The notion of version used by this property is limited to versions resulting from revisions occurring to a resource as part of its life-cycle. Therefore, its semantics is more specific than its super-property dct:isVersionOf, which makes use of a broader notion of version, including editions and adaptations."""@en;
  rdfs:domain dcat:Dataset;
  rdfs:range dcat:Dataset;
  rdfs:label "hasVersion";
  cims:multiplicity cims:M:0..n;
  owl:inverseOf dcat:isVersionOf .

dcat:isVersionOf a owl:ObjectProperty, owl:FunctionalProperty;
  rdfs:comment """This resource has a more specific, versioned resource. This property is intended for relating a non-versioned or abstract resource to several versioned resources, e.g., snapshots.

The notion of version used by this property is limited to versions resulting from revisions occurring to a resource as part of its life-cycle. Therefore, its semantics is more specific than its super-property dct:hasVersion, which makes use of a broader notion of version, including editions and adaptations."""@en;
  rdfs:domain dcat:Dataset;
  rdfs:range dcat:Dataset;
  rdfs:label "isVersionOf";
  cims:multiplicity cims:M:0..1;
  owl:inverseOf dcat:hasVersion .

dcat:keyword a owl:FunctionalProperty, owl:DatatypeProperty;
  rdfs:comment "A keyword or tag describing a resource. [CIM context: The intended content type of the model, usually the profile keyword. Used to identify what profiles and content is expected in the document, e.g., Equipment, Boundary, SSH, AE, etc. The same keyword is used for different versions of same profile. It can be also used to identify different content based on the same profile. For instance, as the equipment profile can be used for both boundary data and equipment not related to boundary, the keyword"@en;
  rdfs:domain dcat:Dataset;
  rdfs:range xsd:string;
  rdfs:label "keyword";
  cims:multiplicity cims:M:0..n, cims:M:0..1 .

dcat:startDate a owl:FunctionalProperty, owl:DatatypeProperty;
  rdfs:comment "This property contains the start of the period. [CIM context: The date and time that this model represents, i.e. for which the model is (or was) valid. It indicates the beginning of the validity period. It is indicating either an instant (in cases where the model is only valid for a point in time) or the start time of a period. If not provided the model is considered valid for any time stamp. The format is an extended format according to the ISO 8601-2005. European exchanges shall refer to UTC.]."@en,
    "This property contains the start of the  period. [CIM context: The date and time that this model represents, i.e. for which the model is (or was) valid. It indicates the beginning of the validity period. It is indicating either an instant (in cases where the model is only valid for a point in time) or the start time of a period. If not provided the model is considered valid for any time stamp. The format is an extended format according to the ISO 8601-2005. European exchanges shall refer to UTC.]."@en;
  rdfs:domain dcat:Dataset;
  rdfs:range xsd:dateTimeStamp;
  rdfs:label "startDate";
  cims:multiplicity cims:M:0..1 .

dcat:temporalResolution a owl:FunctionalProperty, owl:DatatypeProperty;
  rdfs:comment """Minimum time period resolvable in a dataset.
[CIM context: 
Describes the Market Time Unit (MTU), e.g. hourly, 15 min., etc.]"""@en,
    """Minimum time period resolvable in the dataset.
[CIM context: 

Describes the Market Time Unit (MTU), e.g. hourly, 15 min., etc.]"""@en;
  rdfs:domain dcat:Dataset;
  rdfs:range xsd:duration;
  rdfs:label "temporalResolution";
  cims:multiplicity cims:M:0..1 .

dcat:version a owl:FunctionalProperty, owl:DatatypeProperty;
  rdfs:comment "The version indicator (name or identifier) of a resource."@en, "The version number of a resource."@en;
  rdfs:domain dcat:Dataset;
  rdfs:range xsd:string;
  rdfs:label "version";
  cims:multiplicity cims:M:0..1 .

prov:Entity a owl:ObjectProperty, owl:InverseFunctionalProperty;
  rdfs:comment "The entity that generated by this activity."@en;
  rdfs:domain dcat:Dataset;
  rdfs:range dcat:Dataset;
  rdfs:label "Entity";
  cims:multiplicity cims:M:0..n;
  owl:inverseOf prov:wasGeneratedBy .

prov:generatedAtTime a owl:FunctionalProperty, owl:DatatypeProperty;
  rdfs:comment """Generation is the completion of production of a new entity by an activity. This entity did not exist before generation and becomes available for usage after this generation.
[CIM context:
The date and time when the model was serialized in the document where the header is located. The format is an extended format according to the ISO 8601-2005. European exchanges shall refer to UTC.]."""@en;
  rdfs:domain dcat:Dataset;
  rdfs:range xsd:dateTime;
  rdfs:label "generatedAtTime";
  cims:multiplicity cims:M:0..1 .

prov:wasGeneratedBy a owl:ObjectProperty, owl:FunctionalProperty;
  rdfs:comment """Generation is the completion of production of a new entity by an activity. This entity did not exist before generation and becomes available for usage after this generation.
[CIM context:
Reference to an activity or the exact business nature (process, configuration) which produced or uses the model.]."""@en;
  rdfs:domain dcat:Dataset;
  rdfs:range dcat:Dataset;
  rdfs:label "wasGeneratedBy";
  cims:multiplicity cims:M:0..1;
  owl:inverseOf prov:Entity .

cim:ACDCTerminal a owl:Class;
  rdfs:comment "An electrical connection point (AC or DC) to a piece of conducting equipment. Terminals are connected at physical connection points called connectivity nodes."@en;
  rdfs:subClassOf cim:IdentifiedObject;
  rdfs:label "ACDCTerminal" .

cim:ACDCTerminal.OperationalLimitSet a owl:ObjectProperty, owl:InverseFunctionalProperty;
  rdfs:comment "The operational limit sets at the terminal."@en;
  rdfs:domain cim:ACDCTerminal;
  rdfs:range cim:OperationalLimitSet;
  rdfs:label "OperationalLimitSet";
  cims:multiplicity cims:M:0..n;
  owl:inverseOf cim:OperationalLimitSet.Terminal .

cim:ACDCTerminal.connected a owl:FunctionalProperty, owl:DatatypeProperty;
  rdfs:comment "The connected status is related to a bus-branch model and the topological node to terminal relation.  True implies the terminal is connected to the related topological node and false implies it is not.  In a bus-branch model, the connected status is used to tell if equipment is disconnected without having to change the connectivity described by the topological node to terminal relation. A valid case is that conducting equipment can be connected in one end and open in the other. In particular for"@en;
  rdfs:domain cim:ACDCTerminal;
  rdfs:range xsd:boolean;
  rdfs:label "connected";
  cims:multiplicity cims:M:1..1 .

cim:ACDCTerminal.sequenceNumber a owl:FunctionalProperty, owl:DatatypeProperty;
  rdfs:comment "The orientation of the terminal connections for a multiple terminal conducting equipment.  The sequence numbering starts with 1 and additional terminals should follow in increasing order.   The first terminal is the \"starting point\" for a two terminal branch."@en;
  rdfs:domain cim:ACDCTerminal;
  rdfs:range xsd:integer;
  rdfs:label "sequenceNumber";
  cims:multiplicity cims:M:1..1 .

cim:ACLineSegment a owl:Class;
  rdfs:comment "A wire or combination of wires, with consistent electrical characteristics, building a single electrical system, used to carry alternating current between points in the power system. For symmetrical, transposed three phase lines, it is sufficient to use attributes of the line segment, which describe impedances and admittances for the entire length of the segment.  Additionally impedances can be computed by using length and associated per length impedances. The BaseVoltage at the two ends of ACLineSegments"@en;
  rdfs:subClassOf cim:Conductor;
  rdfs:label "ACLineSegment" .

cim:ACLineSegment.b0ch a owl:FunctionalProperty, owl:DatatypeProperty;
  rdfs:comment "Zero sequence shunt (charging) susceptance, uniformly distributed, of the entire line section."@en;
  rdfs:domain cim:ACLineSegment;
  rdfs:range xsd:float;
  rdfs:label "b0ch";
  cims:multiplicity cims:M:1..1;
  cim:unitMultiplier cim:UnitMultiplier.none;
  cim:unitSymbol cim:UnitSymbol.S;
  qudt:hasQuantityKind cim:Susceptance;
  qudt:hasUnit unit:S .

cim:ACLineSegment.bch a owl:FunctionalProperty, owl:DatatypeProperty;
  rdfs:comment "Positive sequence shunt (charging) susceptance, uniformly distributed, of the entire line section.  This value represents the full charging over the full length of the line."@en;
  rdfs:domain cim:ACLineSegment;
  rdfs:range xsd:float;
  rdfs:label "bch";
  cims:multiplicity cims:M:1..1;
  cim:unitMultiplier cim:UnitMultiplier.none;
  cim:unitSymbol cim:UnitSymbol.S;
  qudt:hasQuantityKind cim:Susceptance;
  qudt:hasUnit unit:S .

cim:ACLineSegment.g0ch a owl:FunctionalProperty, owl:DatatypeProperty;
  rdfs:comment "Zero sequence shunt (charging) conductance, uniformly distributed, of the entire line section."@en;
  rdfs:domain cim:ACLineSegment;
  rdfs:range xsd:float;
  rdfs:label "g0ch";
  cims:multiplicity cims:M:1..1;
  cim:unitMultiplier cim:UnitMultiplier.none;
  cim:unitSymbol cim:UnitSymbol.S;
  qudt:hasQuantityKind cim:Conductance;
  qudt:hasUnit unit:S .

cim:ACLineSegment.gch a owl:FunctionalProperty, owl:DatatypeProperty;
  rdfs:comment "Positive sequence shunt (charging) conductance, uniformly distributed, of the entire line section."@en;
  rdfs:domain cim:ACLineSegment;
  rdfs:range xsd:float;
  rdfs:label "gch";
  cims:multiplicity cims:M:0..1;
  cim:unitMultiplier cim:UnitMultiplier.none;
  cim:unitSymbol cim:UnitSymbol.S;
  qudt:hasQuantityKind cim:Conductance;
  qudt:hasUnit unit:S .

cim:ACLineSegment.r a owl:FunctionalProperty, owl:DatatypeProperty;
  rdfs:comment "Positive sequence series resistance of the entire line section."@en;
  rdfs:domain cim:ACLineSegment;
  rdfs:range xsd:float;
  rdfs:label "r";
  cims:multiplicity cims:M:1..1;
  cim:unitMultiplier cim:UnitMultiplier.none;
  cim:unitSymbol cim:UnitSymbol.ohm;
  qudt:hasQuantityKind cim:Resistance;
  qudt:hasUnit unit:OHM .

cim:ACLineSegment.r0 a owl:FunctionalProperty, owl:DatatypeProperty;
  rdfs:comment "Zero sequence series resistance of the entire line section."@en;
  rdfs:domain cim:ACLineSegment;
  rdfs:range xsd:float;
  rdfs:label "r0";
  cims:multiplicity cims:M:1..1;
  cim:unitMultiplier cim:UnitMultiplier.none;
  cim:unitSymbol cim:UnitSymbol.ohm;
  qudt:hasQuantityKind cim:Resistance;
  qudt:hasUnit unit:OHM .

cim:ACLineSegment.shortCircuitEndTemperature a owl:FunctionalProperty, owl:DatatypeProperty;
  rdfs:comment "Maximum permitted temperature at the end of SC for the calculation of minimum short-circuit currents. Used for short circuit data exchange according to IEC 60909."@en;
  rdfs:domain cim:ACLineSegment;
  rdfs:range xsd:float;
  rdfs:label "shortCircuitEndTemperature";
  cims:multiplicity cims:M:1..1;
  cim:unitMultiplier cim:UnitMultiplier.none;
  cim:unitSymbol cim:UnitSymbol.degC;
  qudt:hasQuantityKind cim:Temperature;
  qudt:hasUnit unit:DEG_C .

cim:ACLineSegment.x a owl:FunctionalProperty, owl:DatatypeProperty;
  rdfs:comment "Positive sequence series reactance of the entire line section."@en;
  rdfs:domain cim:ACLineSegment;
  rdfs:range xsd:float;
  rdfs:label "x";
  cims:multiplicity cims:M:1..1;
  cim:unitMultiplier cim:UnitMultiplier.none;
  cim:unitSymbol cim:UnitSymbol.ohm;
  qudt:hasQuantityKind cim:Reactance;
  qudt:hasUnit unit:OHM .

cim:ACLineSegment.x0 a owl:FunctionalProperty, owl:DatatypeProperty;
  rdfs:comment "Zero sequence series reactance of the entire line section."@en;
  rdfs:domain cim:ACLineSegment;
  rdfs:range xsd:float;
  rdfs:label "x0";
  cims:multiplicity cims:M:1..1;
  cim:unitMultiplier cim:UnitMultiplier.none;
  cim:unitSymbol cim:UnitSymbol.ohm;
  qudt:hasQuantityKind cim:Reactance;
  qudt:hasUnit unit:OHM .

cim:ActivePowerLimit a owl:Class;
  rdfs:comment "Limit on active power flow."@en;
  rdfs:subClassOf cim:OperationalLimit;
  rdfs:label "ActivePowerLimit" .

cim:ActivePowerLimit.normalValue a owl:FunctionalProperty, owl:DatatypeProperty;
  rdfs:comment "The normal value of active power limit. The attribute shall be a positive value or zero."@en;
  rdfs:domain cim:ActivePowerLimit;
  rdfs:range xsd:float;
  rdfs:label "normalValue";
  cims:multiplicity cims:M:1..1;
  cim:unitMultiplier cim:UnitMultiplier.M;
  cim:unitSymbol cim:UnitSymbol.W;
  qudt:hasQuantityKind cim:ActivePower;
  qudt:hasUnit unit:MegaW .

cim:ActivePowerLimit.value a owl:FunctionalProperty, owl:DatatypeProperty;
  rdfs:comment "Value of active power limit. The attribute shall be a positive value or zero."@en;
  rdfs:domain cim:ActivePowerLimit;
  rdfs:range xsd:float;
  rdfs:label "value";
  cims:multiplicity cims:M:1..1;
  cim:unitMultiplier cim:UnitMultiplier.M;
  cim:unitSymbol cim:UnitSymbol.W;
  qudt:hasQuantityKind cim:ActivePower;
  qudt:hasUnit unit:MegaW .

cim:Analog a owl:Class;
  rdfs:comment "Analog represents an analog Measurement."@en;
  rdfs:subClassOf cim:Measurement;
  rdfs:label "Analog" .

cim:Analog.AnalogValues a owl:ObjectProperty, owl:InverseFunctionalProperty;
  rdfs:comment "The values connected to this measurement."@en;
  rdfs:domain cim:Analog;
  rdfs:range cim:AnalogValue;
  rdfs:label "AnalogValues";
  cims:multiplicity cims:M:0..n;
  owl:inverseOf cim:AnalogValue.Analog .

cim:Analog.positiveFlowIn a owl:FunctionalProperty, owl:DatatypeProperty;
  rdfs:comment "If true then this measurement is an active power, reactive power or current with the convention that a positive value measured at the Terminal means power is flowing into the related PowerSystemResource."@en;
  rdfs:domain cim:Analog;
  rdfs:range xsd:boolean;
  rdfs:label "positiveFlowIn";
  cims:multiplicity cims:M:0..1;
  cims:pragmatics """For BiddingZoneBorder,
\"true\" means the flow is from BiddingZoneOne to BiddingZoneTwo.
\"false\" means the flow is in the opposite direction""" .

cim:AnalogValue a owl:Class;
  rdfs:comment "AnalogValue represents an analog MeasurementValue."@en;
  rdfs:subClassOf cim:MeasurementValue;
  rdfs:label "AnalogValue" .

cim:AnalogValue.Analog a owl:ObjectProperty, owl:FunctionalProperty;
  rdfs:comment "Measurement to which this value is connected."@en;
  rdfs:domain cim:AnalogValue;
  rdfs:range cim:Analog;
  rdfs:label "Analog";
  cims:multiplicity cims:M:1..1;
  owl:inverseOf cim:Analog.AnalogValues .

cim:Asset a owl:Class;
  rdfs:comment "Tangible resource of the utility, including power system equipment, various end devices, cabinets, buildings, etc. For electrical network equipment, the role of the asset is defined through PowerSystemResource and its subclasses, defined mainly in the Wires model (refer to IEC61970-301 and model package IEC61970::Wires). Asset description places emphasis on the physical characteristics of the equipment fulfilling that role."@en;
  rdfs:subClassOf cim:IdentifiedObject;
  rdfs:label "Asset" .

cim:Asset.AssetContainer a owl:ObjectProperty, owl:FunctionalProperty;
  rdfs:comment "Container of this asset."@en;
  rdfs:domain cim:Asset;
  rdfs:range cim:AssetContainer;
  rdfs:label "AssetContainer";
  cims:multiplicity cims:M:0..1;
  owl:inverseOf cim:AssetContainer.Assets .

cim:Asset.PowerSystemResources a owl:ObjectProperty;
  rdfs:comment "All power system resources used to electrically model this asset. For example, transformer asset is electrically modelled with a transformer and its windings and tap changer."@en;
  rdfs:domain cim:Asset;
  rdfs:range cim:PowerSystemResource;
  rdfs:label "PowerSystemResources";
  cims:multiplicity cims:M:0..n;
  owl:inverseOf cim:PowerSystemResource.Assets .

cim:Asset.inUseState a owl:ObjectProperty, owl:FunctionalProperty;
  rdfs:comment "Indication of whether asset is currently deployed (in use), ready to be put into use or not available for use."@en;
  rdfs:domain cim:Asset;
  rdfs:range cim:InUseStateKind;
  rdfs:label "inUseState";
  cims:multiplicity cims:M:0..1 .

cim:Asset.serialNumber a owl:ObjectProperty, owl:FunctionalProperty;
  rdfs:comment "Serial number of this asset."@en;
  rdfs:domain cim:Asset;
  rdfs:label "serialNumber";
  cims:multiplicity cims:M:0..1;
  cims:dataType cim:String .

cim:Asset.type a owl:ObjectProperty, owl:FunctionalProperty;
  rdfs:comment "Utility-specific classification of Asset and its subtypes, according to their corporate standards, practices, and existing IT systems (e.g., for management of assets, maintenance, work, outage, customers, etc.)."@en;
  rdfs:domain cim:Asset;
  rdfs:label "type";
  cims:multiplicity cims:M:0..1;
  cims:dataType cim:String .

cim:AssetContainer a owl:Class;
  rdfs:comment "Asset that is aggregation of other assets such as conductors, transformers, switchgear, land, fences, buildings, equipment, vehicles, etc."@en;
  rdfs:subClassOf cim:Asset;
  rdfs:label "AssetContainer" .

cim:AssetContainer.Assets a owl:ObjectProperty, owl:InverseFunctionalProperty;
  rdfs:comment "All assets within this container asset."@en;
  rdfs:domain cim:AssetContainer;
  rdfs:range cim:Asset;
  rdfs:label "Assets";
  cims:multiplicity cims:M:0..n;
  owl:inverseOf cim:Asset.AssetContainer .

cim:AssetInfo a owl:Class;
  rdfs:comment """Set of attributes of an asset, representing typical datasheet information of a physical device that can be instantiated and shared in different data exchange contexts:
- as attributes of an asset instance (installed or in stock)
- as attributes of an asset model (product by a manufacturer)
- as attributes of a type asset (generic type of an asset as used in designs/extension planning)."""@en;
  rdfs:subClassOf cim:IdentifiedObject;
  rdfs:label "AssetInfo" .

cim:AssetInfo.ProductAssetModel a owl:ObjectProperty, owl:InverseFunctionalProperty,
    owl:FunctionalProperty;
  rdfs:comment "Product asset model which conforms to this catalog asset type."@en;
  rdfs:domain cim:AssetInfo;
  rdfs:range cim:ProductAssetModel;
  rdfs:label "ProductAssetModel";
  cims:multiplicity cims:M:0..1;
  owl:inverseOf cim:ProductAssetModel.AssetInfo .

cim:AssetModelUsageKind a owl:Class;
  rdfs:comment "Usage for an asset model."@en;
  rdfs:label "AssetModelUsageKind" .

cim:AssetModelUsageKind.transmission a cim:AssetModelUsageKind;
  rdfs:comment "Asset model is intended for use in transmission network."@en;
  rdfs:label "transmission" .

cim:AssetOrganisationRole a owl:Class;
  rdfs:comment "Role an organisation plays with respect to asset."@en;
  rdfs:subClassOf cim:OrganisationRole;
  rdfs:label "AssetOrganisationRole" .

cim:AssetOwner a owl:Class;
  rdfs:comment "Owner of the asset."@en;
  rdfs:subClassOf cim:AssetOrganisationRole;
  rdfs:label "AssetOwner" .

cim:AsynchronousMachineKind a owl:Class;
  rdfs:comment "Kind of Asynchronous Machine."@en;
  rdfs:label "AsynchronousMachineKind" .

cim:AuxiliaryEquipment a owl:Class;
  rdfs:comment """AuxiliaryEquipment describe equipment that is not performing any primary functions but support for the equipment performing the primary function.
AuxiliaryEquipment is attached to primary equipment via an association with Terminal."""@en;
  rdfs:subClassOf cim:Equipment;
  rdfs:label "AuxiliaryEquipment" .

cim:AuxiliaryEquipment.Terminal a owl:ObjectProperty, owl:FunctionalProperty;
  rdfs:comment "The Terminal at the equipment where the AuxiliaryEquipment is attached."@en;
  rdfs:domain cim:AuxiliaryEquipment;
  rdfs:range cim:Terminal;
  rdfs:label "Terminal";
  cims:multiplicity cims:M:1..1;
  owl:inverseOf cim:Terminal.AuxiliaryEquipment .

cim:BaseVoltage a owl:Class;
  rdfs:comment "Defines a system base voltage which is referenced."@en;
  rdfs:subClassOf cim:IdentifiedObject;
  rdfs:label "BaseVoltage" .

cim:BaseVoltage.ConductingEquipment a owl:ObjectProperty, owl:InverseFunctionalProperty;
  rdfs:comment "All conducting equipment with this base voltage.  Use only when there is no voltage level container used and only one base voltage applies.  For example, not used for transformers."@en;
  rdfs:domain cim:BaseVoltage;
  rdfs:range cim:ConductingEquipment;
  rdfs:label "ConductingEquipment";
  cims:multiplicity cims:M:0..n;
  owl:inverseOf cim:ConductingEquipment.BaseVoltage .

cim:BaseVoltage.TopologicalNode a owl:ObjectProperty, owl:InverseFunctionalProperty;
  rdfs:comment "The topological nodes at the base voltage."@en;
  rdfs:domain cim:BaseVoltage;
  rdfs:range cim:TopologicalNode;
  rdfs:label "TopologicalNode";
  cims:multiplicity cims:M:0..n;
  owl:inverseOf cim:TopologicalNode.BaseVoltage .

cim:BaseVoltage.TransformerEnds a owl:ObjectProperty, owl:InverseFunctionalProperty;
  rdfs:comment "Transformer ends at the base voltage.  This is essential for PU calculation."@en;
  rdfs:domain cim:BaseVoltage;
  rdfs:range cim:TransformerEnd;
  rdfs:label "TransformerEnds";
  cims:multiplicity cims:M:0..n;
  owl:inverseOf cim:TransformerEnd.BaseVoltage .

cim:BaseVoltage.VoltageLevel a owl:ObjectProperty, owl:InverseFunctionalProperty;
  rdfs:comment "The voltage levels having this base voltage."@en;
  rdfs:domain cim:BaseVoltage;
  rdfs:range cim:VoltageLevel;
  rdfs:label "VoltageLevel";
  cims:multiplicity cims:M:0..n;
  owl:inverseOf cim:VoltageLevel.BaseVoltage .

cim:BaseVoltage.nominalVoltage a owl:FunctionalProperty, owl:DatatypeProperty;
  rdfs:comment "The power system resource's base voltage.  Shall be a positive value and not zero."@en;
  rdfs:domain cim:BaseVoltage;
  rdfs:range xsd:float;
  rdfs:label "nominalVoltage";
  cims:multiplicity cims:M:1..1;
  cim:unitMultiplier cim:UnitMultiplier.k;
  cim:unitSymbol cim:UnitSymbol.V;
  qudt:hasQuantityKind cim:Voltage;
  qudt:hasUnit unit:KiloV .

cim:BatteryStateKind a owl:Class;
  rdfs:comment "The state of the battery unit."@en;
  rdfs:label "BatteryStateKind" .

cim:Bay a owl:Class;
  rdfs:comment "A collection of power system resources (within a given substation) including conducting equipment, protection relays, measurements, and telemetry.  A bay typically represents a physical grouping related to modularization of equipment."@en;
  rdfs:subClassOf cim:EquipmentContainer;
  rdfs:label "Bay" .

cim:Bay.VoltageLevel a owl:ObjectProperty, owl:FunctionalProperty;
  rdfs:comment "The voltage level containing this bay."@en;
  rdfs:domain cim:Bay;
  rdfs:range cim:VoltageLevel;
  rdfs:label "VoltageLevel";
  cims:multiplicity cims:M:1..1;
  owl:inverseOf cim:VoltageLevel.Bays .

cim:Breaker a owl:Class;
  rdfs:comment "A mechanical switching device capable of making, carrying, and breaking currents under normal circuit conditions and also making, carrying for a specified time, and breaking currents under specified abnormal circuit conditions e.g.  those of short circuit."@en;
  rdfs:subClassOf cim:ProtectedSwitch;
  rdfs:label "Breaker" .

cim:BusbarSection a owl:Class;
  rdfs:comment """A conductor, or group of conductors, with negligible impedance, that serve to connect other conducting equipment within a single substation. 
Voltage measurements are typically obtained from voltage transformers that are connected to busbar sections. A bus bar section may have many physical terminals but for analysis is modelled with exactly one logical terminal."""@en;
  rdfs:subClassOf cim:Connector;
  rdfs:label "BusbarSection" .

cim:BusbarSection.ipMax a owl:FunctionalProperty, owl:DatatypeProperty;
  rdfs:comment """Maximum allowable peak short-circuit current of busbar (Ipmax in IEC 60909-0). 
Mechanical limit of the busbar in the substation itself. Used for short circuit data exchange according to IEC 60909."""@en;
  rdfs:domain cim:BusbarSection;
  rdfs:range xsd:float;
  rdfs:label "ipMax";
  cims:multiplicity cims:M:0..1;
  cim:unitMultiplier cim:UnitMultiplier.none;
  cim:unitSymbol cim:UnitSymbol.A;
  qudt:hasQuantityKind cim:CurrentFlow;
  qudt:hasUnit unit:A .

cim:CableInfo a owl:Class;
  rdfs:comment "Cable data."@en;
  rdfs:subClassOf cim:WireInfo;
  rdfs:label "CableInfo" .

cim:ConductingEquipment a owl:Class;
  rdfs:comment "The parts of the AC power system that are designed to carry current or that are conductively connected through terminals."@en;
  rdfs:subClassOf cim:Equipment;
  rdfs:label "ConductingEquipment";
  cims:pragmatics "This means only AC Conducting Equipment (not DC)" .

cim:ConductingEquipment.BaseVoltage a owl:ObjectProperty, owl:FunctionalProperty;
  rdfs:comment "Base voltage of this conducting equipment.  Use only when there is no voltage level container used and only one base voltage applies.  For example, not used for transformers."@en;
  rdfs:domain cim:ConductingEquipment;
  rdfs:range cim:BaseVoltage;
  rdfs:label "BaseVoltage";
  cims:multiplicity cims:M:0..1;
  owl:inverseOf cim:BaseVoltage.ConductingEquipment .

cim:ConductingEquipment.SvStatus a owl:ObjectProperty, owl:InverseFunctionalProperty,
    owl:FunctionalProperty;
  rdfs:comment "The status state variable associated with this conducting equipment."@en;
  rdfs:domain cim:ConductingEquipment;
  rdfs:range cim:SvStatus;
  rdfs:label "SvStatus";
  cims:multiplicity cims:M:0..1;
  owl:inverseOf cim:SvStatus.ConductingEquipment .

cim:ConductingEquipment.Terminals a owl:ObjectProperty, owl:InverseFunctionalProperty;
  rdfs:comment "Conducting equipment have terminals that may be connected to other conducting equipment terminals via connectivity nodes or topological nodes."@en;
  rdfs:domain cim:ConductingEquipment;
  rdfs:range cim:Terminal;
  rdfs:label "Terminals";
  cims:multiplicity cims:M:0..n;
  owl:inverseOf cim:Terminal.ConductingEquipment .

cim:Conductor a owl:Class;
  rdfs:comment "Combination of conducting material with consistent electrical characteristics, building a single electrical system, used to carry current between points in the power system."@en;
  rdfs:subClassOf cim:ConductingEquipment;
  rdfs:label "Conductor" .

cim:Conductor.length a owl:FunctionalProperty, owl:DatatypeProperty;
  rdfs:comment "Segment length for calculating line section capabilities."@en;
  rdfs:domain cim:Conductor;
  rdfs:range xsd:float;
  rdfs:label "length";
  cims:multiplicity cims:M:0..1;
  cim:unitMultiplier cim:UnitMultiplier.k;
  cim:unitSymbol cim:UnitSymbol.m;
  qudt:hasQuantityKind cim:Length;
  qudt:hasUnit unit:KiloM .

cim:ConformLoad a owl:Class;
  rdfs:comment "ConformLoad represent loads that follow a daily load change pattern where the pattern can be used to scale the load with a system load."@en;
  rdfs:subClassOf cim:EnergyConsumer;
  rdfs:label "ConformLoad" .

cim:ConformLoad.LoadGroup a owl:ObjectProperty, owl:FunctionalProperty;
  rdfs:comment "Group of this ConformLoad."@en;
  rdfs:domain cim:ConformLoad;
  rdfs:range cim:ConformLoadGroup;
  rdfs:label "LoadGroup";
  cims:multiplicity cims:M:1..1;
  owl:inverseOf cim:ConformLoadGroup.EnergyConsumers .

cim:ConformLoadGroup a owl:Class;
  rdfs:comment "A group of loads conforming to an allocation pattern."@en;
  rdfs:subClassOf cim:LoadGroup;
  rdfs:label "ConformLoadGroup" .

cim:ConformLoadGroup.EnergyConsumers a owl:ObjectProperty, owl:InverseFunctionalProperty;
  rdfs:comment "Conform loads assigned to this ConformLoadGroup."@en;
  rdfs:domain cim:ConformLoadGroup;
  rdfs:range cim:ConformLoad;
  rdfs:label "EnergyConsumers";
  cims:multiplicity cims:M:1..n;
  owl:inverseOf cim:ConformLoad.LoadGroup .

cim:ConnectivityNode a owl:Class;
  rdfs:comment "Connectivity nodes are points where terminals of AC conducting equipment are connected together with zero impedance."@en;
  rdfs:subClassOf cim:IdentifiedObject;
  rdfs:label "ConnectivityNode" .

cim:ConnectivityNode.ConnectivityNodeContainer a owl:ObjectProperty, owl:FunctionalProperty;
  rdfs:comment "Container of this connectivity node."@en;
  rdfs:domain cim:ConnectivityNode;
  rdfs:range cim:ConnectivityNodeContainer;
  rdfs:label "ConnectivityNodeContainer";
  cims:multiplicity cims:M:1..1;
  owl:inverseOf cim:ConnectivityNodeContainer.ConnectivityNodes .

cim:ConnectivityNode.Terminals a owl:ObjectProperty, owl:InverseFunctionalProperty;
  rdfs:comment "Terminals interconnected with zero impedance at a this connectivity node."@en;
  rdfs:domain cim:ConnectivityNode;
  rdfs:range cim:Terminal;
  rdfs:label "Terminals";
  cims:multiplicity cims:M:0..n;
  owl:inverseOf cim:Terminal.ConnectivityNode .

cim:ConnectivityNode.TopologicalNode a owl:ObjectProperty, owl:FunctionalProperty;
  rdfs:comment "The topological node to which this connectivity node is assigned.  May depend on the current state of switches in the network."@en;
  rdfs:domain cim:ConnectivityNode;
  rdfs:range cim:TopologicalNode;
  rdfs:label "TopologicalNode";
  cims:multiplicity cims:M:1..1;
  owl:inverseOf cim:TopologicalNode.ConnectivityNodes .

cim:ConnectivityNodeContainer a owl:Class;
  rdfs:comment "A base class for all objects that may contain connectivity nodes or topological nodes."@en;
  rdfs:subClassOf cimr:EquipmentOrContainer;
  rdfs:label "ConnectivityNodeContainer" .

cim:ConnectivityNodeContainer.ConnectivityNodes a owl:ObjectProperty, owl:InverseFunctionalProperty;
  rdfs:comment "Connectivity nodes which belong to this connectivity node container."@en;
  rdfs:domain cim:ConnectivityNodeContainer;
  rdfs:range cim:ConnectivityNode;
  rdfs:label "ConnectivityNodes";
  cims:multiplicity cims:M:0..n;
  owl:inverseOf cim:ConnectivityNode.ConnectivityNodeContainer .

cim:ConnectivityNodeContainer.TopologicalNode a owl:ObjectProperty, owl:InverseFunctionalProperty;
  rdfs:comment "The topological nodes which belong to this connectivity node container."@en;
  rdfs:domain cim:ConnectivityNodeContainer;
  rdfs:range cim:TopologicalNode;
  rdfs:label "TopologicalNode";
  cims:multiplicity cims:M:0..n;
  owl:inverseOf cim:TopologicalNode.ConnectivityNodeContainer .

cim:Connector a owl:Class;
  rdfs:comment "A conductor, or group of conductors, with negligible impedance, that serve to connect other conducting equipment within a single substation and are modelled with a single logical terminal."@en;
  rdfs:subClassOf cim:ConductingEquipment;
  rdfs:label "Connector" .

cim:Contingency a owl:Class;
  rdfs:comment "An event threatening system reliability, consisting of one or more contingency elements."@en;
  rdfs:subClassOf cim:IdentifiedObject;
  rdfs:label "Contingency" .

cim:Contingency.ContingencyElement a owl:ObjectProperty, owl:InverseFunctionalProperty;
  rdfs:comment "A contingency can have any number of contingency elements."@en;
  rdfs:domain cim:Contingency;
  rdfs:range cim:ContingencyElement;
  rdfs:label "ContingencyElement";
  cims:multiplicity cims:M:1..n;
  owl:inverseOf cim:ContingencyElement.Contingency .

cim:Contingency.mustStudy a owl:FunctionalProperty, owl:DatatypeProperty;
  rdfs:comment "Set true if must study this contingency."@en;
  rdfs:domain cim:Contingency;
  rdfs:range xsd:boolean;
  rdfs:label "mustStudy";
  cims:multiplicity cims:M:1..1 .

cim:ContingencyElement a owl:Class;
  rdfs:comment "An element of a system event to be studied by contingency analysis, representing a change in status of a single piece of equipment."@en;
  rdfs:subClassOf cim:IdentifiedObject;
  rdfs:label "ContingencyElement" .

cim:ContingencyElement.Contingency a owl:ObjectProperty, owl:FunctionalProperty;
  rdfs:comment "A contingency element belongs to one contingency."@en;
  rdfs:domain cim:ContingencyElement;
  rdfs:range cim:Contingency;
  rdfs:label "Contingency";
  cims:multiplicity cims:M:1..1;
  owl:inverseOf cim:Contingency.ContingencyElement .

cim:ContingencyEquipment a owl:Class;
  rdfs:comment "Equipment whose in service status is to change, such as a power transformer or AC line segment."@en;
  rdfs:subClassOf cim:ContingencyElement;
  rdfs:label "ContingencyEquipment" .

cim:ContingencyEquipment.Equipment a owl:ObjectProperty, owl:FunctionalProperty;
  rdfs:comment "The single piece of equipment to which to apply the contingency."@en;
  rdfs:domain cim:ContingencyEquipment;
  rdfs:range cim:Equipment;
  rdfs:label "Equipment";
  cims:multiplicity cims:M:1..1;
  owl:inverseOf cim:Equipment.ContingencyEquipment .

cim:ContingencyEquipment.contingentStatus a owl:ObjectProperty, owl:FunctionalProperty;
  rdfs:comment "The status for the associated equipment when in the contingency state.   This status is independent of the case to which the contingency is originally applied, but defines the equipment status when the contingency is applied."@en;
  rdfs:domain cim:ContingencyEquipment;
  rdfs:range cim:ContingencyEquipmentStatusKind;
  rdfs:label "contingentStatus";
  cims:multiplicity cims:M:1..1 .

cim:ContingencyEquipmentStatusKind a owl:Class;
  rdfs:comment "Indicates the state which the contingency equipment is to be in when the contingency is applied."@en;
  rdfs:label "ContingencyEquipmentStatusKind" .

cim:ContingencyEquipmentStatusKind.outOfService a cim:ContingencyEquipmentStatusKind;
  rdfs:comment "The equipment is to be taken out of service."@en;
  rdfs:label "outOfService" .

cim:ControlArea a owl:Class;
  rdfs:comment "A control area is a grouping of generating units and/or loads and a cutset of tie lines (as terminals) which may be used for a variety of purposes including automatic generation control, power flow solution area interchange control specification, and input to load forecasting. All generation and load within the area defined by the terminals on the border are considered in the area interchange control. Note that any number of overlapping control area specifications can be superimposed on the physical"@en;
  rdfs:subClassOf cim:PowerSystemResource;
  rdfs:label "ControlArea" .

cim:ControlArea.ControlAreaGeneratingUnit a owl:ObjectProperty, owl:InverseFunctionalProperty;
  rdfs:comment "The generating unit specifications for the control area."@en;
  rdfs:domain cim:ControlArea;
  rdfs:range cim:ControlAreaGeneratingUnit;
  rdfs:label "ControlAreaGeneratingUnit";
  cims:multiplicity cims:M:0..n;
  owl:inverseOf cim:ControlAreaGeneratingUnit.ControlArea .

cim:ControlArea.EnergyArea a owl:ObjectProperty, owl:InverseFunctionalProperty, owl:FunctionalProperty;
  rdfs:comment "The energy area that is forecast from this control area specification."@en;
  rdfs:domain cim:ControlArea;
  rdfs:range cim:EnergyArea;
  rdfs:label "EnergyArea";
  cims:multiplicity cims:M:1..1;
  owl:inverseOf cim:EnergyArea.ControlArea .

cim:ControlArea.netInterchange a owl:FunctionalProperty, owl:DatatypeProperty;
  rdfs:comment "The specified positive net interchange into the control area, i.e. positive sign means flow into the area."@en;
  rdfs:domain cim:ControlArea;
  rdfs:range xsd:float;
  rdfs:label "netInterchange";
  cims:multiplicity cims:M:1..1;
  cim:unitMultiplier cim:UnitMultiplier.M;
  cim:unitSymbol cim:UnitSymbol.W;
  qudt:hasQuantityKind cim:ActivePower;
  qudt:hasUnit unit:MegaW .

cim:ControlArea.pTolerance a owl:FunctionalProperty, owl:DatatypeProperty;
  rdfs:comment "Active power net interchange tolerance. The attribute shall be a positive value or zero."@en;
  rdfs:domain cim:ControlArea;
  rdfs:range xsd:float;
  rdfs:label "pTolerance";
  cims:multiplicity cims:M:0..1;
  cim:unitMultiplier cim:UnitMultiplier.M;
  cim:unitSymbol cim:UnitSymbol.W;
  qudt:hasQuantityKind cim:ActivePower;
  qudt:hasUnit unit:MegaW .

cim:ControlArea.type a owl:ObjectProperty, owl:FunctionalProperty;
  rdfs:comment "The primary type of control area definition used to determine if this is used for automatic generation control, for planning interchange control, or other purposes.   A control area specified with primary type of automatic generation control could still be forecast and used as an interchange area in power flow analysis."@en;
  rdfs:domain cim:ControlArea;
  rdfs:range cim:ControlAreaTypeKind;
  rdfs:label "type";
  cims:multiplicity cims:M:1..1 .

cim:ControlAreaGeneratingUnit a owl:Class;
  rdfs:comment "A control area generating unit. This class is needed so that alternate control area definitions may include the same generating unit.   It should be noted that only one instance within a control area should reference a specific generating unit."@en;
  rdfs:subClassOf cim:IdentifiedObject;
  rdfs:label "ControlAreaGeneratingUnit" .

cim:ControlAreaGeneratingUnit.ControlArea a owl:ObjectProperty, owl:FunctionalProperty;
  rdfs:comment "The parent control area for the generating unit specifications."@en;
  rdfs:domain cim:ControlAreaGeneratingUnit;
  rdfs:range cim:ControlArea;
  rdfs:label "ControlArea";
  cims:multiplicity cims:M:1..1;
  owl:inverseOf cim:ControlArea.ControlAreaGeneratingUnit .

cim:ControlAreaGeneratingUnit.GeneratingUnit a owl:ObjectProperty, owl:FunctionalProperty;
  rdfs:comment "The generating unit specified for this control area.  Note that a control area should include a GeneratingUnit only once."@en;
  rdfs:domain cim:ControlAreaGeneratingUnit;
  rdfs:range cim:GeneratingUnit;
  rdfs:label "GeneratingUnit";
  cims:multiplicity cims:M:1..1;
  owl:inverseOf cim:GeneratingUnit.ControlAreaGeneratingUnit .

cim:ControlAreaTypeKind a owl:Class;
  rdfs:comment "The type of control area."@en;
  rdfs:label "ControlAreaTypeKind" .

cim:ControlAreaTypeKind.Interchange a cim:ControlAreaTypeKind;
  rdfs:comment "Used for interchange specification or control."@en;
  rdfs:label "Interchange" .

cim:CoordinateSystem a owl:Class;
  rdfs:comment "Coordinate reference system."@en;
  rdfs:subClassOf cim:IdentifiedObject;
  rdfs:label "CoordinateSystem" .

cim:CoordinateSystem.Locations a owl:ObjectProperty, owl:InverseFunctionalProperty;
  rdfs:comment "All locations described with position points in this coordinate system."@en;
  rdfs:domain cim:CoordinateSystem;
  rdfs:range cim:Location;
  rdfs:label "Locations";
  cims:multiplicity cims:M:0..n;
  owl:inverseOf cim:Location.CoordinateSystem .

cim:CoordinateSystem.crsUrn a owl:FunctionalProperty, owl:DatatypeProperty;
  rdfs:comment "A Uniform Resource Name (URN) for the coordinate reference system (crs) used to define 'Location.PositionPoints'. An example would be the European Petroleum Survey Group (EPSG) code for a coordinate reference system, defined in URN under the Open Geospatial Consortium (OGC) namespace as: urn:ogc:def:crs:EPSG::XXXX, where XXXX is an EPSG code (a full list of codes can be found at the EPSG Registry web site http://www.epsg-registry.org/). To define the coordinate system as being WGS84 (latitude, longitude)"@en;
  rdfs:domain cim:CoordinateSystem;
  rdfs:range xsd:string;
  rdfs:label "crsUrn";
  cims:multiplicity cims:M:1..1 .

cim:CsOperatingModeKind a owl:Class;
  rdfs:comment "Operating mode for HVDC line operating as Current Source Converter."@en;
  rdfs:label "CsOperatingModeKind" .

cim:CsPpccControlKind a owl:Class;
  rdfs:comment "Active power control modes for HVDC line operating as Current Source Converter."@en;
  rdfs:label "CsPpccControlKind" .

cim:Currency a owl:Class;
  rdfs:comment "Monetary currencies.  ISO 4217 standard including 3-character currency code."@en;
  rdfs:label "Currency" .

cim:CurrentLimit a owl:Class;
  rdfs:comment "Operational limit on current."@en;
  rdfs:subClassOf cim:OperationalLimit;
  rdfs:label "CurrentLimit" .

cim:CurrentLimit.normalValue a owl:FunctionalProperty, owl:DatatypeProperty;
  rdfs:comment "The normal value for limit on current flow. The attribute shall be a positive value or zero."@en;
  rdfs:domain cim:CurrentLimit;
  rdfs:range xsd:float;
  rdfs:label "normalValue";
  cims:multiplicity cims:M:1..1;
  cim:unitMultiplier cim:UnitMultiplier.none;
  cim:unitSymbol cim:UnitSymbol.A;
  qudt:hasQuantityKind cim:CurrentFlow;
  qudt:hasUnit unit:A .

cim:CurrentLimit.value a owl:FunctionalProperty, owl:DatatypeProperty;
  rdfs:comment "Limit on current flow. The attribute shall be a positive value or zero."@en;
  rdfs:domain cim:CurrentLimit;
  rdfs:range xsd:float;
  rdfs:label "value";
  cims:multiplicity cims:M:1..1;
  cim:unitMultiplier cim:UnitMultiplier.none;
  cim:unitSymbol cim:UnitSymbol.A;
  qudt:hasQuantityKind cim:CurrentFlow;
  qudt:hasUnit unit:A .

cim:CurrentTransformer a owl:Class;
  rdfs:comment "Instrument transformer used to measure electrical qualities of the circuit that is being protected and/or monitored. Typically used as current transducer for the purpose of metering or protection. A typical secondary current rating would be 5A."@en;
  rdfs:subClassOf cim:Sensor;
  rdfs:label "CurrentTransformer" .

cim:Curve a owl:Class;
  rdfs:comment "A multi-purpose curve or functional relationship between an independent variable (X-axis) and dependent (Y-axis) variables."@en;
  rdfs:subClassOf cim:IdentifiedObject;
  rdfs:label "Curve" .

cim:Curve.CurveDatas a owl:ObjectProperty, owl:InverseFunctionalProperty;
  rdfs:comment "The point data values that define this curve."@en;
  rdfs:domain cim:Curve;
  rdfs:range cim:CurveData;
  rdfs:label "CurveDatas";
  cims:multiplicity cims:M:1..n;
  owl:inverseOf cim:CurveData.Curve .

cim:Curve.curveStyle a owl:ObjectProperty, owl:FunctionalProperty;
  rdfs:comment "The style or shape of the curve."@en;
  rdfs:domain cim:Curve;
  rdfs:range cim:CurveStyle;
  rdfs:label "curveStyle";
  cims:multiplicity cims:M:1..1 .

cim:Curve.xUnit a owl:ObjectProperty, owl:FunctionalProperty;
  rdfs:comment "The X-axis units of measure."@en;
  rdfs:domain cim:Curve;
  rdfs:range cim:UnitSymbol;
  rdfs:label "xUnit";
  cims:multiplicity cims:M:1..1 .

cim:Curve.y2Unit a owl:ObjectProperty, owl:FunctionalProperty;
  rdfs:comment "The Y2-axis units of measure."@en;
  rdfs:domain cim:Curve;
  rdfs:range cim:UnitSymbol;
  rdfs:label "y2Unit";
  cims:multiplicity cims:M:0..1 .

cim:CurveData a owl:Class;
  rdfs:comment "Multi-purpose data points for defining a curve.  The use of this generic class is discouraged if a more specific class can be used to specify the X and Y axis values along with their specific data types."@en;
  rdfs:label "CurveData" .

cim:CurveData.Curve a owl:ObjectProperty, owl:FunctionalProperty;
  rdfs:comment "The curve of  this curve data point."@en;
  rdfs:domain cim:CurveData;
  rdfs:range cim:Curve;
  rdfs:label "Curve";
  cims:multiplicity cims:M:1..1;
  owl:inverseOf cim:Curve.CurveDatas .

cim:CurveStyle a owl:Class;
  rdfs:comment "Style or shape of curve."@en;
  rdfs:label "CurveStyle" .

cim:DCConverterOperatingModeKind a owl:Class;
  rdfs:comment "The operating mode of an HVDC bipole."@en;
  rdfs:label "DCConverterOperatingModeKind" .

cim:DCPolarityKind a owl:Class;
  rdfs:comment "Polarity for DC circuits."@en;
  rdfs:label "DCPolarityKind" .

cim:Diagram a owl:Class;
  rdfs:comment "The diagram being exchanged. The coordinate system is a standard Cartesian coordinate system and the orientation attribute defines the orientation. The initial view related attributes can be used to specify an initial view with the x,y coordinates of the diagonal points."@en;
  rdfs:subClassOf cim:IdentifiedObject;
  rdfs:label "Diagram" .

cim:Diagram.DiagramElements a owl:ObjectProperty, owl:InverseFunctionalProperty;
  rdfs:comment "A diagram is made up of multiple diagram objects."@en;
  rdfs:domain cim:Diagram;
  rdfs:range cim:DiagramObject;
  rdfs:label "DiagramElements";
  cims:multiplicity cims:M:0..n;
  owl:inverseOf cim:DiagramObject.Diagram .

cim:Diagram.orientation a owl:ObjectProperty, owl:FunctionalProperty;
  rdfs:comment "Coordinate system orientation of the diagram. A positive orientation gives standard “right-hand” orientation, with negative orientation indicating a “left-hand” orientation. For 2D diagrams, a positive orientation will result in X values increasing from left to right and Y values increasing from bottom to top. A negative orientation gives the “left-hand” orientation (favoured by computer graphics displays) with X values increasing from left to right and Y values increasing from top to bottom."@en;
  rdfs:domain cim:Diagram;
  rdfs:range cim:OrientationKind;
  rdfs:label "orientation";
  cims:multiplicity cims:M:1..1 .

cim:DiagramObject a owl:Class;
  rdfs:comment "An object that defines one or more points in a given space. This object can be associated with anything that specializes IdentifiedObject. For single line diagrams such objects typically include such items as analog values, breakers, disconnectors, power transformers, and transmission lines."@en;
  rdfs:subClassOf cim:IdentifiedObject;
  rdfs:label "DiagramObject" .

cim:DiagramObject.Diagram a owl:ObjectProperty, owl:FunctionalProperty;
  rdfs:comment "A diagram object is part of a diagram."@en;
  rdfs:domain cim:DiagramObject;
  rdfs:range cim:Diagram;
  rdfs:label "Diagram";
  cims:multiplicity cims:M:1..1;
  owl:inverseOf cim:Diagram.DiagramElements .

cim:DiagramObject.DiagramObjectPoints a owl:ObjectProperty, owl:InverseFunctionalProperty;
  rdfs:comment "A diagram object can have 0 or more points to reflect its layout position, routing (for polylines) or boundary (for polygons)."@en;
  rdfs:domain cim:DiagramObject;
  rdfs:range cim:DiagramObjectPoint;
  rdfs:label "DiagramObjectPoints";
  cims:multiplicity cims:M:0..n;
  owl:inverseOf cim:DiagramObjectPoint.DiagramObject .

cim:DiagramObject.DiagramObjectStyle a owl:ObjectProperty, owl:FunctionalProperty;
  rdfs:comment "A diagram object has a style associated that provides a reference for the style used in the originating system."@en;
  rdfs:domain cim:DiagramObject;
  rdfs:range cim:DiagramObjectStyle;
  rdfs:label "DiagramObjectStyle";
  cims:multiplicity cims:M:0..1;
  owl:inverseOf cim:DiagramObjectStyle.StyledObjects .

cim:DiagramObject.IdentifiedObject a owl:ObjectProperty, owl:FunctionalProperty;
  rdfs:comment "The domain object to which this diagram object is associated."@en;
  rdfs:domain cim:DiagramObject;
  rdfs:range cim:IdentifiedObject;
  rdfs:label "IdentifiedObject";
  cims:multiplicity cims:M:0..1;
  owl:inverseOf cim:IdentifiedObject.DiagramObjects .

cim:DiagramObject.rotation a owl:FunctionalProperty, owl:DatatypeProperty;
  rdfs:comment "Sets the angle of rotation of the diagram object.  Zero degrees is pointing to the top of the diagram.  Rotation is clockwise.  DiagramObject.rotation=0 has the following meaning: The connection point of an element which has one terminal is pointing to the top side of the diagram. The connection point \"From side\" of an element which has more than one terminal is pointing to the top side of the diagram. DiagramObject.rotation=90 has the following meaning: The connection point of an element which has"@en;
  rdfs:domain cim:DiagramObject;
  rdfs:range xsd:float;
  rdfs:label "rotation";
  cims:multiplicity cims:M:0..1;
  cim:unitMultiplier cim:UnitMultiplier.none;
  cim:unitSymbol cim:UnitSymbol.deg;
  qudt:hasQuantityKind cim:AngleDegrees;
  qudt:hasUnit unit:DEG .

cim:DiagramObjectPoint a owl:Class;
  rdfs:comment "A point in a given space defined by 3 coordinates and associated to a diagram object.  The coordinates may be positive or negative as the origin does not have to be in the corner of a diagram."@en;
  rdfs:label "DiagramObjectPoint" .

cim:DiagramObjectPoint.DiagramObject a owl:ObjectProperty, owl:FunctionalProperty;
  rdfs:comment "The diagram object with which the points are associated."@en;
  rdfs:domain cim:DiagramObjectPoint;
  rdfs:range cim:DiagramObject;
  rdfs:label "DiagramObject";
  cims:multiplicity cims:M:1..1;
  owl:inverseOf cim:DiagramObject.DiagramObjectPoints .

cim:DiagramObjectPoint.sequenceNumber a owl:FunctionalProperty, owl:DatatypeProperty;
  rdfs:comment "The sequence position of the point, used for defining the order of points for diagram objects acting as a polyline or polygon with more than one point. The attribute shall be a positive value."@en;
  rdfs:domain cim:DiagramObjectPoint;
  rdfs:range xsd:integer;
  rdfs:label "sequenceNumber";
  cims:multiplicity cims:M:0..1 .

cim:DiagramObjectPoint.xPosition a owl:FunctionalProperty, owl:DatatypeProperty;
  rdfs:comment "The X coordinate of this point."@en;
  rdfs:domain cim:DiagramObjectPoint;
  rdfs:range xsd:float;
  rdfs:label "xPosition";
  cims:multiplicity cims:M:1..1 .

cim:DiagramObjectPoint.yPosition a owl:FunctionalProperty, owl:DatatypeProperty;
  rdfs:comment "The Y coordinate of this point."@en;
  rdfs:domain cim:DiagramObjectPoint;
  rdfs:range xsd:float;
  rdfs:label "yPosition";
  cims:multiplicity cims:M:1..1 .

cim:DiagramObjectStyle a owl:Class;
  rdfs:comment "A reference to a style used by the originating system for a diagram object.  A diagram object style describes information such as line thickness, shape such as circle or rectangle etc, and colour."@en;
  rdfs:subClassOf cim:IdentifiedObject;
  rdfs:label "DiagramObjectStyle" .

cim:DiagramObjectStyle.StyledObjects a owl:ObjectProperty, owl:InverseFunctionalProperty;
  rdfs:comment "A style can be assigned to multiple diagram objects."@en;
  rdfs:domain cim:DiagramObjectStyle;
  rdfs:range cim:DiagramObject;
  rdfs:label "StyledObjects";
  cims:multiplicity cims:M:0..n;
  owl:inverseOf cim:DiagramObject.DiagramObjectStyle .

cim:Disconnector a owl:Class;
  rdfs:comment "A manually operated or motor operated mechanical switching device used for changing the connections in a circuit, or for isolating a circuit or equipment from a source of power. It is required to open or close circuits when negligible current is broken or made."@en;
  rdfs:subClassOf cim:Switch;
  rdfs:label "Disconnector" .

cim:Discrete a owl:Class;
  rdfs:comment "Discrete represents a discrete Measurement, i.e. a Measurement representing discrete values, e.g. a Breaker position."@en;
  rdfs:subClassOf cim:Measurement;
  rdfs:label "Discrete" .

cim:Discrete.DiscreteValues a owl:ObjectProperty, owl:InverseFunctionalProperty;
  rdfs:comment "The values connected to this measurement."@en;
  rdfs:domain cim:Discrete;
  rdfs:range cim:DiscreteValue;
  rdfs:label "DiscreteValues";
  cims:multiplicity cims:M:0..n;
  owl:inverseOf cim:DiscreteValue.Discrete .

cim:DiscreteValue a owl:Class;
  rdfs:comment "DiscreteValue represents a discrete MeasurementValue."@en;
  rdfs:subClassOf cim:MeasurementValue;
  rdfs:label "DiscreteValue" .

cim:DiscreteValue.Discrete a owl:ObjectProperty, owl:FunctionalProperty;
  rdfs:comment "Measurement to which this value is connected."@en;
  rdfs:domain cim:DiscreteValue;
  rdfs:range cim:Discrete;
  rdfs:label "Discrete";
  cims:multiplicity cims:M:1..1;
  owl:inverseOf cim:Discrete.DiscreteValues .

cim:DroopSignalFeedbackKind a owl:Class;
  rdfs:comment "Governor droop signal feedback source."@en;
  rdfs:label "DroopSignalFeedbackKind" .

cim:EarthFaultCompensator a owl:Class;
  rdfs:comment "A conducting equipment used to represent a connection to ground which is typically used to compensate earth faults.   An earth fault compensator device modelled with a single terminal implies a second terminal solidly connected to ground.  If two terminals are modelled, the ground is not assumed and normal connection rules apply."@en;
  rdfs:subClassOf cim:ConductingEquipment;
  rdfs:label "EarthFaultCompensator" .

cim:EndDevice a owl:Class;
  rdfs:comment "Asset container that performs one or more end device functions. One type of end device is a meter which can perform metering, load management, connect/disconnect, accounting functions, etc. Some end devices, such as ones monitoring and controlling air conditioners, refrigerators, pool pumps may be connected to a meter. All end devices may have communication capability defined by the associated communication function(s). An end device may be owned by a consumer, a service provider, utility or otherwise."@en;
  rdfs:subClassOf cim:AssetContainer;
  rdfs:label "EndDevice" .

cim:EnergyArea a owl:Class;
  rdfs:comment "Describes an area having energy production or consumption.  Specializations are intended to support the load allocation function as typically required in energy management systems or planning studies to allocate hypothesized load levels to individual load points for power flow analysis.  Often the energy area can be linked to both measured and forecast load levels."@en;
  rdfs:subClassOf cim:IdentifiedObject;
  rdfs:label "EnergyArea" .

cim:EnergyArea.ControlArea a owl:ObjectProperty, owl:InverseFunctionalProperty, owl:FunctionalProperty;
  rdfs:comment "The control area specification that is used for the load forecast."@en;
  rdfs:domain cim:EnergyArea;
  rdfs:range cim:ControlArea;
  rdfs:label "ControlArea";
  cims:multiplicity cims:M:0..1;
  owl:inverseOf cim:ControlArea.EnergyArea .

cim:EnergyConnection a owl:Class;
  rdfs:comment "A connection of energy generation or consumption on the power system model."@en;
  rdfs:subClassOf cim:ConductingEquipment;
  rdfs:label "EnergyConnection" .

cim:EnergyConsumer a owl:Class;
  rdfs:comment """Generic user of energy - a  point of consumption on the power system model.
EnergyConsumer.pfixed, .qfixed, .pfixedPct and .qfixedPct have meaning only if there is no LoadResponseCharacteristic associated with EnergyConsumer or if LoadResponseCharacteristic.exponentModel is set to False."""@en;
  rdfs:subClassOf cim:EnergyConnection;
  rdfs:label "EnergyConsumer" .

cim:EnergyConsumer.LoadResponse a owl:ObjectProperty, owl:FunctionalProperty;
  rdfs:comment "The load response characteristic of this load.  If missing, this load is assumed to be constant power."@en;
  rdfs:domain cim:EnergyConsumer;
  rdfs:range cim:LoadResponseCharacteristic;
  rdfs:label "LoadResponse";
  cims:multiplicity cims:M:0..1;
  owl:inverseOf cim:LoadResponseCharacteristic.EnergyConsumer .

cim:EnergyConsumer.p a owl:FunctionalProperty, owl:DatatypeProperty;
  rdfs:comment """Active power of the load. Load sign convention is used, i.e. positive sign means flow out from a node.
For voltage dependent loads the value is at rated voltage.
Starting value for a steady state solution."""@en;
  rdfs:domain cim:EnergyConsumer;
  rdfs:range xsd:float;
  rdfs:label "p";
  cims:multiplicity cims:M:1..1;
  cim:unitMultiplier cim:UnitMultiplier.M;
  cim:unitSymbol cim:UnitSymbol.W;
  qudt:hasQuantityKind cim:ActivePower;
  qudt:hasUnit unit:MegaW .

cim:EnergyConsumer.pfixed a owl:FunctionalProperty, owl:DatatypeProperty;
  rdfs:comment "Active power of the load that is a fixed quantity and does not vary as load group value varies. Load sign convention is used, i.e. positive sign means flow out from a node."@en;
  rdfs:domain cim:EnergyConsumer;
  rdfs:range xsd:float;
  rdfs:label "pfixed";
  cims:multiplicity cims:M:0..1;
  cim:unitMultiplier cim:UnitMultiplier.M;
  cim:unitSymbol cim:UnitSymbol.W;
  qudt:hasQuantityKind cim:ActivePower;
  qudt:hasUnit unit:MegaW .

cim:EnergyConsumer.pfixedPct a owl:FunctionalProperty, owl:DatatypeProperty;
  rdfs:comment "Fixed active power as a percentage of load group fixed active power. Used to represent the time-varying components.  Load sign convention is used, i.e. positive sign means flow out from a node."@en;
  rdfs:domain cim:EnergyConsumer;
  rdfs:range xsd:float;
  rdfs:label "pfixedPct";
  cims:multiplicity cims:M:0..1;
  cim:unitMultiplier cim:UnitMultiplier.none;
  cim:unitSymbol cim:UnitSymbol.none;
  qudt:hasQuantityKind cim:PerCent;
  qudt:hasUnit unit:PERCENT .

cim:EnergyConsumer.q a owl:FunctionalProperty, owl:DatatypeProperty;
  rdfs:comment """Reactive power of the load. Load sign convention is used, i.e. positive sign means flow out from a node.
For voltage dependent loads the value is at rated voltage.
Starting value for a steady state solution."""@en;
  rdfs:domain cim:EnergyConsumer;
  rdfs:range xsd:float;
  rdfs:label "q";
  cims:multiplicity cims:M:1..1;
  cim:unitMultiplier cim:UnitMultiplier.M;
  cim:unitSymbol cim:UnitSymbol.VAr;
  qudt:hasQuantityKind cim:ReactivePower;
  qudt:hasUnit unit:MegaV-A_Reactive .

cim:EnergyConsumer.qfixed a owl:FunctionalProperty, owl:DatatypeProperty;
  rdfs:comment "Reactive power of the load that is a fixed quantity and does not vary as load group value varies. Load sign convention is used, i.e. positive sign means flow out from a node."@en;
  rdfs:domain cim:EnergyConsumer;
  rdfs:range xsd:float;
  rdfs:label "qfixed";
  cims:multiplicity cims:M:0..1;
  cim:unitMultiplier cim:UnitMultiplier.M;
  cim:unitSymbol cim:UnitSymbol.VAr;
  qudt:hasQuantityKind cim:ReactivePower;
  qudt:hasUnit unit:MegaV-A_Reactive .

cim:EnergyConsumer.qfixedPct a owl:FunctionalProperty, owl:DatatypeProperty;
  rdfs:comment "Fixed reactive power as a percentage of load group fixed reactive power. Used to represent the time-varying components.  Load sign convention is used, i.e. positive sign means flow out from a node."@en;
  rdfs:domain cim:EnergyConsumer;
  rdfs:range xsd:float;
  rdfs:label "qfixedPct";
  cims:multiplicity cims:M:0..1;
  cim:unitMultiplier cim:UnitMultiplier.none;
  cim:unitSymbol cim:UnitSymbol.none;
  qudt:hasQuantityKind cim:PerCent;
  qudt:hasUnit unit:PERCENT .

cim:Equipment a owl:Class;
  rdfs:comment "The parts of a power system that are physical devices, electronic or mechanical."@en;
  rdfs:subClassOf cimr:EquipmentOrContainer;
  rdfs:label "Equipment" .

cim:Equipment.ContingencyEquipment a owl:ObjectProperty, owl:InverseFunctionalProperty;
  rdfs:comment "The contingency equipments in which this equipment participates."@en;
  rdfs:domain cim:Equipment;
  rdfs:range cim:ContingencyEquipment;
  rdfs:label "ContingencyEquipment";
  cims:multiplicity cims:M:0..n;
  owl:inverseOf cim:ContingencyEquipment.Equipment .

cim:Equipment.EquipmentContainer a owl:ObjectProperty, owl:FunctionalProperty;
  rdfs:comment "Container of this equipment."@en;
  rdfs:domain cim:Equipment;
  rdfs:range cim:EquipmentContainer;
  rdfs:label "EquipmentContainer";
  cims:multiplicity cims:M:0..1;
  owl:inverseOf cim:EquipmentContainer.Equipments .

cim:Equipment.aggregate a owl:FunctionalProperty, owl:DatatypeProperty;
  rdfs:comment "The aggregate flag provides an alternative way of representing an aggregated (equivalent) element. It is applicable in cases when the dedicated classes for equivalent equipment do not have all of the attributes necessary to represent the required level of detail.  In case the flag is set to “true” the single instance of equipment represents multiple pieces of equipment that have been modelled together as an aggregate equivalent obtained by a network reduction procedure. Examples would be power transformers"@en;
  rdfs:domain cim:Equipment;
  rdfs:range xsd:boolean;
  rdfs:label "aggregate";
  cims:multiplicity cims:M:0..1 .

cim:Equipment.inService a owl:FunctionalProperty, owl:DatatypeProperty;
  rdfs:comment "Specifies the availability of the equipment. True means the equipment is available for topology processing, which determines if the equipment is energized or not. False means that the equipment is treated by network applications as if it is not in the model."@en;
  rdfs:domain cim:Equipment;
  rdfs:range xsd:boolean;
  rdfs:label "inService";
  cims:multiplicity cims:M:1..1 .

cim:Equipment.networkAnalysisEnabled a owl:FunctionalProperty, owl:DatatypeProperty;
  rdfs:comment "The equipment is enabled to participate in network analysis.  If unspecified, the value is assumed to be true."@en;
  rdfs:domain cim:Equipment;
  rdfs:range xsd:boolean;
  rdfs:label "networkAnalysisEnabled";
  cims:multiplicity cims:M:0..1 .

cim:Equipment.normallyInService a owl:FunctionalProperty, owl:DatatypeProperty;
  rdfs:comment "Specifies the availability of the equipment under normal operating conditions. True means the equipment is available for topology processing, which determines if the equipment is energized or not. False means that the equipment is treated by network applications as if it is not in the model."@en;
  rdfs:domain cim:Equipment;
  rdfs:range xsd:boolean;
  rdfs:label "normallyInService";
  cims:multiplicity cims:M:0..1 .

cim:EquipmentContainer a owl:Class;
  rdfs:comment "A modelling construct to provide a root class for containing equipment."@en;
  rdfs:subClassOf cim:ConnectivityNodeContainer;
  rdfs:label "EquipmentContainer" .

cim:EquipmentContainer.Equipments a owl:ObjectProperty, owl:InverseFunctionalProperty;
  rdfs:comment "Contained equipment."@en;
  rdfs:subPropertyOf cimr:hasPart;
  rdfs:domain cim:EquipmentContainer;
  rdfs:range cim:Equipment;
  rdfs:label "Equipments";
  cims:multiplicity cims:M:0..n;
  owl:inverseOf cim:Equipment.EquipmentContainer .

cim:EquivalentEquipment a owl:Class;
  rdfs:comment "The class represents equivalent objects that are the result of a network reduction. The class is the base for equivalent objects of different types."@en;
  rdfs:subClassOf cim:ConductingEquipment;
  rdfs:label "EquivalentEquipment" .

cim:EquivalentInjection a owl:Class;
  rdfs:comment "This class represents equivalent injections (generation or load).  Voltage regulation is allowed only at the point of connection."@en;
  rdfs:subClassOf cim:EquivalentEquipment;
  rdfs:label "EquivalentInjection" .

cim:EquivalentInjection.maxP a owl:FunctionalProperty, owl:DatatypeProperty;
  rdfs:comment "Maximum active power of the injection."@en;
  rdfs:domain cim:EquivalentInjection;
  rdfs:range xsd:float;
  rdfs:label "maxP";
  cims:multiplicity cims:M:0..1;
  cim:unitMultiplier cim:UnitMultiplier.M;
  cim:unitSymbol cim:UnitSymbol.W;
  qudt:hasQuantityKind cim:ActivePower;
  qudt:hasUnit unit:MegaW .

cim:EquivalentInjection.maxQ a owl:FunctionalProperty, owl:DatatypeProperty;
  rdfs:comment "Maximum reactive power of the injection.  Used for modelling of infeed for load flow exchange. Not used for short circuit modelling.  If maxQ and minQ are not used ReactiveCapabilityCurve can be used."@en;
  rdfs:domain cim:EquivalentInjection;
  rdfs:range xsd:float;
  rdfs:label "maxQ";
  cims:multiplicity cims:M:0..1;
  cim:unitMultiplier cim:UnitMultiplier.M;
  cim:unitSymbol cim:UnitSymbol.VAr;
  qudt:hasQuantityKind cim:ReactivePower;
  qudt:hasUnit unit:MegaV-A_Reactive .

cim:EquivalentInjection.minP a owl:FunctionalProperty, owl:DatatypeProperty;
  rdfs:comment "Minimum active power of the injection."@en;
  rdfs:domain cim:EquivalentInjection;
  rdfs:range xsd:float;
  rdfs:label "minP";
  cims:multiplicity cims:M:0..1;
  cim:unitMultiplier cim:UnitMultiplier.M;
  cim:unitSymbol cim:UnitSymbol.W;
  qudt:hasQuantityKind cim:ActivePower;
  qudt:hasUnit unit:MegaW .

cim:EquivalentInjection.minQ a owl:FunctionalProperty, owl:DatatypeProperty;
  rdfs:comment "Minimum reactive power of the injection.  Used for modelling of infeed for load flow exchange. Not used for short circuit modelling.  If maxQ and minQ are not used ReactiveCapabilityCurve can be used."@en;
  rdfs:domain cim:EquivalentInjection;
  rdfs:range xsd:float;
  rdfs:label "minQ";
  cims:multiplicity cims:M:0..1;
  cim:unitMultiplier cim:UnitMultiplier.M;
  cim:unitSymbol cim:UnitSymbol.VAr;
  qudt:hasQuantityKind cim:ReactivePower;
  qudt:hasUnit unit:MegaV-A_Reactive .

cim:EquivalentInjection.p a owl:FunctionalProperty, owl:DatatypeProperty;
  rdfs:comment """Equivalent active power injection. Load sign convention is used, i.e. positive sign means flow out from a node.
Starting value for steady state solutions."""@en;
  rdfs:domain cim:EquivalentInjection;
  rdfs:range xsd:float;
  rdfs:label "p";
  cims:multiplicity cims:M:1..1;
  cim:unitMultiplier cim:UnitMultiplier.M;
  cim:unitSymbol cim:UnitSymbol.W;
  qudt:hasQuantityKind cim:ActivePower;
  qudt:hasUnit unit:MegaW .

cim:EquivalentInjection.q a owl:FunctionalProperty, owl:DatatypeProperty;
  rdfs:comment """Equivalent reactive power injection. Load sign convention is used, i.e. positive sign means flow out from a node.
Starting value for steady state solutions."""@en;
  rdfs:domain cim:EquivalentInjection;
  rdfs:range xsd:float;
  rdfs:label "q";
  cims:multiplicity cims:M:1..1;
  cim:unitMultiplier cim:UnitMultiplier.M;
  cim:unitSymbol cim:UnitSymbol.VAr;
  qudt:hasQuantityKind cim:ReactivePower;
  qudt:hasUnit unit:MegaV-A_Reactive .

cim:EquivalentInjection.r a owl:FunctionalProperty, owl:DatatypeProperty;
  rdfs:comment """Positive sequence resistance. Used to represent Extended-Ward (IEC 60909).
Usage : Extended-Ward is a result of network reduction prior to the data exchange."""@en;
  rdfs:domain cim:EquivalentInjection;
  rdfs:range xsd:float;
  rdfs:label "r";
  cims:multiplicity cims:M:1..1;
  cim:unitMultiplier cim:UnitMultiplier.none;
  cim:unitSymbol cim:UnitSymbol.ohm;
  qudt:hasQuantityKind cim:Resistance;
  qudt:hasUnit unit:OHM .

cim:EquivalentInjection.r0 a owl:FunctionalProperty, owl:DatatypeProperty;
  rdfs:comment """Zero sequence resistance. Used to represent Extended-Ward (IEC 60909).
Usage : Extended-Ward is a result of network reduction prior to the data exchange."""@en;
  rdfs:domain cim:EquivalentInjection;
  rdfs:range xsd:float;
  rdfs:label "r0";
  cims:multiplicity cims:M:1..1;
  cim:unitMultiplier cim:UnitMultiplier.none;
  cim:unitSymbol cim:UnitSymbol.ohm;
  qudt:hasQuantityKind cim:Resistance;
  qudt:hasUnit unit:OHM .

cim:EquivalentInjection.regulationCapability a owl:FunctionalProperty, owl:DatatypeProperty;
  rdfs:comment "Specifies whether or not the EquivalentInjection has the capability to regulate the local voltage. If true the EquivalentInjection can regulate. If false the EquivalentInjection cannot regulate. ReactiveCapabilityCurve can only be associated with EquivalentInjection  if the flag is true."@en;
  rdfs:domain cim:EquivalentInjection;
  rdfs:range xsd:boolean;
  rdfs:label "regulationCapability";
  cims:multiplicity cims:M:1..1 .

cim:EquivalentInjection.x a owl:FunctionalProperty, owl:DatatypeProperty;
  rdfs:comment """Positive sequence reactance. Used to represent Extended-Ward (IEC 60909).
Usage : Extended-Ward is a result of network reduction prior to the data exchange."""@en;
  rdfs:domain cim:EquivalentInjection;
  rdfs:range xsd:float;
  rdfs:label "x";
  cims:multiplicity cims:M:1..1;
  cim:unitMultiplier cim:UnitMultiplier.none;
  cim:unitSymbol cim:UnitSymbol.ohm;
  qudt:hasQuantityKind cim:Reactance;
  qudt:hasUnit unit:OHM .

cim:EquivalentInjection.x0 a owl:FunctionalProperty, owl:DatatypeProperty;
  rdfs:comment """Zero sequence reactance. Used to represent Extended-Ward (IEC 60909).
Usage : Extended-Ward is a result of network reduction prior to the data exchange."""@en;
  rdfs:domain cim:EquivalentInjection;
  rdfs:range xsd:float;
  rdfs:label "x0";
  cims:multiplicity cims:M:1..1;
  cim:unitMultiplier cim:UnitMultiplier.none;
  cim:unitSymbol cim:UnitSymbol.ohm;
  qudt:hasQuantityKind cim:Reactance;
  qudt:hasUnit unit:OHM .

cim:ExcIEEEST1AUELselectorKind a owl:Class;
  rdfs:comment "Types of connections for the UEL input used in ExcIEEEST1A."@en;
  rdfs:label "ExcIEEEST1AUELselectorKind" .

cim:ExcREXSFeedbackSignalKind a owl:Class;
  rdfs:comment "Types of rate feedback signals."@en;
  rdfs:label "ExcREXSFeedbackSignalKind" .

cim:ExcST6BOELselectorKind a owl:Class;
  rdfs:comment "Types of connections for the OEL input used for static excitation systems type 6B."@en;
  rdfs:label "ExcST6BOELselectorKind" .

cim:ExcST7BOELselectorKind a owl:Class;
  rdfs:comment "Types of connections for the OEL input used for static excitation systems type 7B."@en;
  rdfs:label "ExcST7BOELselectorKind" .

cim:ExcST7BUELselectorKind a owl:Class;
  rdfs:comment "Types of connections for the UEL input used for static excitation systems type 7B."@en;
  rdfs:label "ExcST7BUELselectorKind" .

cim:Feeder a owl:Class;
  rdfs:comment """A collection of equipment for organizational purposes, used for grouping distribution resources.
The organization a feeder does not necessarily reflect connectivity or current operation state."""@en;
  rdfs:subClassOf cim:EquipmentContainer;
  rdfs:label "Feeder" .

cim:FrancisGovernorControlKind a owl:Class;
  rdfs:comment "Governor control flag for Francis hydro model."@en;
  rdfs:label "FrancisGovernorControlKind" .

cim:FuelType a owl:Class;
  rdfs:comment "Type of fuel."@en;
  rdfs:label "FuelType" .

cim:Fuse a owl:Class;
  rdfs:comment "An overcurrent protective device with a circuit opening fusible part that is heated and severed by the passage of overcurrent through it. A fuse is considered a switching device because it breaks current."@en;
  rdfs:subClassOf cim:Switch;
  rdfs:label "Fuse" .

cim:GeneratingUnit a owl:Class;
  rdfs:comment "A single or set of synchronous machines for converting mechanical power into alternating-current power. For example, individual machines within a set may be defined for scheduling purposes while a single control signal is derived for the set. In this case there would be a GeneratingUnit for each member of the set and an additional GeneratingUnit corresponding to the set."@en;
  rdfs:subClassOf cim:Equipment;
  rdfs:label "GeneratingUnit" .

cim:GeneratingUnit.ControlAreaGeneratingUnit a owl:ObjectProperty, owl:InverseFunctionalProperty;
  rdfs:comment "ControlArea specifications for this generating unit."@en;
  rdfs:domain cim:GeneratingUnit;
  rdfs:range cim:ControlAreaGeneratingUnit;
  rdfs:label "ControlAreaGeneratingUnit";
  cims:multiplicity cims:M:0..n;
  owl:inverseOf cim:ControlAreaGeneratingUnit.GeneratingUnit .

cim:GeneratingUnit.RotatingMachine a owl:ObjectProperty, owl:InverseFunctionalProperty;
  rdfs:comment "A synchronous machine may operate as a generator and as such becomes a member of a generating unit."@en;
  rdfs:domain cim:GeneratingUnit;
  rdfs:range cim:RotatingMachine;
  rdfs:label "RotatingMachine";
  cims:multiplicity cims:M:1..n;
  owl:inverseOf cim:RotatingMachine.GeneratingUnit .

cim:GeneratingUnit.maxEconomicP a owl:FunctionalProperty, owl:DatatypeProperty;
  rdfs:comment "Maximum high economic active power limit, that should not exceed the maximum operating active power limit."@en;
  rdfs:domain cim:GeneratingUnit;
  rdfs:range xsd:float;
  rdfs:label "maxEconomicP";
  cims:multiplicity cims:M:0..1;
  cim:unitMultiplier cim:UnitMultiplier.M;
  cim:unitSymbol cim:UnitSymbol.W;
  qudt:hasQuantityKind cim:ActivePower;
  qudt:hasUnit unit:MegaW .

cim:GeneratingUnit.maxOperatingP a owl:FunctionalProperty, owl:DatatypeProperty;
  rdfs:comment "This is the maximum operating active power limit the dispatcher can enter for this unit."@en;
  rdfs:domain cim:GeneratingUnit;
  rdfs:range xsd:float;
  rdfs:label "maxOperatingP";
  cims:multiplicity cims:M:1..1;
  cim:unitMultiplier cim:UnitMultiplier.M;
  cim:unitSymbol cim:UnitSymbol.W;
  qudt:hasQuantityKind cim:ActivePower;
  qudt:hasUnit unit:MegaW .

cim:GeneratingUnit.minEconomicP a owl:FunctionalProperty, owl:DatatypeProperty;
  rdfs:comment "Low economic active power limit that shall be greater than or equal to the minimum operating active power limit."@en;
  rdfs:domain cim:GeneratingUnit;
  rdfs:range xsd:float;
  rdfs:label "minEconomicP";
  cims:multiplicity cims:M:0..1;
  cim:unitMultiplier cim:UnitMultiplier.M;
  cim:unitSymbol cim:UnitSymbol.W;
  qudt:hasQuantityKind cim:ActivePower;
  qudt:hasUnit unit:MegaW .

cim:GeneratingUnit.minOperatingP a owl:FunctionalProperty, owl:DatatypeProperty;
  rdfs:comment "This is the minimum operating active power limit the dispatcher can enter for this unit."@en;
  rdfs:domain cim:GeneratingUnit;
  rdfs:range xsd:float;
  rdfs:label "minOperatingP";
  cims:multiplicity cims:M:1..1;
  cim:unitMultiplier cim:UnitMultiplier.M;
  cim:unitSymbol cim:UnitSymbol.W;
  qudt:hasQuantityKind cim:ActivePower;
  qudt:hasUnit unit:MegaW .

cim:GeneratingUnit.nominalP a owl:FunctionalProperty, owl:DatatypeProperty;
  rdfs:comment """The nominal power of the generating unit.  Used to give precise meaning to percentage based attributes such as the governor speed change droop (governorSCD attribute).
The attribute shall be a positive value equal to or less than RotatingMachine.ratedS."""@en;
  rdfs:domain cim:GeneratingUnit;
  rdfs:range xsd:float;
  rdfs:label "nominalP";
  cims:multiplicity cims:M:0..1;
  cim:unitMultiplier cim:UnitMultiplier.M;
  cim:unitSymbol cim:UnitSymbol.W;
  qudt:hasQuantityKind cim:ActivePower;
  qudt:hasUnit unit:MegaW .

cim:GeneratingUnit.normalPF a owl:FunctionalProperty, owl:DatatypeProperty;
  rdfs:comment "Generating unit economic participation factor.  The sum of the participation factors across generating units does not have to sum to one.  It is used for representing distributed slack participation factor. The attribute shall be a positive value or zero."@en;
  rdfs:domain cim:GeneratingUnit;
  rdfs:range xsd:float;
  rdfs:label "normalPF";
  cims:multiplicity cims:M:1..1 .

cim:GeneratingUnit.ratedGrossMaxP a owl:FunctionalProperty, owl:DatatypeProperty;
  rdfs:comment """The unit's gross rated maximum capacity (book value).
The attribute shall be a positive value."""@en;
  rdfs:domain cim:GeneratingUnit;
  rdfs:range xsd:float;
  rdfs:label "ratedGrossMaxP";
  cims:multiplicity cims:M:0..1;
  cim:unitMultiplier cim:UnitMultiplier.M;
  cim:unitSymbol cim:UnitSymbol.W;
  qudt:hasQuantityKind cim:ActivePower;
  qudt:hasUnit unit:MegaW .

cim:GeneratingUnit.ratedNetMaxP a owl:FunctionalProperty, owl:DatatypeProperty;
  rdfs:comment """The net rated maximum capacity determined by subtracting the auxiliary power used to operate the internal plant machinery from the rated gross maximum capacity.
The attribute shall be a positive value."""@en;
  rdfs:domain cim:GeneratingUnit;
  rdfs:range xsd:float;
  rdfs:label "ratedNetMaxP";
  cims:multiplicity cims:M:0..1;
  cim:unitMultiplier cim:UnitMultiplier.M;
  cim:unitSymbol cim:UnitSymbol.W;
  qudt:hasQuantityKind cim:ActivePower;
  qudt:hasUnit unit:MegaW .

cim:GeneratorControlSource a owl:Class;
  rdfs:comment "The source of controls for a generating unit."@en;
  rdfs:label "GeneratorControlSource" .

cim:GenericNonLinearLoadModelKind a owl:Class;
  rdfs:comment "Type of generic non-linear load model."@en;
  rdfs:label "GenericNonLinearLoadModelKind" .

cim:GeographicalRegion a owl:Class;
  rdfs:comment "A geographical region of a power system network model."@en;
  rdfs:subClassOf cim:IdentifiedObject;
  rdfs:label "GeographicalRegion" .

cim:GeographicalRegion.Regions a owl:ObjectProperty, owl:InverseFunctionalProperty;
  rdfs:comment "All sub-geographical regions within this geographical region."@en;
  rdfs:domain cim:GeographicalRegion;
  rdfs:range cim:SubGeographicalRegion;
  rdfs:label "Regions";
  cims:multiplicity cims:M:0..n;
  owl:inverseOf cim:SubGeographicalRegion.Region .

cim:GovHydro4ModelKind a owl:Class;
  rdfs:comment "Possible types of GovHydro4 models."@en;
  rdfs:label "GovHydro4ModelKind" .

cim:HydroEnergyConversionKind a owl:Class;
  rdfs:comment "Specifies the capability of the hydro generating unit to convert energy as a generator or pump."@en;
  rdfs:label "HydroEnergyConversionKind" .

cim:HydroPlantStorageKind a owl:Class;
  rdfs:comment "The type of hydro power plant."@en;
  rdfs:label "HydroPlantStorageKind" .

cim:HydroTurbineKind a owl:Class;
  rdfs:comment "Type of turbine."@en;
  rdfs:label "HydroTurbineKind" .

cim:IOPoint a owl:Class;
  rdfs:comment "The class describe a measurement or control value. The purpose is to enable having attributes and associations common for measurement and control."@en;
  rdfs:subClassOf cim:IdentifiedObject;
  rdfs:label "IOPoint" .

cim:IdentifiedObject a owl:Class;
  rdfs:comment "This is a root class to provide common identification for all classes needing identification and naming attributes."@en;
  rdfs:label "IdentifiedObject" .

cim:IdentifiedObject.DiagramObjects a owl:ObjectProperty, owl:InverseFunctionalProperty;
  rdfs:comment "The diagram objects that are associated with the domain object."@en;
  rdfs:domain cim:IdentifiedObject;
  rdfs:range cim:DiagramObject;
  rdfs:label "DiagramObjects";
  cims:multiplicity cims:M:0..n;
  owl:inverseOf cim:DiagramObject.IdentifiedObject .

cim:IdentifiedObject.aliasName a owl:FunctionalProperty, owl:DatatypeProperty;
  rdfs:comment """The aliasName is free text human readable name of the object alternative to IdentifiedObject.name. It may be non unique and may not correlate to a naming hierarchy.
The attribute aliasName is retained because of backwards compatibility between CIM relases. It is however recommended to replace aliasName with the Name class as aliasName is planned for retirement at a future time."""@en;
  rdfs:domain cim:IdentifiedObject;
  rdfs:range xsd:string;
  rdfs:label "aliasName";
  cims:multiplicity cims:M:0..1 .

cim:IdentifiedObject.description a owl:ObjectProperty, owl:FunctionalProperty, owl:DatatypeProperty;
  rdfs:comment "The description is a free human readable text describing or naming the object. It may be non unique and may not correlate to a naming hierarchy."@en;
  rdfs:domain cim:IdentifiedObject;
  rdfs:range xsd:string;
  rdfs:label "description";
  cims:multiplicity cims:M:0..1;
  cims:dataType cim:String .

cim:IdentifiedObject.mRID a owl:ObjectProperty, owl:FunctionalProperty, owl:DatatypeProperty;
  rdfs:comment """Master resource identifier issued by a model authority. The mRID is unique within an exchange context. Global uniqueness is easily achieved by using a UUID, as specified in RFC 4122, for the mRID. The use of UUID is strongly recommended.
For CIMXML data files in RDF syntax conforming to IEC 61970-552, the mRID is mapped to rdf:ID or rdf:about attributes that identify CIM object elements."""@en;
  rdfs:domain cim:IdentifiedObject;
  rdfs:range xsd:string;
  rdfs:label "mRID";
  cims:multiplicity cims:M:0..1, cims:M:1..1;
  cims:dataType cim:String .

cim:IdentifiedObject.name a owl:ObjectProperty, owl:FunctionalProperty, owl:DatatypeProperty;
  rdfs:comment "The name is any free human readable and possibly non unique text naming the object."@en;
  rdfs:domain cim:IdentifiedObject;
  rdfs:range xsd:string;
  rdfs:label "name";
  cims:multiplicity cims:M:0..1, cims:M:1..1;
  cims:dataType cim:String .

cim:IfdBaseKind a owl:Class;
  rdfs:comment "Excitation base system mode."@en;
  rdfs:label "IfdBaseKind" .

cim:InUseStateKind a owl:Class;
  rdfs:comment "Possible 'in use' states that an asset can be in."@en;
  rdfs:label "InUseStateKind" .

cim:InUseStateKind.inUse a cim:InUseStateKind;
  rdfs:comment "Asset is deployed (in use) or is being put into use."@en;
  rdfs:label "inUse" .

cim:InputSignalKind a owl:Class;
  rdfs:comment "Types of input signals.  In dynamics modelling, commonly represented by the <i>j</i> parameter."@en;
  rdfs:label "InputSignalKind" .

cim:Line a owl:Class;
  rdfs:comment "Contains equipment beyond a substation belonging to a power transmission line."@en;
  rdfs:subClassOf cim:EquipmentContainer;
  rdfs:label "Line";
  cims:pragmatics "This means only AC Line (not DC)" .

cim:Line.Region a owl:ObjectProperty, owl:FunctionalProperty;
  rdfs:comment "The sub-geographical region of the line."@en;
  rdfs:domain cim:Line;
  rdfs:range cim:SubGeographicalRegion;
  rdfs:label "Region";
  cims:multiplicity cims:M:0..1;
  owl:inverseOf cim:SubGeographicalRegion.Lines .

cim:LinearShuntCompensator a owl:Class;
  rdfs:comment "A linear shunt compensator has banks or sections with equal admittance values."@en;
  rdfs:subClassOf cim:ShuntCompensator;
  rdfs:label "LinearShuntCompensator" .

cim:LinearShuntCompensator.bPerSection a owl:FunctionalProperty, owl:DatatypeProperty;
  rdfs:comment "Positive sequence shunt (charging) susceptance per section."@en;
  rdfs:domain cim:LinearShuntCompensator;
  rdfs:range xsd:float;
  rdfs:label "bPerSection";
  cims:multiplicity cims:M:1..1;
  cim:unitMultiplier cim:UnitMultiplier.none;
  cim:unitSymbol cim:UnitSymbol.S;
  qudt:hasQuantityKind cim:Susceptance;
  qudt:hasUnit unit:S .

cim:LinearShuntCompensator.gPerSection a owl:FunctionalProperty, owl:DatatypeProperty;
  rdfs:comment "Positive sequence shunt (charging) conductance per section."@en;
  rdfs:domain cim:LinearShuntCompensator;
  rdfs:range xsd:float;
  rdfs:label "gPerSection";
  cims:multiplicity cims:M:1..1;
  cim:unitMultiplier cim:UnitMultiplier.none;
  cim:unitSymbol cim:UnitSymbol.S;
  qudt:hasQuantityKind cim:Conductance;
  qudt:hasUnit unit:S .

cim:LoadArea a owl:Class;
  rdfs:comment "The class is the root or first level in a hierarchical structure for grouping of loads for the purpose of load flow load scaling."@en;
  rdfs:subClassOf cim:EnergyArea;
  rdfs:label "LoadArea" .

cim:LoadArea.SubLoadAreas a owl:ObjectProperty, owl:InverseFunctionalProperty;
  rdfs:comment "The SubLoadAreas in the LoadArea."@en;
  rdfs:domain cim:LoadArea;
  rdfs:range cim:SubLoadArea;
  rdfs:label "SubLoadAreas";
  cims:multiplicity cims:M:1..n;
  owl:inverseOf cim:SubLoadArea.LoadArea .

cim:LoadBreakSwitch a owl:Class;
  rdfs:comment "A mechanical switching device capable of making, carrying, and breaking currents under normal operating conditions."@en;
  rdfs:subClassOf cim:ProtectedSwitch;
  rdfs:label "LoadBreakSwitch" .

cim:LoadGroup a owl:Class;
  rdfs:comment "The class is the third level in a hierarchical structure for grouping of loads for the purpose of load flow load scaling."@en;
  rdfs:subClassOf cim:IdentifiedObject;
  rdfs:label "LoadGroup" .

cim:LoadGroup.SubLoadArea a owl:ObjectProperty, owl:FunctionalProperty;
  rdfs:comment "The SubLoadArea where the Loadgroup belongs."@en;
  rdfs:domain cim:LoadGroup;
  rdfs:range cim:SubLoadArea;
  rdfs:label "SubLoadArea";
  cims:multiplicity cims:M:1..1;
  owl:inverseOf cim:SubLoadArea.LoadGroups .

cim:LoadResponseCharacteristic a owl:Class;
  rdfs:comment "Models the characteristic response of the load demand due to changes in system conditions such as voltage and frequency. It is not related to demand response. If LoadResponseCharacteristic.exponentModel is True, the exponential voltage or frequency dependent models are specified and used as to calculate active and reactive power components of the load model. The equations to calculate active and reactive power components of the load model are internal to the power flow calculation, hence they use"@en;
  rdfs:subClassOf cim:IdentifiedObject;
  rdfs:label "LoadResponseCharacteristic" .

cim:LoadResponseCharacteristic.EnergyConsumer a owl:ObjectProperty, owl:InverseFunctionalProperty;
  rdfs:comment "The set of loads that have the response characteristics."@en;
  rdfs:domain cim:LoadResponseCharacteristic;
  rdfs:range cim:EnergyConsumer;
  rdfs:label "EnergyConsumer";
  cims:multiplicity cims:M:0..n;
  owl:inverseOf cim:EnergyConsumer.LoadResponse .

cim:LoadResponseCharacteristic.exponentModel a owl:FunctionalProperty, owl:DatatypeProperty;
  rdfs:comment "Indicates the exponential voltage dependency model is to be used. If false, the coefficient model is to be used. The exponential voltage dependency model consist of the attributes: - pVoltageExponent - qVoltageExponent - pFrequencyExponent - qFrequencyExponent. The coefficient model consist of the attributes: - pConstantImpedance - pConstantCurrent - pConstantPower - qConstantImpedance - qConstantCurrent - qConstantPower. The sum of pConstantImpedance, pConstantCurrent and pConstantPower shall equal"@en;
  rdfs:domain cim:LoadResponseCharacteristic;
  rdfs:range xsd:boolean;
  rdfs:label "exponentModel";
  cims:multiplicity cims:M:1..1 .

cim:LoadResponseCharacteristic.pConstantCurrent a owl:FunctionalProperty, owl:DatatypeProperty;
  rdfs:comment "Portion of active power load modelled as constant current."@en;
  rdfs:domain cim:LoadResponseCharacteristic;
  rdfs:range xsd:float;
  rdfs:label "pConstantCurrent";
  cims:multiplicity cims:M:0..1 .

cim:LoadResponseCharacteristic.pConstantImpedance a owl:FunctionalProperty, owl:DatatypeProperty;
  rdfs:comment "Portion of active power load modelled as constant impedance."@en;
  rdfs:domain cim:LoadResponseCharacteristic;
  rdfs:range xsd:float;
  rdfs:label "pConstantImpedance";
  cims:multiplicity cims:M:0..1 .

cim:LoadResponseCharacteristic.pConstantPower a owl:FunctionalProperty, owl:DatatypeProperty;
  rdfs:comment "Portion of active power load modelled as constant power."@en;
  rdfs:domain cim:LoadResponseCharacteristic;
  rdfs:range xsd:float;
  rdfs:label "pConstantPower";
  cims:multiplicity cims:M:0..1 .

cim:LoadResponseCharacteristic.qConstantCurrent a owl:FunctionalProperty, owl:DatatypeProperty;
  rdfs:comment "Portion of reactive power load modelled as constant current."@en;
  rdfs:domain cim:LoadResponseCharacteristic;
  rdfs:range xsd:float;
  rdfs:label "qConstantCurrent";
  cims:multiplicity cims:M:0..1 .

cim:LoadResponseCharacteristic.qConstantImpedance a owl:FunctionalProperty, owl:DatatypeProperty;
  rdfs:comment "Portion of reactive power load modelled as constant impedance."@en;
  rdfs:domain cim:LoadResponseCharacteristic;
  rdfs:range xsd:float;
  rdfs:label "qConstantImpedance";
  cims:multiplicity cims:M:0..1 .

cim:LoadResponseCharacteristic.qConstantPower a owl:FunctionalProperty, owl:DatatypeProperty;
  rdfs:comment "Portion of reactive power load modelled as constant power."@en;
  rdfs:domain cim:LoadResponseCharacteristic;
  rdfs:range xsd:float;
  rdfs:label "qConstantPower";
  cims:multiplicity cims:M:0..1 .

cim:Location a owl:Class;
  rdfs:comment "The place, scene, or point of something where someone or something has been, is, and/or will be at a given moment in time. It can be defined with one or more position points (coordinates) in a given coordinate system."@en;
  rdfs:subClassOf cim:IdentifiedObject;
  rdfs:label "Location" .

cim:Location.CoordinateSystem a owl:ObjectProperty, owl:FunctionalProperty;
  rdfs:comment "Coordinate system used to describe position points of this location."@en;
  rdfs:domain cim:Location;
  rdfs:range cim:CoordinateSystem;
  rdfs:label "CoordinateSystem";
  cims:multiplicity cims:M:1..1;
  owl:inverseOf cim:CoordinateSystem.Locations .

cim:Location.PowerSystemResources a owl:ObjectProperty, owl:InverseFunctionalProperty,
    owl:FunctionalProperty;
  rdfs:comment "All power system resources at this location."@en;
  rdfs:domain cim:Location;
  rdfs:range cim:PowerSystemResource;
  rdfs:label "PowerSystemResources";
  cims:multiplicity cims:M:1..1;
  owl:inverseOf cim:PowerSystemResource.Location .

cim:Manufacturer a owl:Class;
  rdfs:comment "Organisation that manufactures asset products."@en;
  rdfs:subClassOf cim:OrganisationRole;
  rdfs:label "Manufacturer" .

cim:Manufacturer.ProductAssetModels a owl:ObjectProperty, owl:InverseFunctionalProperty;
  rdfs:comment "All asset models by this manufacturer."@en;
  rdfs:domain cim:Manufacturer;
  rdfs:range cim:ProductAssetModel;
  rdfs:label "ProductAssetModels";
  cims:multiplicity cims:M:0..n;
  owl:inverseOf cim:ProductAssetModel.Manufacturer .

cim:Measurement a owl:Class;
  rdfs:comment "A Measurement represents any measured, calculated or non-measured non-calculated quantity. Any piece of equipment may contain Measurements, e.g. a substation may have temperature measurements and door open indications, a transformer may have oil temperature and tank pressure measurements, a bay may contain a number of power flow measurements and a Breaker may contain a switch status measurement.  The PSR - Measurement association is intended to capture this use of Measurement and is included in the"@en;
  rdfs:subClassOf cim:IdentifiedObject;
  rdfs:label "Measurement" .

cim:Measurement.PowerSystemResource a owl:ObjectProperty, owl:FunctionalProperty;
  rdfs:comment "The power system resource that contains the measurement."@en;
  rdfs:domain cim:Measurement;
  rdfs:range cim:PowerSystemResource;
  rdfs:label "PowerSystemResource";
  cims:multiplicity cims:M:1..1;
  owl:inverseOf cim:PowerSystemResource.Measurements .

cim:Measurement.measurementType a owl:FunctionalProperty, owl:DatatypeProperty;
  rdfs:comment """Specifies the type of measurement.  For example, this specifies if the measurement represents an indoor temperature, outdoor temperature, bus voltage, line flow, etc.
When the measurementType is set to \"Specialization\", the type of Measurement is defined in more detail by the specialized class which inherits from Measurement."""@en;
  rdfs:domain cim:Measurement;
  rdfs:range xsd:string;
  rdfs:label "measurementType";
  cims:multiplicity cims:M:1..1;
  skos:example "CurrencyExchange-Actual", "Price-Actual", "ThreePhaseActivePower", "ThreePhaseActivePower-Flow-Estimated";
  cims:pragmatics "Possible values: CurrencyExchange-Actual, Price-Actual, ThreePhaseActivePower, ThreePhaseActivePower-Flow-Estimated" .

cim:Measurement.phases a owl:ObjectProperty, owl:FunctionalProperty;
  rdfs:comment """Indicates to which phases the measurement applies and avoids the need to use 'measurementType' to also encode phase information (which would explode the types). The phase information in Measurement, along with 'measurementType' and 'phases' uniquely defines a Measurement for a device, based on normal network phase. Their meaning will not change when the computed energizing phasing is changed due to jumpers or other reasons.
If the attribute is missing three phases (ABC) shall be assumed."""@en;
  rdfs:domain cim:Measurement;
  rdfs:range cim:PhaseCode;
  rdfs:label "phases";
  cims:multiplicity cims:M:0..1 .

cim:Measurement.unitMultiplier a owl:ObjectProperty, owl:FunctionalProperty;
  rdfs:comment "The unit multiplier of the measured quantity."@en;
  rdfs:domain cim:Measurement;
  rdfs:range cim:UnitMultiplier;
  rdfs:label "unitMultiplier";
  cims:multiplicity cims:M:1..1 .

cim:Measurement.unitSymbol a owl:ObjectProperty, owl:FunctionalProperty;
  rdfs:comment "The unit of measure of the measured quantity."@en;
  rdfs:domain cim:Measurement;
  rdfs:range cim:UnitSymbol;
  rdfs:label "unitSymbol";
  cims:multiplicity cims:M:1..1 .

cim:MeasurementValue a owl:Class;
  rdfs:comment "The current state for a measurement. A state value is an instance of a measurement from a specific source. Measurements can be associated with many state values, each representing a different source for the measurement."@en;
  rdfs:subClassOf cim:IOPoint;
  rdfs:label "MeasurementValue" .

cim:MeasurementValue.MeasurementValueSource a owl:ObjectProperty, owl:FunctionalProperty;
  rdfs:comment "A reference to the type of source that updates the MeasurementValue, e.g. SCADA, CCLink, manual, etc. User conventions for the names of sources are contained in the introduction to IEC 61970-301."@en;
  rdfs:domain cim:MeasurementValue;
  rdfs:range cim:MeasurementValueSource;
  rdfs:label "MeasurementValueSource";
  cims:multiplicity cims:M:1..1;
  owl:inverseOf cim:MeasurementValueSource.MeasurementValues .

cim:MeasurementValue.sensorAccuracy a owl:FunctionalProperty, owl:DatatypeProperty;
  rdfs:comment "The limit, expressed as a percentage of the sensor maximum, that errors will not exceed when the sensor is used under  reference conditions."@en;
  rdfs:domain cim:MeasurementValue;
  rdfs:range xsd:float;
  rdfs:label "sensorAccuracy";
  cims:multiplicity cims:M:0..1;
  cim:unitMultiplier cim:UnitMultiplier.none;
  cim:unitSymbol cim:UnitSymbol.none;
  qudt:hasQuantityKind cim:PerCent;
  qudt:hasUnit unit:PERCENT .

cim:MeasurementValue.timeStamp a owl:FunctionalProperty, owl:DatatypeProperty;
  rdfs:comment "The time when the value was last updated."@en;
  rdfs:domain cim:MeasurementValue;
  rdfs:range xsd:dateTime;
  rdfs:label "timeStamp";
  cims:multiplicity cims:M:0..1 .

cim:MeasurementValueSource a owl:Class;
  rdfs:comment "MeasurementValueSource describes the alternative sources updating a MeasurementValue. User conventions for how to use the MeasurementValueSource attributes are defined in IEC 61970-301."@en;
  rdfs:subClassOf cim:IdentifiedObject;
  rdfs:label "MeasurementValueSource" .

cim:MeasurementValueSource.MeasurementValues a owl:ObjectProperty, owl:InverseFunctionalProperty;
  rdfs:comment "The MeasurementValues updated by the source."@en;
  rdfs:domain cim:MeasurementValueSource;
  rdfs:range cim:MeasurementValue;
  rdfs:label "MeasurementValues";
  cims:multiplicity cims:M:0..n;
  owl:inverseOf cim:MeasurementValue.MeasurementValueSource .

cim:Meter a owl:Class;
  rdfs:comment "Physical asset that performs the metering role of the usage point. Used for measuring consumption and detection of events."@en;
  rdfs:subClassOf cim:EndDevice;
  rdfs:label "Meter" .

cim:Name a owl:Class;
  rdfs:comment "The Name class provides the means to define any number of human readable  names for an object. A name is <b>not</b> to be used for defining inter-object relationships. For inter-object relationships instead use the object identification 'mRID'."@en;
  rdfs:label "Name" .

cim:Name.name a owl:FunctionalProperty, owl:DatatypeProperty;
  rdfs:comment "Any free text that used as a name or alternative identifier of the object."@en;
  rdfs:domain cim:Name;
  rdfs:range xsd:string;
  rdfs:label "name";
  cims:multiplicity cims:M:1..1 .

cim:NameType a owl:Class;
  rdfs:comment "Type of name. Possible values for attribute 'name' are implementation dependent but standard profiles may specify types. An enterprise may have multiple IT systems each having its own local name for the same object, e.g. a planning system may have different names from an EMS. An object may also have different names within the same IT system, e.g. localName as defined in CIM version 14. The definition from CIM14 is: The localName is a human readable name of the object. It is a free text name local"@en;
  rdfs:label "NameType" .

cim:NameType.description a owl:FunctionalProperty, owl:DatatypeProperty;
  rdfs:comment "Description of the name type."@en;
  rdfs:domain cim:NameType;
  rdfs:range xsd:string;
  rdfs:label "description";
  cims:multiplicity cims:M:0..1 .

cim:NameType.name a owl:FunctionalProperty, owl:DatatypeProperty;
  rdfs:comment "Name of the name type."@en;
  rdfs:domain cim:NameType;
  rdfs:range xsd:string;
  rdfs:label "name";
  cims:multiplicity cims:M:1..1 .

cim:NonConformLoad a owl:Class;
  rdfs:comment "NonConformLoad represents loads that do not follow a daily load change pattern and whose changes are not correlated with the daily load change pattern."@en;
  rdfs:subClassOf cim:EnergyConsumer;
  rdfs:label "NonConformLoad" .

cim:NonConformLoad.LoadGroup a owl:ObjectProperty, owl:FunctionalProperty;
  rdfs:comment "Group of this ConformLoad."@en;
  rdfs:domain cim:NonConformLoad;
  rdfs:range cim:NonConformLoadGroup;
  rdfs:label "LoadGroup";
  cims:multiplicity cims:M:1..1;
  owl:inverseOf cim:NonConformLoadGroup.EnergyConsumers .

cim:NonConformLoadGroup a owl:Class;
  rdfs:comment "Loads that do not follow a daily and seasonal load variation pattern."@en;
  rdfs:subClassOf cim:LoadGroup;
  rdfs:label "NonConformLoadGroup" .

cim:NonConformLoadGroup.EnergyConsumers a owl:ObjectProperty, owl:InverseFunctionalProperty;
  rdfs:comment "Conform loads assigned to this ConformLoadGroup."@en;
  rdfs:domain cim:NonConformLoadGroup;
  rdfs:range cim:NonConformLoad;
  rdfs:label "EnergyConsumers";
  cims:multiplicity cims:M:1..n;
  owl:inverseOf cim:NonConformLoad.LoadGroup .

cim:OperationalLimit a owl:Class;
  rdfs:comment "A value and normal value associated with a specific kind of limit.  The sub class value and normalValue attributes vary inversely to the associated OperationalLimitType.acceptableDuration (acceptableDuration for short).   If a particular piece of equipment has multiple operational limits of the same kind (apparent power, current, etc.), the limit with the greatest acceptableDuration shall have the smallest limit value and the limit with the smallest acceptableDuration shall have the largest limit"@en;
  rdfs:subClassOf cim:IdentifiedObject;
  rdfs:label "OperationalLimit" .

cim:OperationalLimit.OperationalLimitSet a owl:ObjectProperty, owl:FunctionalProperty;
  rdfs:comment "The limit set to which the limit values belong."@en;
  rdfs:domain cim:OperationalLimit;
  rdfs:range cim:OperationalLimitSet;
  rdfs:label "OperationalLimitSet";
  cims:multiplicity cims:M:1..1;
  owl:inverseOf cim:OperationalLimitSet.OperationalLimitValue .

cim:OperationalLimit.OperationalLimitType a owl:ObjectProperty, owl:FunctionalProperty;
  rdfs:comment "The limit type associated with this limit."@en;
  rdfs:domain cim:OperationalLimit;
  rdfs:range cim:OperationalLimitType;
  rdfs:label "OperationalLimitType";
  cims:multiplicity cims:M:1..1;
  owl:inverseOf cim:OperationalLimitType.OperationalLimit .

cim:OperationalLimitDirectionKind a owl:Class;
  rdfs:comment "The direction attribute describes the side of  a limit that is a violation."@en;
  rdfs:label "OperationalLimitDirectionKind" .

cim:OperationalLimitDirectionKind.absoluteValue a cim:OperationalLimitDirectionKind;
  rdfs:comment "An absoluteValue limit means that a monitored absolute value above the limit value is a violation."@en;
  rdfs:label "absoluteValue" .

cim:OperationalLimitDirectionKind.high a cim:OperationalLimitDirectionKind;
  rdfs:comment "High means that a monitored value above the limit value is a violation.   If applied to a terminal flow, the positive direction is into the terminal."@en;
  rdfs:label "high" .

cim:OperationalLimitDirectionKind.low a cim:OperationalLimitDirectionKind;
  rdfs:comment "Low means a monitored value below the limit is a violation.  If applied to a terminal flow, the positive direction is into the terminal."@en;
  rdfs:label "low" .

cim:OperationalLimitSet a owl:Class;
  rdfs:comment "A set of limits associated with equipment.  Sets of limits might apply to a specific temperature, or season for example. A set of limits may contain different severities of limit levels that would apply to the same equipment. The set may contain limits of different types such as apparent power and current limits or high and low voltage limits  that are logically applied together as a set."@en;
  rdfs:subClassOf cim:IdentifiedObject;
  rdfs:label "OperationalLimitSet" .

cim:OperationalLimitSet.OperationalLimitValue a owl:ObjectProperty, owl:InverseFunctionalProperty;
  rdfs:comment "Values of equipment limits."@en;
  rdfs:domain cim:OperationalLimitSet;
  rdfs:range cim:OperationalLimit;
  rdfs:label "OperationalLimitValue";
  cims:multiplicity cims:M:0..n, cims:M:1..n;
  owl:inverseOf cim:OperationalLimit.OperationalLimitSet .

cim:OperationalLimitSet.Terminal a owl:ObjectProperty, owl:FunctionalProperty;
  rdfs:comment "The terminal where the operational limit set apply."@en;
  rdfs:domain cim:OperationalLimitSet;
  rdfs:range cim:ACDCTerminal;
  rdfs:label "Terminal";
  cims:multiplicity cims:M:1..1;
  owl:inverseOf cim:ACDCTerminal.OperationalLimitSet .

cim:OperationalLimitType a owl:Class;
  rdfs:comment "The operational meaning of a category of limits."@en;
  rdfs:subClassOf cim:IdentifiedObject;
  rdfs:label "OperationalLimitType" .

cim:OperationalLimitType.OperationalLimit a owl:ObjectProperty, owl:InverseFunctionalProperty;
  rdfs:comment "The operational limits associated with this type of limit."@en;
  rdfs:domain cim:OperationalLimitType;
  rdfs:range cim:OperationalLimit;
  rdfs:label "OperationalLimit";
  cims:multiplicity cims:M:0..n, cims:M:1..n;
  owl:inverseOf cim:OperationalLimit.OperationalLimitType .

cim:OperationalLimitType.acceptableDuration a owl:FunctionalProperty, owl:DatatypeProperty;
  rdfs:comment "The nominal acceptable duration of the limit. Limits are commonly expressed in terms of the time limit for which the limit is normally acceptable. The actual acceptable duration of a specific limit may depend on other local factors such as temperature or wind speed. The attribute has meaning only if the flag isInfiniteDuration is set to false, hence it shall not be exchanged when isInfiniteDuration is set to true."@en;
  rdfs:domain cim:OperationalLimitType;
  rdfs:range xsd:float;
  rdfs:label "acceptableDuration";
  cims:multiplicity cims:M:0..1;
  cim:unitMultiplier cim:UnitMultiplier.none;
  cim:unitSymbol cim:UnitSymbol.s;
  qudt:hasQuantityKind cim:Seconds;
  qudt:hasUnit unit:SEC .

cim:OperationalLimitType.direction a owl:ObjectProperty, owl:FunctionalProperty;
  rdfs:comment "The direction of the limit."@en;
  rdfs:domain cim:OperationalLimitType;
  rdfs:range cim:OperationalLimitDirectionKind;
  rdfs:label "direction";
  cims:multiplicity cims:M:1..1 .

cim:OperationalLimitType.isInfiniteDuration a owl:FunctionalProperty, owl:DatatypeProperty;
  rdfs:comment "Defines if the operational limit type has infinite duration. If true, the limit has infinite duration. If false, the limit has definite duration which is defined by the attribute acceptableDuration."@en;
  rdfs:domain cim:OperationalLimitType;
  rdfs:range xsd:boolean;
  rdfs:label "isInfiniteDuration";
  cims:multiplicity cims:M:1..1 .

cim:Organisation a owl:Class;
  rdfs:comment "Organisation that might have roles as utility, contractor, supplier, manufacturer, customer, etc."@en;
  rdfs:subClassOf cim:IdentifiedObject;
  rdfs:label "Organisation" .

cim:Organisation.Roles a owl:ObjectProperty, owl:InverseFunctionalProperty;
  rdfs:comment "All roles of this organisation."@en;
  rdfs:domain cim:Organisation;
  rdfs:range cim:OrganisationRole;
  rdfs:label "Roles";
  cims:multiplicity cims:M:0..n;
  owl:inverseOf cim:OrganisationRole.Organisation .

cim:OrganisationRole a owl:Class;
  rdfs:comment "Identifies a way in which an organisation may participate in the utility enterprise (e.g., customer, manufacturer, etc)."@en;
  rdfs:subClassOf cim:IdentifiedObject;
  rdfs:label "OrganisationRole" .

cim:OrganisationRole.Organisation a owl:ObjectProperty, owl:FunctionalProperty;
  rdfs:comment "Organisation having this role."@en;
  rdfs:domain cim:OrganisationRole;
  rdfs:range cim:Organisation;
  rdfs:label "Organisation";
  cims:multiplicity cims:M:0..1;
  owl:inverseOf cim:Organisation.Roles .

cim:OrientationKind a owl:Class;
  rdfs:comment "The orientation of the coordinate system with respect to top, left, and the coordinate number system."@en;
  rdfs:label "OrientationKind" .

cim:OrientationKind.negative a cim:OrientationKind;
  rdfs:comment "For 2D diagrams, a negative orientation gives the left-hand orientation (favoured by computer graphics displays) with X values increasing from left to right and Y values increasing from top to bottom.   This is also known as a left hand orientation."@en;
  rdfs:label "negative" .

cim:OverheadWireInfo a owl:Class;
  rdfs:comment "Overhead wire data."@en;
  rdfs:subClassOf cim:WireInfo;
  rdfs:label "OverheadWireInfo" .

cim:PetersenCoil a owl:Class;
  rdfs:comment "A variable impedance device normally used to offset line charging during single line faults in an ungrounded section of network."@en;
  rdfs:subClassOf cim:EarthFaultCompensator;
  rdfs:label "PetersenCoil" .

cim:PetersenCoilModeKind a owl:Class;
  rdfs:comment "The mode of operation for a Petersen coil."@en;
  rdfs:label "PetersenCoilModeKind" .

cim:PhaseCode a owl:Class;
  rdfs:comment "An unordered enumeration of phase identifiers.  Allows designation of phases for both transmission and distribution equipment, circuits and loads.   The enumeration, by itself, does not describe how the phases are connected together or connected to ground.  Ground is not explicitly denoted as a phase. Residential and small commercial loads are often served from single-phase, or split-phase, secondary circuits. For the example of s12N, phases 1 and 2 refer to hot wires that are 180 degrees out of"@en;
  rdfs:label "PhaseCode" .

cim:PhaseCode.A a cim:PhaseCode;
  rdfs:comment "Phase A."@en;
  rdfs:label "A" .

cim:PhaseCode.AB a cim:PhaseCode;
  rdfs:comment "Phases A and B."@en;
  rdfs:label "AB" .

cim:PhaseCode.ABC a cim:PhaseCode;
  rdfs:comment "Phases A, B, and C."@en;
  rdfs:label "ABC" .

cim:PhaseCode.ABCN a cim:PhaseCode;
  rdfs:comment "Phases A, B, C, and N."@en;
  rdfs:label "ABCN" .

cim:PhaseCode.AC a cim:PhaseCode;
  rdfs:comment "Phases A and C."@en;
  rdfs:label "AC" .

cim:PhaseCode.B a cim:PhaseCode;
  rdfs:comment "Phase B."@en;
  rdfs:label "B" .

cim:PhaseCode.BC a cim:PhaseCode;
  rdfs:comment "Phases B and C."@en;
  rdfs:label "BC" .

cim:PhaseCode.C a cim:PhaseCode;
  rdfs:comment "Phase C."@en;
  rdfs:label "C" .

cim:PhaseCode.N a cim:PhaseCode;
  rdfs:comment "Neutral phase."@en;
  rdfs:label "N" .

cim:PhaseCode.none a cim:PhaseCode;
  rdfs:comment "No phases specified."@en;
  rdfs:label "none" .

cim:PhaseConnectedFaultKind a owl:Class;
  rdfs:comment "The type of fault connection among phases."@en;
  rdfs:label "PhaseConnectedFaultKind" .

cim:PotentialTransformer a owl:Class;
  rdfs:comment "Instrument transformer (also known as Voltage Transformer) used to measure electrical qualities of the circuit that is being protected and/or monitored. Typically used as voltage transducer for the purpose of metering, protection, or sometimes auxiliary substation supply. A typical secondary voltage rating would be 120V."@en;
  rdfs:subClassOf cim:Sensor;
  rdfs:label "PotentialTransformer" .

cim:PowerSystemResource a owl:Class;
  rdfs:comment "A power system resource (PSR) can be an item of equipment such as a switch, an equipment container containing many individual items of equipment such as a substation, or an organisational entity such as sub-control area. Power system resources can have measurements associated."@en;
  rdfs:subClassOf cim:IdentifiedObject;
  rdfs:label "PowerSystemResource" .

cim:PowerSystemResource.Assets a owl:ObjectProperty;
  rdfs:comment "All assets represented by this power system resource. For example, multiple conductor assets are electrically modelled as a single AC line segment."@en;
  rdfs:domain cim:PowerSystemResource;
  rdfs:range cim:Asset;
  rdfs:label "Assets";
  cims:multiplicity cims:M:0..n;
  owl:inverseOf cim:Asset.PowerSystemResources .

cim:PowerSystemResource.Location a owl:ObjectProperty, owl:InverseFunctionalProperty,
    owl:FunctionalProperty;
  rdfs:comment "Location of this power system resource."@en;
  rdfs:domain cim:PowerSystemResource;
  rdfs:range cim:Location;
  rdfs:label "Location";
  cims:multiplicity cims:M:0..1;
  owl:inverseOf cim:Location.PowerSystemResources .

cim:PowerSystemResource.Measurements a owl:ObjectProperty, owl:InverseFunctionalProperty;
  rdfs:comment "The measurements associated with this power system resource."@en;
  rdfs:domain cim:PowerSystemResource;
  rdfs:range cim:Measurement;
  rdfs:label "Measurements";
  cims:multiplicity cims:M:0..n;
  owl:inverseOf cim:Measurement.PowerSystemResource .

cim:PowerTransformer a owl:Class;
  rdfs:comment "An electrical device consisting of  two or more coupled windings, with or without a magnetic core, for introducing mutual coupling between electric circuits. Transformers can be used to control voltage and phase shift (active power flow). A power transformer may be composed of separate transformer tanks that need not be identical. A power transformer can be modelled with or without tanks and is intended for use in both balanced and unbalanced representations.   A power transformer typically has two"@en;
  rdfs:subClassOf cim:ConductingEquipment;
  rdfs:label "PowerTransformer" .

cim:PowerTransformer.PowerTransformerEnd a owl:ObjectProperty, owl:InverseFunctionalProperty;
  rdfs:comment "The ends of this power transformer."@en;
  rdfs:domain cim:PowerTransformer;
  rdfs:range cim:PowerTransformerEnd;
  rdfs:label "PowerTransformerEnd";
  cims:multiplicity cims:M:0..n;
  owl:inverseOf cim:PowerTransformerEnd.PowerTransformer .

cim:PowerTransformer.isPartOfGeneratorUnit a owl:FunctionalProperty, owl:DatatypeProperty;
  rdfs:comment "Indicates whether the machine is part of a power station unit. Used for short circuit data exchange according to IEC 60909.  It has an impact on how the correction factors are calculated for transformers, since the transformer is not necessarily part of a synchronous machine and generating unit. It is not always possible to derive this information from the model. This is why the attribute is necessary."@en;
  rdfs:domain cim:PowerTransformer;
  rdfs:range xsd:boolean;
  rdfs:label "isPartOfGeneratorUnit";
  cims:multiplicity cims:M:1..1 .

cim:PowerTransformerEnd a owl:Class;
  rdfs:comment "A PowerTransformerEnd is associated with each Terminal of a PowerTransformer. The impedance values r, r0, x, and x0 of a PowerTransformerEnd represents a star equivalent as follows. 1) for a two Terminal PowerTransformer the high voltage (TransformerEnd.endNumber=1) PowerTransformerEnd has non zero values on r, r0, x, and x0 while the low voltage (TransformerEnd.endNumber=2) PowerTransformerEnd has zero values for r, r0, x, and x0.  Parameters are always provided, even if the PowerTransformerEnds"@en;
  rdfs:subClassOf cim:TransformerEnd;
  rdfs:label "PowerTransformerEnd" .

cim:PowerTransformerEnd.PowerTransformer a owl:ObjectProperty, owl:FunctionalProperty;
  rdfs:comment "The power transformer of this power transformer end."@en;
  rdfs:domain cim:PowerTransformerEnd;
  rdfs:range cim:PowerTransformer;
  rdfs:label "PowerTransformer";
  cims:multiplicity cims:M:1..1;
  owl:inverseOf cim:PowerTransformer.PowerTransformerEnd .

cim:PowerTransformerEnd.b a owl:FunctionalProperty, owl:DatatypeProperty;
  rdfs:comment "Magnetizing branch susceptance (B mag).  The value can be positive or negative."@en;
  rdfs:domain cim:PowerTransformerEnd;
  rdfs:range xsd:float;
  rdfs:label "b";
  cims:multiplicity cims:M:1..1;
  cim:unitMultiplier cim:UnitMultiplier.none;
  cim:unitSymbol cim:UnitSymbol.S;
  qudt:hasQuantityKind cim:Susceptance;
  qudt:hasUnit unit:S .

cim:PowerTransformerEnd.connectionKind a owl:ObjectProperty, owl:FunctionalProperty;
  rdfs:comment "Kind of connection."@en;
  rdfs:domain cim:PowerTransformerEnd;
  rdfs:range cim:WindingConnection;
  rdfs:label "connectionKind";
  cims:multiplicity cims:M:0..1 .

cim:PowerTransformerEnd.g a owl:FunctionalProperty, owl:DatatypeProperty;
  rdfs:comment "Magnetizing branch conductance."@en;
  rdfs:domain cim:PowerTransformerEnd;
  rdfs:range xsd:float;
  rdfs:label "g";
  cims:multiplicity cims:M:0..1;
  cim:unitMultiplier cim:UnitMultiplier.none;
  cim:unitSymbol cim:UnitSymbol.S;
  qudt:hasQuantityKind cim:Conductance;
  qudt:hasUnit unit:S .

cim:PowerTransformerEnd.r a owl:FunctionalProperty, owl:DatatypeProperty;
  rdfs:comment """Resistance (star-model) of the transformer end.
The attribute shall be equal to or greater than zero for non-equivalent transformers."""@en;
  rdfs:domain cim:PowerTransformerEnd;
  rdfs:range xsd:float;
  rdfs:label "r";
  cims:multiplicity cims:M:1..1;
  cim:unitMultiplier cim:UnitMultiplier.none;
  cim:unitSymbol cim:UnitSymbol.ohm;
  qudt:hasQuantityKind cim:Resistance;
  qudt:hasUnit unit:OHM .

cim:PowerTransformerEnd.ratedS a owl:FunctionalProperty, owl:DatatypeProperty;
  rdfs:comment """Normal apparent power rating.
The attribute shall be a positive value. For a two-winding transformer the values for the high and low voltage sides shall be identical."""@en;
  rdfs:domain cim:PowerTransformerEnd;
  rdfs:range xsd:float;
  rdfs:label "ratedS";
  cims:multiplicity cims:M:0..1;
  cim:unitMultiplier cim:UnitMultiplier.M;
  cim:unitSymbol cim:UnitSymbol.VA;
  qudt:hasQuantityKind cim:ApparentPower;
  qudt:hasUnit unit:MegaV-A .

cim:PowerTransformerEnd.ratedU a owl:FunctionalProperty, owl:DatatypeProperty;
  rdfs:comment """Rated voltage: phase-phase for three-phase windings, and either phase-phase or phase-neutral for single-phase windings.
A high voltage side, as given by TransformerEnd.endNumber, shall have a ratedU that is greater than or equal to ratedU for the lower voltage sides.
The attribute shall be a positive value."""@en;
  rdfs:domain cim:PowerTransformerEnd;
  rdfs:range xsd:float;
  rdfs:label "ratedU";
  cims:multiplicity cims:M:1..1;
  cim:unitMultiplier cim:UnitMultiplier.k;
  cim:unitSymbol cim:UnitSymbol.V;
  qudt:hasQuantityKind cim:Voltage;
  qudt:hasUnit unit:KiloV .

cim:PowerTransformerEnd.x a owl:FunctionalProperty, owl:DatatypeProperty;
  rdfs:comment "Positive sequence series reactance (star-model) of the transformer end."@en;
  rdfs:domain cim:PowerTransformerEnd;
  rdfs:range xsd:float;
  rdfs:label "x";
  cims:multiplicity cims:M:1..1;
  cim:unitMultiplier cim:UnitMultiplier.none;
  cim:unitSymbol cim:UnitSymbol.ohm;
  qudt:hasQuantityKind cim:Reactance;
  qudt:hasUnit unit:OHM .

cim:ProductAssetModel a owl:Class;
  rdfs:comment "Asset model by a specific manufacturer."@en;
  rdfs:subClassOf cim:IdentifiedObject;
  rdfs:label "ProductAssetModel" .

cim:ProductAssetModel.AssetInfo a owl:ObjectProperty, owl:InverseFunctionalProperty,
    owl:FunctionalProperty;
  rdfs:comment "Asset information (nameplate) for this product asset model."@en;
  rdfs:domain cim:ProductAssetModel;
  rdfs:range cim:AssetInfo;
  rdfs:label "AssetInfo";
  cims:multiplicity cims:M:0..1;
  owl:inverseOf cim:AssetInfo.ProductAssetModel .

cim:ProductAssetModel.Manufacturer a owl:ObjectProperty, owl:FunctionalProperty;
  rdfs:comment "Manufacturer of this asset model."@en;
  rdfs:domain cim:ProductAssetModel;
  rdfs:range cim:Manufacturer;
  rdfs:label "Manufacturer";
  cims:multiplicity cims:M:0..1;
  owl:inverseOf cim:Manufacturer.ProductAssetModels .

cim:ProductAssetModel.modelNumber a owl:ObjectProperty, owl:FunctionalProperty;
  rdfs:comment "Manufacturer's model number."@en;
  rdfs:domain cim:ProductAssetModel;
  rdfs:label "modelNumber";
  cims:multiplicity cims:M:0..1;
  cims:dataType cim:String .

cim:ProductAssetModel.modelVersion a owl:ObjectProperty, owl:FunctionalProperty;
  rdfs:comment "Version number for product model, which indicates vintage of the product."@en;
  rdfs:domain cim:ProductAssetModel;
  rdfs:label "modelVersion";
  cims:multiplicity cims:M:0..1;
  cims:dataType cim:String .

cim:ProductAssetModel.usageKind a owl:ObjectProperty, owl:FunctionalProperty;
  rdfs:comment "Intended usage for this asset model."@en;
  rdfs:domain cim:ProductAssetModel;
  rdfs:range cim:AssetModelUsageKind;
  rdfs:label "usageKind";
  cims:multiplicity cims:M:0..1 .

cim:ProtectedSwitch a owl:Class;
  rdfs:comment "A ProtectedSwitch is a switching device that can be operated by ProtectionEquipment."@en;
  rdfs:subClassOf cim:Switch;
  rdfs:label "ProtectedSwitch" .

cim:RatioTapChanger a owl:Class;
  rdfs:comment """A tap changer that changes the voltage ratio impacting the voltage magnitude but not the phase angle across the transformer.

Angle sign convention (general): Positive value indicates a positive phase shift from the winding where the tap is located to the other winding (for a two-winding transformer)."""@en;
  rdfs:subClassOf cim:TapChanger;
  rdfs:label "RatioTapChanger" .

cim:RatioTapChanger.TransformerEnd a owl:ObjectProperty, owl:InverseFunctionalProperty,
    owl:FunctionalProperty;
  rdfs:comment "Transformer end to which this ratio tap changer belongs."@en;
  rdfs:domain cim:RatioTapChanger;
  rdfs:range cim:TransformerEnd;
  rdfs:label "TransformerEnd";
  cims:multiplicity cims:M:1..1;
  owl:inverseOf cim:TransformerEnd.RatioTapChanger .

cim:RatioTapChanger.stepVoltageIncrement a owl:FunctionalProperty, owl:DatatypeProperty;
  rdfs:comment """Tap step increment, in per cent of rated voltage of the power transformer end, per step position.
When the increment is negative, the voltage decreases when the tap step increases."""@en;
  rdfs:domain cim:RatioTapChanger;
  rdfs:range xsd:float;
  rdfs:label "stepVoltageIncrement";
  cims:multiplicity cims:M:1..1;
  cim:unitMultiplier cim:UnitMultiplier.none;
  cim:unitSymbol cim:UnitSymbol.none;
  qudt:hasQuantityKind cim:PerCent;
  qudt:hasUnit unit:PERCENT .

cim:RegulatingCondEq a owl:Class;
  rdfs:comment "A type of conducting equipment that can regulate a quantity (i.e. voltage or flow) at a specific point in the network."@en;
  rdfs:subClassOf cim:EnergyConnection;
  rdfs:label "RegulatingCondEq" .

cim:RegulatingCondEq.RegulatingControl a owl:ObjectProperty, owl:FunctionalProperty;
  rdfs:comment "The regulating control scheme in which this equipment participates."@en;
  rdfs:domain cim:RegulatingCondEq;
  rdfs:range cim:RegulatingControl;
  rdfs:label "RegulatingControl";
  cims:multiplicity cims:M:0..1;
  owl:inverseOf cim:RegulatingControl.RegulatingCondEq .

cim:RegulatingCondEq.controlEnabled a owl:FunctionalProperty, owl:DatatypeProperty;
  rdfs:comment "Specifies the regulation status of the equipment.  True is regulating, false is not regulating."@en;
  rdfs:domain cim:RegulatingCondEq;
  rdfs:range xsd:boolean;
  rdfs:label "controlEnabled";
  cims:multiplicity cims:M:1..1 .

cim:RegulatingControl a owl:Class;
  rdfs:comment "Specifies a set of equipment that works together to control a power system quantity such as voltage or flow.  Remote bus voltage control is possible by specifying the controlled terminal located at some place remote from the controlling equipment. The specified terminal shall be associated with the connectivity node of the controlled point.  The most specific subtype of RegulatingControl shall be used in case such equipment participate in the control, e.g. TapChangerControl for tap changers. For"@en;
  rdfs:subClassOf cim:PowerSystemResource;
  rdfs:label "RegulatingControl" .

cim:RegulatingControl.RegulatingCondEq a owl:ObjectProperty, owl:InverseFunctionalProperty;
  rdfs:comment "The equipment that participates in this regulating control scheme."@en;
  rdfs:domain cim:RegulatingControl;
  rdfs:range cim:RegulatingCondEq;
  rdfs:label "RegulatingCondEq";
  cims:multiplicity cims:M:0..n;
  owl:inverseOf cim:RegulatingCondEq.RegulatingControl .

cim:RegulatingControl.Terminal a owl:ObjectProperty, owl:FunctionalProperty;
  rdfs:comment "The terminal associated with this regulating control.  The terminal is associated instead of a node, since the terminal could connect into either a topological node or a connectivity node.  Sometimes it is useful to model regulation at a terminal of a bus bar object."@en;
  rdfs:domain cim:RegulatingControl;
  rdfs:range cim:Terminal;
  rdfs:label "Terminal";
  cims:multiplicity cims:M:1..1;
  owl:inverseOf cim:Terminal.RegulatingControl .

cim:RegulatingControl.discrete a owl:FunctionalProperty, owl:DatatypeProperty;
  rdfs:comment "The regulation is performed in a discrete mode. This applies to equipment with discrete controls, e.g. tap changers and shunt compensators."@en;
  rdfs:domain cim:RegulatingControl;
  rdfs:range xsd:boolean;
  rdfs:label "discrete";
  cims:multiplicity cims:M:1..1 .

cim:RegulatingControl.enabled a owl:FunctionalProperty, owl:DatatypeProperty;
  rdfs:comment "The flag tells if regulation is enabled."@en;
  rdfs:domain cim:RegulatingControl;
  rdfs:range xsd:boolean;
  rdfs:label "enabled";
  cims:multiplicity cims:M:1..1 .

cim:RegulatingControl.mode a owl:ObjectProperty, owl:FunctionalProperty;
  rdfs:comment "The regulating control mode presently available.  This specification allows for determining the kind of regulation without need for obtaining the units from a schedule."@en;
  rdfs:domain cim:RegulatingControl;
  rdfs:range cim:RegulatingControlModeKind;
  rdfs:label "mode";
  cims:multiplicity cims:M:1..1 .

cim:RegulatingControl.targetDeadband a owl:FunctionalProperty, owl:DatatypeProperty;
  rdfs:comment """This is a deadband used with discrete control to avoid excessive update of controls like tap changers and shunt compensator banks while regulating.  The units of those appropriate for the mode. The attribute shall be a positive value or zero. If RegulatingControl.discrete is set to \"false\", the RegulatingControl.targetDeadband is to be ignored.
Note that for instance, if the targetValue is 100 kV and the targetDeadband is 2 kV the range is from 99 to 101 kV."""@en;
  rdfs:domain cim:RegulatingControl;
  rdfs:range xsd:float;
  rdfs:label "targetDeadband";
  cims:multiplicity cims:M:0..1 .

cim:RegulatingControl.targetValue a owl:FunctionalProperty, owl:DatatypeProperty;
  rdfs:comment "The target value specified for case input.   This value can be used for the target value without the use of schedules. The value has the units appropriate to the mode attribute."@en;
  rdfs:domain cim:RegulatingControl;
  rdfs:range xsd:float;
  rdfs:label "targetValue";
  cims:multiplicity cims:M:1..1 .

cim:RegulatingControl.targetValueUnitMultiplier a owl:ObjectProperty, owl:FunctionalProperty;
  rdfs:comment "Specify the multiplier for used for the targetValue."@en;
  rdfs:domain cim:RegulatingControl;
  rdfs:range cim:UnitMultiplier;
  rdfs:label "targetValueUnitMultiplier";
  cims:multiplicity cims:M:1..1 .

cim:RegulatingControlModeKind a owl:Class;
  rdfs:comment "The kind of regulation model.   For example regulating voltage, reactive power, active power, etc."@en;
  rdfs:label "RegulatingControlModeKind" .

cim:RegulatingControlModeKind.voltage a cim:RegulatingControlModeKind;
  rdfs:comment "Voltage is specified."@en;
  rdfs:label "voltage" .

cim:RemoteSignalKind a owl:Class;
  rdfs:comment "Type of input signal coming from remote bus."@en;
  rdfs:label "RemoteSignalKind" .

cim:RotatingMachine a owl:Class;
  rdfs:comment "A rotating machine which may be used as a generator or motor."@en;
  rdfs:subClassOf cim:RegulatingCondEq;
  rdfs:label "RotatingMachine" .

cim:RotatingMachine.GeneratingUnit a owl:ObjectProperty, owl:FunctionalProperty;
  rdfs:comment "A synchronous machine may operate as a generator and as such becomes a member of a generating unit."@en;
  rdfs:domain cim:RotatingMachine;
  rdfs:range cim:GeneratingUnit;
  rdfs:label "GeneratingUnit";
  cims:multiplicity cims:M:0..1;
  owl:inverseOf cim:GeneratingUnit.RotatingMachine .

cim:RotatingMachine.p a owl:FunctionalProperty, owl:DatatypeProperty;
  rdfs:comment """Active power injection. Load sign convention is used, i.e. positive sign means flow out from a node.
Starting value for a steady state solution."""@en;
  rdfs:domain cim:RotatingMachine;
  rdfs:range xsd:float;
  rdfs:label "p";
  cims:multiplicity cims:M:1..1;
  cim:unitMultiplier cim:UnitMultiplier.M;
  cim:unitSymbol cim:UnitSymbol.W;
  qudt:hasQuantityKind cim:ActivePower;
  qudt:hasUnit unit:MegaW .

cim:RotatingMachine.q a owl:FunctionalProperty, owl:DatatypeProperty;
  rdfs:comment """Reactive power injection. Load sign convention is used, i.e. positive sign means flow out from a node.
Starting value for a steady state solution."""@en;
  rdfs:domain cim:RotatingMachine;
  rdfs:range xsd:float;
  rdfs:label "q";
  cims:multiplicity cims:M:1..1;
  cim:unitMultiplier cim:UnitMultiplier.M;
  cim:unitSymbol cim:UnitSymbol.VAr;
  qudt:hasQuantityKind cim:ReactivePower;
  qudt:hasUnit unit:MegaV-A_Reactive .

cim:RotatingMachine.ratedS a owl:FunctionalProperty, owl:DatatypeProperty;
  rdfs:comment """Nameplate apparent power rating for the unit.
The attribute shall have a positive value."""@en;
  rdfs:domain cim:RotatingMachine;
  rdfs:range xsd:float;
  rdfs:label "ratedS";
  cims:multiplicity cims:M:0..1;
  cim:unitMultiplier cim:UnitMultiplier.M;
  cim:unitSymbol cim:UnitSymbol.VA;
  qudt:hasQuantityKind cim:ApparentPower;
  qudt:hasUnit unit:MegaV-A .

cim:RotorKind a owl:Class;
  rdfs:comment "Type of rotor on physical machine."@en;
  rdfs:label "RotorKind" .

cim:SVCControlMode a owl:Class;
  rdfs:comment "Static VAr Compensator control mode."@en;
  rdfs:label "SVCControlMode";
  owl:deprecated true .

cim:Sensor a owl:Class;
  rdfs:comment "This class describe devices that transform a measured quantity into signals that can be presented at displays, used in control or be recorded."@en;
  rdfs:subClassOf cim:AuxiliaryEquipment;
  rdfs:label "Sensor" .

cim:ShortCircuitRotorKind a owl:Class;
  rdfs:comment "Type of rotor, used by short circuit applications."@en;
  rdfs:label "ShortCircuitRotorKind" .

cim:ShuntCompensator a owl:Class;
  rdfs:comment "A shunt capacitor or reactor or switchable bank of shunt capacitors or reactors. A section of a shunt compensator is an individual capacitor or reactor. A negative value for bPerSection indicates that the compensator is a reactor. ShuntCompensator is a single terminal device.  Ground is implied."@en;
  rdfs:subClassOf cim:RegulatingCondEq;
  rdfs:label "ShuntCompensator" .

cim:ShuntCompensator.SvShuntCompensatorSections a owl:ObjectProperty, owl:InverseFunctionalProperty,
    owl:FunctionalProperty;
  rdfs:comment "The state for the number of shunt compensator sections in service."@en;
  rdfs:domain cim:ShuntCompensator;
  rdfs:range cim:SvShuntCompensatorSections;
  rdfs:label "SvShuntCompensatorSections";
  cims:multiplicity cims:M:0..1;
  owl:inverseOf cim:SvShuntCompensatorSections.ShuntCompensator .

cim:ShuntCompensator.aVRDelay a owl:FunctionalProperty, owl:DatatypeProperty;
  rdfs:comment "An automatic voltage regulation delay (AVRDelay) which is the time delay from a change in voltage to when the capacitor is allowed to change state. This filters out temporary changes in voltage."@en;
  rdfs:domain cim:ShuntCompensator;
  rdfs:range xsd:float;
  rdfs:label "aVRDelay";
  cims:multiplicity cims:M:0..1;
  cim:unitMultiplier cim:UnitMultiplier.none;
  cim:unitSymbol cim:UnitSymbol.s;
  qudt:hasQuantityKind cim:Seconds;
  qudt:hasUnit unit:SEC .

cim:ShuntCompensator.maximumSections a owl:FunctionalProperty, owl:DatatypeProperty;
  rdfs:comment "The maximum number of sections that may be switched in."@en;
  rdfs:domain cim:ShuntCompensator;
  rdfs:range xsd:integer;
  rdfs:label "maximumSections";
  cims:multiplicity cims:M:1..1 .

cim:ShuntCompensator.nomU a owl:FunctionalProperty, owl:DatatypeProperty;
  rdfs:comment "The voltage at which the nominal reactive power may be calculated. This should normally be within 10% of the voltage at which the capacitor is connected to the network."@en;
  rdfs:domain cim:ShuntCompensator;
  rdfs:range xsd:float;
  rdfs:label "nomU";
  cims:multiplicity cims:M:1..1;
  cim:unitMultiplier cim:UnitMultiplier.k;
  cim:unitSymbol cim:UnitSymbol.V;
  qudt:hasQuantityKind cim:Voltage;
  qudt:hasUnit unit:KiloV .

cim:ShuntCompensator.normalSections a owl:FunctionalProperty, owl:DatatypeProperty;
  rdfs:comment "The normal number of sections switched in. The value shall be between zero and ShuntCompensator.maximumSections."@en;
  rdfs:domain cim:ShuntCompensator;
  rdfs:range xsd:integer;
  rdfs:label "normalSections";
  cims:multiplicity cims:M:1..1 .

cim:ShuntCompensator.sections a owl:FunctionalProperty, owl:DatatypeProperty;
  rdfs:comment "Shunt compensator sections in use. Starting value for steady state solution. The attribute shall be a positive value or zero. Non integer values are allowed to support continuous variables. The reasons for continuous value are to support study cases where no discrete shunt compensators has yet been designed, a solutions where a narrow voltage band force the sections to oscillate or accommodate for a continuous solution as input.  For LinearShuntConpensator the value shall be between zero and ShuntCompensator.maximumSections."@en;
  rdfs:domain cim:ShuntCompensator;
  rdfs:range xsd:float;
  rdfs:label "sections";
  cims:multiplicity cims:M:1..1 .

cim:ShuntCompensatorInfo a owl:Class;
  rdfs:comment "Properties of shunt capacitor, shunt reactor or switchable bank of shunt capacitor or reactor assets."@en;
  rdfs:subClassOf cim:AssetInfo;
  rdfs:label "ShuntCompensatorInfo" .

cim:ShuntCompensatorInfo.ratedReactivePower a owl:ObjectProperty, owl:FunctionalProperty;
  rdfs:comment "Rated reactive power."@en;
  rdfs:domain cim:ShuntCompensatorInfo;
  rdfs:label "ratedReactivePower";
  cims:multiplicity cims:M:0..1;
  cims:dataType cim:ReactivePower .

cim:ShuntCompensatorInfo.ratedVoltage a owl:ObjectProperty, owl:FunctionalProperty;
  rdfs:comment "Rated voltage."@en;
  rdfs:domain cim:ShuntCompensatorInfo;
  rdfs:label "ratedVoltage";
  cims:multiplicity cims:M:0..1;
  cims:dataType cim:Voltage .

cim:SinglePhaseKind a owl:Class;
  rdfs:comment "Enumeration of single phase identifiers. Allows designation of single phases for both transmission and distribution equipment, circuits and loads."@en;
  rdfs:label "SinglePhaseKind" .

cim:Source a owl:Class;
  rdfs:comment "Source gives information related to the origin of a value."@en;
  rdfs:label "Source" .

cim:StaticLoadModelKind a owl:Class;
  rdfs:comment "Type of static load model."@en;
  rdfs:label "StaticLoadModelKind" .

cim:StationSupply a owl:Class;
  rdfs:comment "Station supply with load derived from the station output."@en;
  rdfs:subClassOf cim:EnergyConsumer;
  rdfs:label "StationSupply" .

cim:SubGeographicalRegion a owl:Class;
  rdfs:comment "A subset of a geographical region of a power system network model."@en;
  rdfs:subClassOf cim:IdentifiedObject;
  rdfs:label "SubGeographicalRegion" .

cim:SubGeographicalRegion.Lines a owl:ObjectProperty, owl:InverseFunctionalProperty;
  rdfs:comment "The lines within the sub-geographical region."@en;
  rdfs:domain cim:SubGeographicalRegion;
  rdfs:range cim:Line;
  rdfs:label "Lines";
  cims:multiplicity cims:M:0..n;
  owl:inverseOf cim:Line.Region .

cim:SubGeographicalRegion.Region a owl:ObjectProperty, owl:FunctionalProperty;
  rdfs:comment "The geographical region which this sub-geographical region is within."@en;
  rdfs:domain cim:SubGeographicalRegion;
  rdfs:range cim:GeographicalRegion;
  rdfs:label "Region";
  cims:multiplicity cims:M:1..1;
  owl:inverseOf cim:GeographicalRegion.Regions .

cim:SubGeographicalRegion.Substations a owl:ObjectProperty, owl:InverseFunctionalProperty;
  rdfs:comment "The substations in this sub-geographical region."@en;
  rdfs:domain cim:SubGeographicalRegion;
  rdfs:range cim:Substation;
  rdfs:label "Substations";
  cims:multiplicity cims:M:0..n;
  owl:inverseOf cim:Substation.Region .

cim:SubLoadArea a owl:Class;
  rdfs:comment "The class is the second level in a hierarchical structure for grouping of loads for the purpose of load flow load scaling."@en;
  rdfs:subClassOf cim:EnergyArea;
  rdfs:label "SubLoadArea" .

cim:SubLoadArea.LoadArea a owl:ObjectProperty, owl:FunctionalProperty;
  rdfs:comment "The LoadArea where the SubLoadArea belongs."@en;
  rdfs:domain cim:SubLoadArea;
  rdfs:range cim:LoadArea;
  rdfs:label "LoadArea";
  cims:multiplicity cims:M:1..1;
  owl:inverseOf cim:LoadArea.SubLoadAreas .

cim:SubLoadArea.LoadGroups a owl:ObjectProperty, owl:InverseFunctionalProperty;
  rdfs:comment "The Loadgroups in the SubLoadArea."@en;
  rdfs:domain cim:SubLoadArea;
  rdfs:range cim:LoadGroup;
  rdfs:label "LoadGroups";
  cims:multiplicity cims:M:1..n;
  owl:inverseOf cim:LoadGroup.SubLoadArea .

cim:Substation a owl:Class;
  rdfs:comment "A collection of equipment for purposes other than generation or utilization, through which electric energy in bulk is passed for the purposes of switching or modifying its characteristics."@en;
  rdfs:subClassOf cim:EquipmentContainer;
  rdfs:label "Substation" .

cim:Substation.Region a owl:ObjectProperty, owl:FunctionalProperty;
  rdfs:comment "The SubGeographicalRegion containing the substation."@en;
  rdfs:domain cim:Substation;
  rdfs:range cim:SubGeographicalRegion;
  rdfs:label "Region";
  cims:multiplicity cims:M:1..1;
  owl:inverseOf cim:SubGeographicalRegion.Substations .

cim:Substation.VoltageLevels a owl:ObjectProperty, owl:InverseFunctionalProperty;
  rdfs:comment "The voltage levels within this substation."@en;
  rdfs:subPropertyOf cimr:hasPart;
  rdfs:domain cim:Substation;
  rdfs:range cim:VoltageLevel;
  rdfs:label "VoltageLevels";
  cims:multiplicity cims:M:0..n;
  owl:inverseOf cim:VoltageLevel.Substation .

cim:SvPowerFlow a owl:Class;
  rdfs:comment "State variable for power flow. Load convention is used for flow direction. This means flow out from the TopologicalNode into the equipment is positive."@en;
  rdfs:label "SvPowerFlow" .

cim:SvPowerFlow.Terminal a owl:ObjectProperty, owl:InverseFunctionalProperty, owl:FunctionalProperty;
  rdfs:comment "The terminal associated with the power flow state variable."@en;
  rdfs:domain cim:SvPowerFlow;
  rdfs:range cim:Terminal;
  rdfs:label "Terminal";
  cims:multiplicity cims:M:1..1;
  owl:inverseOf cim:Terminal.SvPowerFlow .

cim:SvPowerFlow.p a owl:FunctionalProperty, owl:DatatypeProperty;
  rdfs:comment "The active power flow. Load sign convention is used, i.e. positive sign means flow out from a TopologicalNode (bus) into the conducting equipment."@en;
  rdfs:domain cim:SvPowerFlow;
  rdfs:range xsd:float;
  rdfs:label "p";
  cims:multiplicity cims:M:1..1;
  cim:unitMultiplier cim:UnitMultiplier.M;
  cim:unitSymbol cim:UnitSymbol.W;
  qudt:hasQuantityKind cim:ActivePower;
  qudt:hasUnit unit:MegaW .

cim:SvPowerFlow.q a owl:FunctionalProperty, owl:DatatypeProperty;
  rdfs:comment "The reactive power flow. Load sign convention is used, i.e. positive sign means flow out from a TopologicalNode (bus) into the conducting equipment."@en;
  rdfs:domain cim:SvPowerFlow;
  rdfs:range xsd:float;
  rdfs:label "q";
  cims:multiplicity cims:M:1..1;
  cim:unitMultiplier cim:UnitMultiplier.M;
  cim:unitSymbol cim:UnitSymbol.VAr;
  qudt:hasQuantityKind cim:ReactivePower;
  qudt:hasUnit unit:MegaV-A_Reactive .

cim:SvShuntCompensatorSections a owl:Class;
  rdfs:comment "State variable for the number of sections in service for a shunt compensator."@en;
  rdfs:label "SvShuntCompensatorSections" .

cim:SvShuntCompensatorSections.ShuntCompensator a owl:ObjectProperty, owl:InverseFunctionalProperty,
    owl:FunctionalProperty;
  rdfs:comment "The shunt compensator for which the state applies."@en;
  rdfs:domain cim:SvShuntCompensatorSections;
  rdfs:range cim:ShuntCompensator;
  rdfs:label "ShuntCompensator";
  cims:multiplicity cims:M:1..1;
  owl:inverseOf cim:ShuntCompensator.SvShuntCompensatorSections .

cim:SvShuntCompensatorSections.sections a owl:FunctionalProperty, owl:DatatypeProperty;
  rdfs:comment "The number of sections in service as a continuous variable. The attribute shall be a positive value or zero. To get integer value scale with ShuntCompensator.bPerSection."@en;
  rdfs:domain cim:SvShuntCompensatorSections;
  rdfs:range xsd:float;
  rdfs:label "sections";
  cims:multiplicity cims:M:1..1 .

cim:SvStatus a owl:Class;
  rdfs:comment "State variable for status."@en;
  rdfs:label "SvStatus" .

cim:SvStatus.ConductingEquipment a owl:ObjectProperty, owl:InverseFunctionalProperty,
    owl:FunctionalProperty;
  rdfs:comment "The conducting equipment associated with the status state variable."@en;
  rdfs:domain cim:SvStatus;
  rdfs:range cim:ConductingEquipment;
  rdfs:label "ConductingEquipment";
  cims:multiplicity cims:M:1..1;
  owl:inverseOf cim:ConductingEquipment.SvStatus .

cim:SvStatus.inService a owl:FunctionalProperty, owl:DatatypeProperty;
  rdfs:comment "The in service status as a result of topology processing.  It indicates if the equipment is considered as energized by the power flow. It reflects if the equipment is connected within a solvable island.  It does not necessarily reflect whether or not the island was solved by the power flow."@en;
  rdfs:domain cim:SvStatus;
  rdfs:range xsd:boolean;
  rdfs:label "inService";
  cims:multiplicity cims:M:1..1 .

cim:SvSwitch a owl:Class;
  rdfs:comment "State variable for switch."@en;
  rdfs:label "SvSwitch" .

cim:SvSwitch.Switch a owl:ObjectProperty, owl:FunctionalProperty;
  rdfs:comment "The switch associated with the switch state."@en;
  rdfs:domain cim:SvSwitch;
  rdfs:range cim:Switch;
  rdfs:label "Switch";
  cims:multiplicity cims:M:1..1;
  owl:inverseOf cim:Switch.SvSwitch .

cim:SvSwitch.open a owl:FunctionalProperty, owl:DatatypeProperty;
  rdfs:comment "The attribute tells if the computed state of the switch is considered open."@en;
  rdfs:domain cim:SvSwitch;
  rdfs:range xsd:boolean;
  rdfs:label "open";
  cims:multiplicity cims:M:1..1 .

cim:SvTapStep a owl:Class;
  rdfs:comment "State variable for transformer tap step."@en;
  rdfs:label "SvTapStep" .

cim:SvTapStep.TapChanger a owl:ObjectProperty, owl:InverseFunctionalProperty, owl:FunctionalProperty;
  rdfs:comment "The tap changer associated with the tap step state."@en;
  rdfs:domain cim:SvTapStep;
  rdfs:range cim:TapChanger;
  rdfs:label "TapChanger";
  cims:multiplicity cims:M:1..1;
  owl:inverseOf cim:TapChanger.SvTapStep .

cim:SvTapStep.position a owl:FunctionalProperty, owl:DatatypeProperty;
  rdfs:comment "The floating point tap position.   This is not the tap ratio, but rather the tap step position as defined by the related tap changer model and normally is constrained to be within the range of minimum and maximum tap positions."@en;
  rdfs:domain cim:SvTapStep;
  rdfs:range xsd:float;
  rdfs:label "position";
  cims:multiplicity cims:M:1..1 .

cim:SvVoltage a owl:Class;
  rdfs:comment "State variable for voltage."@en;
  rdfs:label "SvVoltage" .

cim:SvVoltage.TopologicalNode a owl:ObjectProperty, owl:InverseFunctionalProperty,
    owl:FunctionalProperty;
  rdfs:comment "The topological node associated with the voltage state."@en;
  rdfs:domain cim:SvVoltage;
  rdfs:range cim:TopologicalNode;
  rdfs:label "TopologicalNode";
  cims:multiplicity cims:M:1..1;
  owl:inverseOf cim:TopologicalNode.SvVoltage .

cim:SvVoltage.angle a owl:FunctionalProperty, owl:DatatypeProperty;
  rdfs:comment "The voltage angle of the topological node complex voltage with respect to system reference."@en;
  rdfs:domain cim:SvVoltage;
  rdfs:range xsd:float;
  rdfs:label "angle";
  cims:multiplicity cims:M:1..1;
  cim:unitMultiplier cim:UnitMultiplier.none;
  cim:unitSymbol cim:UnitSymbol.deg;
  qudt:hasQuantityKind cim:AngleDegrees;
  qudt:hasUnit unit:DEG .

cim:SvVoltage.v a owl:FunctionalProperty, owl:DatatypeProperty;
  rdfs:comment "The voltage magnitude at the topological node. The attribute shall be a positive value."@en;
  rdfs:domain cim:SvVoltage;
  rdfs:range xsd:float;
  rdfs:label "v";
  cims:multiplicity cims:M:1..1;
  cim:unitMultiplier cim:UnitMultiplier.k;
  cim:unitSymbol cim:UnitSymbol.V;
  qudt:hasQuantityKind cim:Voltage;
  qudt:hasUnit unit:KiloV .

cim:Switch a owl:Class;
  rdfs:comment "A generic device designed to close, or open, or both, one or more electric circuits.  All switches are two terminal devices including grounding switches. The ACDCTerminal.connected at the two sides of the switch shall not be considered for assessing switch connectivity, i.e. only Switch.open, .normalOpen and .locked are relevant."@en;
  rdfs:subClassOf cim:ConductingEquipment;
  rdfs:label "Switch" .

cim:Switch.SvSwitch a owl:ObjectProperty, owl:InverseFunctionalProperty;
  rdfs:comment "The switch state associated with the switch."@en;
  rdfs:domain cim:Switch;
  rdfs:range cim:SvSwitch;
  rdfs:label "SvSwitch";
  cims:multiplicity cims:M:0..n;
  owl:inverseOf cim:SvSwitch.Switch .

cim:Switch.locked a owl:FunctionalProperty, owl:DatatypeProperty;
  rdfs:comment """If true, the switch is locked. The resulting switch state is a combination of locked and Switch.open attributes as follows:
<ul>
	<li>locked=true and Switch.open=true. The resulting state is open and locked;</li>
	<li>locked=false and Switch.open=true. The resulting state is open;</li>
	<li>locked=false and Switch.open=false. The resulting state is closed.</li>
</ul>"""@en;
  rdfs:domain cim:Switch;
  rdfs:range xsd:boolean;
  rdfs:label "locked";
  cims:multiplicity cims:M:1..1 .

cim:Switch.normalOpen a owl:FunctionalProperty, owl:DatatypeProperty;
  rdfs:comment "The attribute is used in cases when no Measurement for the status value is present. If the Switch has a status measurement the Discrete.normalValue is expected to match with the Switch.normalOpen."@en;
  rdfs:domain cim:Switch;
  rdfs:range xsd:boolean;
  rdfs:label "normalOpen";
  cims:multiplicity cims:M:1..1 .

cim:Switch.open a owl:FunctionalProperty, owl:DatatypeProperty;
  rdfs:comment "The attribute tells if the switch is considered open when used as input to topology processing."@en;
  rdfs:domain cim:Switch;
  rdfs:range xsd:boolean;
  rdfs:label "open";
  cims:multiplicity cims:M:1..1 .

cim:Switch.ratedCurrent a owl:FunctionalProperty, owl:DatatypeProperty;
  rdfs:comment """The maximum continuous current carrying capacity in amps governed by the device material and construction.
The attribute shall be a positive value."""@en;
  rdfs:domain cim:Switch;
  rdfs:range xsd:float;
  rdfs:label "ratedCurrent";
  cims:multiplicity cims:M:0..1;
  cim:unitMultiplier cim:UnitMultiplier.none;
  cim:unitSymbol cim:UnitSymbol.A;
  qudt:hasQuantityKind cim:CurrentFlow;
  qudt:hasUnit unit:A .

cim:Switch.retained a owl:FunctionalProperty, owl:DatatypeProperty;
  rdfs:comment "Branch is retained in the topological solution.  The flow through retained switches will normally be calculated in power flow."@en;
  rdfs:domain cim:Switch;
  rdfs:range xsd:boolean;
  rdfs:label "retained";
  cims:multiplicity cims:M:1..1 .

cim:SwitchInfo a owl:Class;
  rdfs:comment """<was Switch data.>
Switch datasheet information."""@en;
  rdfs:subClassOf cim:AssetInfo;
  rdfs:label "SwitchInfo" .

cim:SwitchInfo.breakingCapacity a owl:ObjectProperty, owl:FunctionalProperty;
  rdfs:comment "The maximum fault current a breaking device can break safely under prescribed conditions of use."@en;
  rdfs:domain cim:SwitchInfo;
  rdfs:label "breakingCapacity";
  cims:multiplicity cims:M:0..1;
  cims:dataType cim:CurrentFlow .

cim:SwitchInfo.isUnganged a owl:ObjectProperty, owl:FunctionalProperty;
  rdfs:comment "If true, the switch is not ganged (i.e., a switch phase may be operated separately from other phases)."@en;
  rdfs:domain cim:SwitchInfo;
  rdfs:label "isUnganged";
  cims:multiplicity cims:M:0..1;
  cims:dataType cim:Boolean .

cim:SwitchInfo.ratedCurrent a owl:ObjectProperty, owl:FunctionalProperty;
  rdfs:comment "Rated current."@en;
  rdfs:domain cim:SwitchInfo;
  rdfs:label "ratedCurrent";
  cims:multiplicity cims:M:0..1;
  cims:dataType cim:CurrentFlow .

cim:SwitchInfo.ratedVoltage a owl:ObjectProperty, owl:FunctionalProperty;
  rdfs:comment "Rated voltage."@en;
  rdfs:domain cim:SwitchInfo;
  rdfs:label "ratedVoltage";
  cims:multiplicity cims:M:0..1;
  cims:dataType cim:Voltage .

cim:SynchronousMachine a owl:Class;
  rdfs:comment "An electromechanical device that operates with shaft rotating synchronously with the network. It is a single machine operating either as a generator or synchronous condenser or pump."@en;
  rdfs:subClassOf cim:RotatingMachine;
  rdfs:label "SynchronousMachine" .

cim:SynchronousMachine.maxQ a owl:FunctionalProperty, owl:DatatypeProperty;
  rdfs:comment "Maximum reactive power limit. This is the maximum (nameplate) limit for the unit."@en;
  rdfs:domain cim:SynchronousMachine;
  rdfs:range xsd:float;
  rdfs:label "maxQ";
  cims:multiplicity cims:M:0..1;
  cim:unitMultiplier cim:UnitMultiplier.M;
  cim:unitSymbol cim:UnitSymbol.VAr;
  qudt:hasQuantityKind cim:ReactivePower;
  qudt:hasUnit unit:MegaV-A_Reactive .

cim:SynchronousMachine.minQ a owl:FunctionalProperty, owl:DatatypeProperty;
  rdfs:comment "Minimum reactive power limit for the unit."@en;
  rdfs:domain cim:SynchronousMachine;
  rdfs:range xsd:float;
  rdfs:label "minQ";
  cims:multiplicity cims:M:0..1;
  cim:unitMultiplier cim:UnitMultiplier.M;
  cim:unitSymbol cim:UnitSymbol.VAr;
  qudt:hasQuantityKind cim:ReactivePower;
  qudt:hasUnit unit:MegaV-A_Reactive .

cim:SynchronousMachine.operatingMode a owl:ObjectProperty, owl:FunctionalProperty;
  rdfs:comment "Current mode of operation."@en;
  rdfs:domain cim:SynchronousMachine;
  rdfs:range cim:SynchronousMachineOperatingMode;
  rdfs:label "operatingMode";
  cims:multiplicity cims:M:1..1 .

cim:SynchronousMachine.qPercent a owl:FunctionalProperty, owl:DatatypeProperty;
  rdfs:comment "Part of the coordinated reactive control that comes from this machine. The attribute is used as a participation factor not necessarily summing up to 100% for the participating devices in the control."@en;
  rdfs:domain cim:SynchronousMachine;
  rdfs:range xsd:float;
  rdfs:label "qPercent";
  cims:multiplicity cims:M:0..1;
  cim:unitMultiplier cim:UnitMultiplier.none;
  cim:unitSymbol cim:UnitSymbol.none;
  qudt:hasQuantityKind cim:PerCent;
  qudt:hasUnit unit:PERCENT .

cim:SynchronousMachine.r a owl:FunctionalProperty, owl:DatatypeProperty;
  rdfs:comment "Equivalent resistance (RG) of generator. RG is considered for the calculation of all currents, except for the calculation of the peak current ip. Used for short circuit data exchange according to IEC 60909."@en;
  rdfs:domain cim:SynchronousMachine;
  rdfs:range xsd:float;
  rdfs:label "r";
  cims:multiplicity cims:M:1..1;
  cim:unitMultiplier cim:UnitMultiplier.none;
  cim:unitSymbol cim:UnitSymbol.ohm;
  qudt:hasQuantityKind cim:Resistance;
  qudt:hasUnit unit:OHM .

cim:SynchronousMachine.referencePriority a owl:FunctionalProperty, owl:DatatypeProperty;
  rdfs:comment "Priority of unit for use as powerflow voltage phase angle reference bus selection. 0 = don t care (default) 1 = highest priority. 2 is less than 1 and so on."@en;
  rdfs:domain cim:SynchronousMachine;
  rdfs:range xsd:integer;
  rdfs:label "referencePriority";
  cims:multiplicity cims:M:1..1 .

cim:SynchronousMachine.type a owl:ObjectProperty, owl:FunctionalProperty;
  rdfs:comment "Modes that this synchronous machine can operate in."@en;
  rdfs:domain cim:SynchronousMachine;
  rdfs:range cim:SynchronousMachineKind;
  rdfs:label "type";
  cims:multiplicity cims:M:1..1 .

cim:SynchronousMachineKind a owl:Class;
  rdfs:comment "Synchronous machine type."@en;
  rdfs:label "SynchronousMachineKind" .

cim:SynchronousMachineKind.generator a cim:SynchronousMachineKind;
  rdfs:comment "Indicates the synchronous machine can operate as a generator."@en;
  rdfs:label "generator" .

cim:SynchronousMachineModelKind a owl:Class;
  rdfs:comment "Type of synchronous machine model used in dynamic simulation applications."@en;
  rdfs:label "SynchronousMachineModelKind" .

cim:SynchronousMachineOperatingMode a owl:Class;
  rdfs:comment "Synchronous machine operating mode."@en;
  rdfs:label "SynchronousMachineOperatingMode" .

cim:SynchronousMachineOperatingMode.generator a cim:SynchronousMachineOperatingMode;
  rdfs:comment "Operating as generator."@en;
  rdfs:label "generator" .

cim:TapChanger a owl:Class;
  rdfs:comment "Mechanism for changing transformer winding tap positions."@en;
  rdfs:subClassOf cim:PowerSystemResource;
  rdfs:label "TapChanger" .

cim:TapChanger.SvTapStep a owl:ObjectProperty, owl:InverseFunctionalProperty, owl:FunctionalProperty;
  rdfs:comment "The tap step state associated with the tap changer."@en;
  rdfs:domain cim:TapChanger;
  rdfs:range cim:SvTapStep;
  rdfs:label "SvTapStep";
  cims:multiplicity cims:M:0..1;
  owl:inverseOf cim:SvTapStep.TapChanger .

cim:TapChanger.TapChangerControl a owl:ObjectProperty, owl:FunctionalProperty;
  rdfs:comment "The regulating control scheme in which this tap changer participates."@en;
  rdfs:domain cim:TapChanger;
  rdfs:range cim:TapChangerControl;
  rdfs:label "TapChangerControl";
  cims:multiplicity cims:M:0..1;
  owl:inverseOf cim:TapChangerControl.TapChanger .

cim:TapChanger.controlEnabled a owl:FunctionalProperty, owl:DatatypeProperty;
  rdfs:comment "Specifies the regulation status of the equipment.  True is regulating, false is not regulating."@en;
  rdfs:domain cim:TapChanger;
  rdfs:range xsd:boolean;
  rdfs:label "controlEnabled";
  cims:multiplicity cims:M:1..1 .

cim:TapChanger.highStep a owl:FunctionalProperty, owl:DatatypeProperty;
  rdfs:comment """Highest possible tap step position, advance from neutral.
The attribute shall be greater than lowStep."""@en;
  rdfs:domain cim:TapChanger;
  rdfs:range xsd:integer;
  rdfs:label "highStep";
  cims:multiplicity cims:M:1..1 .

cim:TapChanger.lowStep a owl:FunctionalProperty, owl:DatatypeProperty;
  rdfs:comment "Lowest possible tap step position, retard from neutral."@en;
  rdfs:domain cim:TapChanger;
  rdfs:range xsd:integer;
  rdfs:label "lowStep";
  cims:multiplicity cims:M:1..1 .

cim:TapChanger.ltcFlag a owl:FunctionalProperty, owl:DatatypeProperty;
  rdfs:comment "Specifies whether or not a TapChanger has load tap changing capabilities."@en;
  rdfs:domain cim:TapChanger;
  rdfs:range xsd:boolean;
  rdfs:label "ltcFlag";
  cims:multiplicity cims:M:1..1 .

cim:TapChanger.neutralStep a owl:FunctionalProperty, owl:DatatypeProperty;
  rdfs:comment """The neutral tap step position for this winding.
The attribute shall be equal to or greater than lowStep and equal or less than highStep.
It is the step position where the voltage is neutralU when the other terminals of the transformer are at the ratedU.  If there are other tap changers on the transformer those taps are kept constant at their neutralStep."""@en;
  rdfs:domain cim:TapChanger;
  rdfs:range xsd:integer;
  rdfs:label "neutralStep";
  cims:multiplicity cims:M:1..1 .

cim:TapChanger.neutralU a owl:FunctionalProperty, owl:DatatypeProperty;
  rdfs:comment "Voltage at which the winding operates at the neutral tap setting. It is the voltage at the terminal of the PowerTransformerEnd associated with the tap changer when all tap changers on the transformer are at their neutralStep position.  Normally neutralU of the tap changer is the same as ratedU of the PowerTransformerEnd, but it can differ in special cases such as when the tapping mechanism is separate from the winding more common on lower voltage transformers. This attribute is not relevant for PhaseTapChangerAsymmetrical,"@en;
  rdfs:domain cim:TapChanger;
  rdfs:range xsd:float;
  rdfs:label "neutralU";
  cims:multiplicity cims:M:1..1;
  cim:unitMultiplier cim:UnitMultiplier.k;
  cim:unitSymbol cim:UnitSymbol.V;
  qudt:hasQuantityKind cim:Voltage;
  qudt:hasUnit unit:KiloV .

cim:TapChanger.normalStep a owl:FunctionalProperty, owl:DatatypeProperty;
  rdfs:comment """The tap step position used in \"normal\" network operation for this winding. For a \"Fixed\" tap changer indicates the current physical tap setting.
The attribute shall be equal to or greater than lowStep and equal to or less than highStep."""@en;
  rdfs:domain cim:TapChanger;
  rdfs:range xsd:integer;
  rdfs:label "normalStep";
  cims:multiplicity cims:M:1..1 .

cim:TapChanger.step a owl:FunctionalProperty, owl:DatatypeProperty;
  rdfs:comment """Tap changer position.
Starting step for a steady state solution. Non integer values are allowed to support continuous tap variables. The reasons for continuous value are to support study cases where no discrete tap changer has yet been designed, a solution where a narrow voltage band forces the tap step to oscillate or to accommodate for a continuous solution as input.
The attribute shall be equal to or greater than lowStep and equal to or less than highStep."""@en;
  rdfs:domain cim:TapChanger;
  rdfs:range xsd:float;
  rdfs:label "step";
  cims:multiplicity cims:M:1..1 .

cim:TapChangerControl a owl:Class;
  rdfs:comment "Describes behaviour specific to tap changers, e.g. how the voltage at the end of a line varies with the load level and compensation of the voltage drop by tap adjustment."@en;
  rdfs:subClassOf cim:RegulatingControl;
  rdfs:label "TapChangerControl" .

cim:TapChangerControl.TapChanger a owl:ObjectProperty, owl:InverseFunctionalProperty;
  rdfs:comment "The tap changers that participates in this regulating tap control scheme."@en;
  rdfs:domain cim:TapChangerControl;
  rdfs:range cim:TapChanger;
  rdfs:label "TapChanger";
  cims:multiplicity cims:M:1..n;
  owl:inverseOf cim:TapChanger.TapChangerControl .

cim:TapChangerInfo a owl:Class;
  rdfs:comment "Tap changer data."@en;
  rdfs:subClassOf cim:AssetInfo;
  rdfs:label "TapChangerInfo" .

cim:Terminal a owl:Class;
  rdfs:comment "An AC electrical connection point to a piece of conducting equipment. Terminals are connected at physical connection points called connectivity nodes."@en;
  rdfs:subClassOf cim:ACDCTerminal;
  rdfs:label "Terminal" .

cim:Terminal.AuxiliaryEquipment a owl:ObjectProperty, owl:InverseFunctionalProperty;
  rdfs:comment "The auxiliary equipment connected to the terminal."@en;
  rdfs:subPropertyOf cimr:Terminal.Equipment;
  rdfs:domain cim:Terminal;
  rdfs:range cim:AuxiliaryEquipment;
  rdfs:label "AuxiliaryEquipment";
  cims:multiplicity cims:M:0..n;
  owl:inverseOf cim:AuxiliaryEquipment.Terminal .

cim:Terminal.ConductingEquipment a owl:ObjectProperty, owl:FunctionalProperty;
  rdfs:comment "The conducting equipment of the terminal.  Conducting equipment have  terminals that may be connected to other conducting equipment terminals via connectivity nodes or topological nodes."@en;
  rdfs:subPropertyOf cimr:Terminal.Equipment;
  rdfs:domain cim:Terminal;
  rdfs:range cim:ConductingEquipment;
  rdfs:label "ConductingEquipment";
  cims:multiplicity cims:M:1..1;
  owl:inverseOf cim:ConductingEquipment.Terminals .

cim:Terminal.ConnectivityNode a owl:ObjectProperty, owl:FunctionalProperty;
  rdfs:comment "The connectivity node to which this terminal connects with zero impedance."@en;
  rdfs:domain cim:Terminal;
  rdfs:range cim:ConnectivityNode;
  rdfs:label "ConnectivityNode";
  cims:multiplicity cims:M:0..1;
  owl:inverseOf cim:ConnectivityNode.Terminals .

cim:Terminal.RegulatingControl a owl:ObjectProperty, owl:InverseFunctionalProperty;
  rdfs:comment "The controls regulating this terminal."@en;
  rdfs:domain cim:Terminal;
  rdfs:range cim:RegulatingControl;
  rdfs:label "RegulatingControl";
  cims:multiplicity cims:M:0..n;
  owl:inverseOf cim:RegulatingControl.Terminal .

cim:Terminal.SvPowerFlow a owl:ObjectProperty, owl:InverseFunctionalProperty, owl:FunctionalProperty;
  rdfs:comment "The power flow state variable associated with the terminal."@en;
  rdfs:domain cim:Terminal;
  rdfs:range cim:SvPowerFlow;
  rdfs:label "SvPowerFlow";
  cims:multiplicity cims:M:0..1;
  owl:inverseOf cim:SvPowerFlow.Terminal .

cim:Terminal.TopologicalNode a owl:ObjectProperty, owl:FunctionalProperty;
  rdfs:comment "The topological node associated with the terminal.   This can be used as an alternative to the connectivity node path to topological node, thus making it unnecessary to model connectivity nodes in some cases.   Note that the if connectivity nodes are in the model, this association would probably not be used as an input specification."@en;
  rdfs:domain cim:Terminal;
  rdfs:range cim:TopologicalNode;
  rdfs:label "TopologicalNode";
  cims:multiplicity cims:M:0..1;
  owl:inverseOf cim:TopologicalNode.Terminal .

cim:Terminal.TransformerEnd a owl:ObjectProperty, owl:InverseFunctionalProperty;
  rdfs:comment "All transformer ends connected at this terminal."@en;
  rdfs:domain cim:Terminal;
  rdfs:range cim:TransformerEnd;
  rdfs:label "TransformerEnd";
  cims:multiplicity cims:M:0..n;
  owl:inverseOf cim:TransformerEnd.Terminal .

cim:Terminal.phases a owl:ObjectProperty, owl:FunctionalProperty;
  rdfs:comment "Represents the normal network phasing condition. If the attribute is missing, three phases (ABC) shall be assumed, except for terminals of grounding classes (specializations of EarthFaultCompensator, GroundDisconnector, and Ground) which will be assumed to be N. Therefore, phase code ABCN is explicitly declared when needed, e.g. for star point grounding equipment. The phase code on terminals connecting same ConnectivityNode or same TopologicalNode as well as for equipment between two terminals shall"@en;
  rdfs:domain cim:Terminal;
  rdfs:range cim:PhaseCode;
  rdfs:label "phases";
  cims:multiplicity cims:M:0..1 .

cim:TextDiagramObject a owl:Class;
  rdfs:comment "A diagram object for placing free-text or text derived from an associated domain object."@en;
  rdfs:subClassOf cim:DiagramObject;
  rdfs:label "TextDiagramObject" .

cim:TextDiagramObject.text a owl:FunctionalProperty, owl:DatatypeProperty;
  rdfs:comment "The text that is displayed by this text diagram object."@en;
  rdfs:domain cim:TextDiagramObject;
  rdfs:range xsd:string;
  rdfs:label "text";
  cims:multiplicity cims:M:1..1 .

cim:TopologicalIsland a owl:Class;
  rdfs:comment """An electrically connected subset of the network. Topological islands can change as the current network state changes, e.g. due to: 
- disconnect switches or breakers changing state in a SCADA/EMS.
- manual creation, change or deletion of topological nodes in a planning tool.
Only energised TopologicalNode-s shall be part of the topological island."""@en;
  rdfs:subClassOf cim:IdentifiedObject;
  rdfs:label "TopologicalIsland" .

cim:TopologicalIsland.AngleRefTopologicalNode a owl:ObjectProperty, owl:InverseFunctionalProperty,
    owl:FunctionalProperty;
  rdfs:comment "The angle reference for the island.   Normally there is one TopologicalNode that is selected as the angle reference for each island.   Other reference schemes exist, so the association is typically optional."@en;
  rdfs:domain cim:TopologicalIsland;
  rdfs:range cim:TopologicalNode;
  rdfs:label "AngleRefTopologicalNode";
  cims:multiplicity cims:M:1..1;
  owl:inverseOf cim:TopologicalNode.AngleRefTopologicalIsland .

cim:TopologicalIsland.TopologicalNodes a owl:ObjectProperty, owl:InverseFunctionalProperty;
  rdfs:comment "A topological node belongs to a topological island."@en;
  rdfs:domain cim:TopologicalIsland;
  rdfs:range cim:TopologicalNode;
  rdfs:label "TopologicalNodes";
  cims:multiplicity cims:M:1..n;
  owl:inverseOf cim:TopologicalNode.TopologicalIsland .

cim:TopologicalNode a owl:Class;
  rdfs:comment "For a detailed substation model a topological node is a set of connectivity nodes that, in the current network state, are connected together through any type of closed switches, including  jumpers. Topological nodes change as the current network state changes (i.e., switches, breakers, etc. change state). For a planning model, switch statuses are not used to form topological nodes. Instead they are manually created or deleted in a model builder tool. Topological nodes maintained this way are also"@en;
  rdfs:subClassOf cim:IdentifiedObject;
  rdfs:label "TopologicalNode" .

cim:TopologicalNode.AngleRefTopologicalIsland a owl:ObjectProperty, owl:InverseFunctionalProperty,
    owl:FunctionalProperty;
  rdfs:comment "The island for which the node is an angle reference.   Normally there is one angle reference node for each island."@en;
  rdfs:domain cim:TopologicalNode;
  rdfs:range cim:TopologicalIsland;
  rdfs:label "AngleRefTopologicalIsland";
  cims:multiplicity cims:M:0..1;
  owl:inverseOf cim:TopologicalIsland.AngleRefTopologicalNode .

cim:TopologicalNode.BaseVoltage a owl:ObjectProperty, owl:FunctionalProperty;
  rdfs:comment "The base voltage of the topological node."@en;
  rdfs:domain cim:TopologicalNode;
  rdfs:range cim:BaseVoltage;
  rdfs:label "BaseVoltage";
  cims:multiplicity cims:M:1..1;
  owl:inverseOf cim:BaseVoltage.TopologicalNode .

cim:TopologicalNode.ConnectivityNodeContainer a owl:ObjectProperty, owl:FunctionalProperty;
  rdfs:comment "The connectivity node container to which the topological node belongs."@en;
  rdfs:domain cim:TopologicalNode;
  rdfs:range cim:ConnectivityNodeContainer;
  rdfs:label "ConnectivityNodeContainer";
  cims:multiplicity cims:M:1..1;
  owl:inverseOf cim:ConnectivityNodeContainer.TopologicalNode .

cim:TopologicalNode.ConnectivityNodes a owl:ObjectProperty, owl:InverseFunctionalProperty;
  rdfs:comment "The connectivity nodes combine together to form this topological node.  May depend on the current state of switches in the network."@en;
  rdfs:domain cim:TopologicalNode;
  rdfs:range cim:ConnectivityNode;
  rdfs:label "ConnectivityNodes";
  cims:multiplicity cims:M:0..n;
  owl:inverseOf cim:ConnectivityNode.TopologicalNode .

cim:TopologicalNode.SvVoltage a owl:ObjectProperty, owl:InverseFunctionalProperty,
    owl:FunctionalProperty;
  rdfs:comment "The state voltage associated with the topological node."@en;
  rdfs:domain cim:TopologicalNode;
  rdfs:range cim:SvVoltage;
  rdfs:label "SvVoltage";
  cims:multiplicity cims:M:0..1;
  owl:inverseOf cim:SvVoltage.TopologicalNode .

cim:TopologicalNode.Terminal a owl:ObjectProperty, owl:InverseFunctionalProperty;
  rdfs:comment "The terminals associated with the topological node.   This can be used as an alternative to the connectivity node path to terminal, thus making it unnecessary to model connectivity nodes in some cases.   Note that if connectivity nodes are in the model, this association would probably not be used as an input specification."@en;
  rdfs:domain cim:TopologicalNode;
  rdfs:range cim:Terminal;
  rdfs:label "Terminal";
  cims:multiplicity cims:M:1..n;
  owl:inverseOf cim:Terminal.TopologicalNode .

cim:TopologicalNode.TopologicalIsland a owl:ObjectProperty, owl:FunctionalProperty;
  rdfs:comment "A topological node belongs to a topological island."@en;
  rdfs:domain cim:TopologicalNode;
  rdfs:range cim:TopologicalIsland;
  rdfs:label "TopologicalIsland";
  cims:multiplicity cims:M:0..1;
  owl:inverseOf cim:TopologicalIsland.TopologicalNodes .

cim:TransformerEnd a owl:Class;
  rdfs:comment "A conducting connection point of a power transformer. It corresponds to a physical transformer winding terminal.  In earlier CIM versions, the TransformerWinding class served a similar purpose, but this class is more flexible because it associates to terminal but is not a specialization of ConductingEquipment."@en;
  rdfs:subClassOf cim:IdentifiedObject;
  rdfs:label "TransformerEnd" .

cim:TransformerEnd.BaseVoltage a owl:ObjectProperty, owl:FunctionalProperty;
  rdfs:comment "Base voltage of the transformer end.  This is essential for PU calculation."@en;
  rdfs:domain cim:TransformerEnd;
  rdfs:range cim:BaseVoltage;
  rdfs:label "BaseVoltage";
  cims:multiplicity cims:M:1..1;
  owl:inverseOf cim:BaseVoltage.TransformerEnds .

cim:TransformerEnd.RatioTapChanger a owl:ObjectProperty, owl:InverseFunctionalProperty,
    owl:FunctionalProperty;
  rdfs:comment "Ratio tap changer associated with this transformer end."@en;
  rdfs:domain cim:TransformerEnd;
  rdfs:range cim:RatioTapChanger;
  rdfs:label "RatioTapChanger";
  cims:multiplicity cims:M:0..1;
  owl:inverseOf cim:RatioTapChanger.TransformerEnd .

cim:TransformerEnd.Terminal a owl:ObjectProperty, owl:FunctionalProperty;
  rdfs:comment "Terminal of the power transformer to which this transformer end belongs."@en;
  rdfs:domain cim:TransformerEnd;
  rdfs:range cim:Terminal;
  rdfs:label "Terminal";
  cims:multiplicity cims:M:1..1;
  owl:inverseOf cim:Terminal.TransformerEnd .

cim:TransformerEnd.endNumber a owl:FunctionalProperty, owl:DatatypeProperty;
  rdfs:comment "Number for this transformer end, corresponding to the end's order in the power transformer vector group or phase angle clock number.  Highest voltage winding should be 1.  Each end within a power transformer should have a unique subsequent end number.   Note the transformer end number need not match the terminal sequence number."@en;
  rdfs:domain cim:TransformerEnd;
  rdfs:range xsd:integer;
  rdfs:label "endNumber";
  cims:multiplicity cims:M:1..1 .

cim:TransformerEnd.grounded a owl:FunctionalProperty, owl:DatatypeProperty;
  rdfs:comment "(for Yn and Zn connections) True if the neutral is solidly grounded."@en;
  rdfs:domain cim:TransformerEnd;
  rdfs:range xsd:boolean;
  rdfs:label "grounded";
  cims:multiplicity cims:M:1..1 .

cim:TransformerEndInfo a owl:Class;
  rdfs:comment "Transformer end data."@en;
  rdfs:subClassOf cim:AssetInfo;
  rdfs:label "TransformerEndInfo" .

cim:TransformerEndInfo.TransformerTankInfo a owl:ObjectProperty, owl:FunctionalProperty;
  rdfs:comment "Transformer tank data that this end description is part of."@en;
  rdfs:domain cim:TransformerEndInfo;
  rdfs:range cim:TransformerTankInfo;
  rdfs:label "TransformerTankInfo";
  cims:multiplicity cims:M:1..1;
  owl:inverseOf cim:TransformerTankInfo.TransformerEndInfos .

cim:TransformerEndInfo.ratedS a owl:ObjectProperty, owl:FunctionalProperty;
  rdfs:comment "Normal apparent power rating."@en;
  rdfs:domain cim:TransformerEndInfo;
  rdfs:label "ratedS";
  cims:multiplicity cims:M:0..1;
  cims:dataType cim:ApparentPower .

cim:TransformerEndInfo.ratedU a owl:ObjectProperty, owl:FunctionalProperty;
  rdfs:comment "Rated voltage: phase-phase for three-phase windings, and either phase-phase or phase-neutral for single-phase windings."@en;
  rdfs:domain cim:TransformerEndInfo;
  rdfs:label "ratedU";
  cims:multiplicity cims:M:0..1;
  cims:dataType cim:Voltage .

cim:TransformerTankInfo a owl:Class;
  rdfs:comment "Set of transformer tank data, from an equipment library."@en;
  rdfs:subClassOf cim:AssetInfo;
  rdfs:label "TransformerTankInfo" .

cim:TransformerTankInfo.TransformerEndInfos a owl:ObjectProperty, owl:InverseFunctionalProperty;
  rdfs:comment "Data for all the ends described by this transformer tank data."@en;
  rdfs:domain cim:TransformerTankInfo;
  rdfs:range cim:TransformerEndInfo;
  rdfs:label "TransformerEndInfos";
  cims:multiplicity cims:M:1..n;
  owl:inverseOf cim:TransformerEndInfo.TransformerTankInfo .

cim:UnitMultiplier a owl:Class;
  rdfs:comment "The unit multipliers defined for the CIM.  When applied to unit symbols, the unit symbol is treated as a derived unit. Regardless of the contents of the unit symbol text, the unit symbol shall be treated as if it were a single-character unit symbol. Unit symbols should not contain multipliers, and it should be left to the multiplier to define the multiple for an entire data type.   For example, if a unit symbol is \"m2Pers\" and the multiplier is \"k\", then the value is k(m**2/s), and the multiplier"@en;
  rdfs:label "UnitMultiplier" .

cim:UnitMultiplier.M a cim:UnitMultiplier;
  rdfs:comment "Mega 10**6."@en;
  rdfs:label "M";
  skos:exactMatch prefix:Mega;
  qudt:prefixMultiplier 1.0E6 .

cim:UnitMultiplier.k a cim:UnitMultiplier;
  rdfs:comment "Kilo 10**3."@en;
  rdfs:label "k";
  skos:exactMatch prefix:Kilo;
  qudt:prefixMultiplier 1.0E3 .

cim:UnitMultiplier.none a cim:UnitMultiplier;
  rdfs:comment "No multiplier or equivalently multiply by 1."@en;
  rdfs:label "none";
  qudt:prefixMultiplier 1.0E0 .

cim:UnitSymbol a owl:Class;
  rdfs:comment "The derived units defined for usage in the CIM. In some cases, the derived unit is equal to an SI unit. Whenever possible, the standard derived symbol is used instead of the formula for the derived unit. For example, the unit symbol Farad is defined as \"F\" instead of \"CPerV\". In cases where a standard symbol does not exist for a derived unit, the formula for the unit is used as the unit symbol. For example, density does not have a standard symbol and so it is represented as \"kgPerm3\". With the exception"@en;
  rdfs:label "UnitSymbol" .

cim:UnitSymbol.A a cim:UnitSymbol;
  rdfs:comment "Current in amperes."@en;
  rdfs:label "A";
  skos:exactMatch unit:A .

cim:UnitSymbol.DKKperEUR skos:exactMatch unit:CCY_DKK-PER-CCY_EUR .

cim:UnitSymbol.EURperMWh skos:exactMatch unit:CCY_EUR-PER-MegaW-HR .

cim:UnitSymbol.NOKperEUR skos:exactMatch unit:CCY_NOK-PER-CCY_EUR .

cim:UnitSymbol.NOKperMWh skos:exactMatch unit:CCY_NOK-PER-MegaW-HR .

cim:UnitSymbol.SEKperEUR skos:exactMatch unit:CCY_SEK-PER-CCY_EUR .

cim:UnitSymbol.V a cim:UnitSymbol;
  rdfs:comment "Electric potential in volts (W/A)."@en;
  rdfs:label "V";
  skos:exactMatch unit:V .

cim:UnitSymbol.W a cim:UnitSymbol;
  rdfs:comment "Real power in watts (J/s). Electrical power may have real and reactive components. The real portion of electrical power (I&#178;R or VIcos(phi)), is expressed in Watts. See also apparent power and reactive power."@en;
  rdfs:label "W";
  skos:exactMatch unit:W .

cim:UnitSymbol.degC a cim:UnitSymbol;
  rdfs:comment """Relative temperature in degrees Celsius.
In the SI unit system the symbol is °C. Electric charge is measured in coulomb that has the unit symbol C. To distinguish degree Celsius from coulomb the symbol used in the UML is degC. The reason for not using °C is that the special character ° is difficult to manage in software."""@en;
  rdfs:label "degC";
  skos:exactMatch unit:DEG_C .

cim:UnitSymbol.none a cim:UnitSymbol;
  rdfs:comment "Dimension less quantity, e.g. count, per unit, etc."@en;
  rdfs:label "none" .

cim:UsagePoint a owl:Class;
  rdfs:comment "Logical or physical point in the network to which readings or events may be attributed. Used at the place where a physical or virtual meter may be located; however, it is not required that a meter be present."@en;
  rdfs:subClassOf cim:IdentifiedObject;
  rdfs:label "UsagePoint" .

cim:Validity a owl:Class;
  rdfs:comment "Validity for MeasurementValue."@en;
  rdfs:label "Validity" .

cim:VoltageLevel a owl:Class;
  rdfs:comment "A collection of equipment at one common system voltage forming a switchgear. The equipment typically consists of breakers, busbars, instrumentation, control, regulation and protection devices as well as assemblies of all these."@en;
  rdfs:subClassOf cim:EquipmentContainer;
  rdfs:label "VoltageLevel" .

cim:VoltageLevel.BaseVoltage a owl:ObjectProperty, owl:FunctionalProperty;
  rdfs:comment "The base voltage used for all equipment within the voltage level."@en;
  rdfs:domain cim:VoltageLevel;
  rdfs:range cim:BaseVoltage;
  rdfs:label "BaseVoltage";
  cims:multiplicity cims:M:1..1;
  owl:inverseOf cim:BaseVoltage.VoltageLevel .

cim:VoltageLevel.Bays a owl:ObjectProperty, owl:InverseFunctionalProperty;
  rdfs:comment "The bays within this voltage level."@en;
  rdfs:subPropertyOf cimr:hasPart;
  rdfs:domain cim:VoltageLevel;
  rdfs:range cim:Bay;
  rdfs:label "Bays";
  cims:multiplicity cims:M:0..n;
  owl:inverseOf cim:Bay.VoltageLevel .

cim:VoltageLevel.Substation a owl:ObjectProperty, owl:FunctionalProperty;
  rdfs:comment "The substation of the voltage level."@en;
  rdfs:domain cim:VoltageLevel;
  rdfs:range cim:Substation;
  rdfs:label "Substation";
  cims:multiplicity cims:M:1..1;
  owl:inverseOf cim:Substation.VoltageLevels .

cim:VoltageLimit a owl:Class;
  rdfs:comment """Operational limit applied to voltage.
The use of operational VoltageLimit is preferred instead of limits defined at VoltageLevel. The operational VoltageLimits are used, if present."""@en;
  rdfs:subClassOf cim:OperationalLimit;
  rdfs:label "VoltageLimit" .

cim:VoltageLimit.normalValue a owl:FunctionalProperty, owl:DatatypeProperty;
  rdfs:comment "The normal limit on voltage. High or low limit nature of the limit depends upon the properties of the operational limit type. The attribute shall be a positive value or zero."@en;
  rdfs:domain cim:VoltageLimit;
  rdfs:range xsd:float;
  rdfs:label "normalValue";
  cims:multiplicity cims:M:1..1;
  cim:unitMultiplier cim:UnitMultiplier.k;
  cim:unitSymbol cim:UnitSymbol.V;
  qudt:hasQuantityKind cim:Voltage;
  qudt:hasUnit unit:KiloV .

cim:VoltageLimit.value a owl:FunctionalProperty, owl:DatatypeProperty;
  rdfs:comment "Limit on voltage. High or low limit nature of the limit depends upon the properties of the operational limit type. The attribute shall be a positive value or zero."@en;
  rdfs:domain cim:VoltageLimit;
  rdfs:range xsd:float;
  rdfs:label "value";
  cims:multiplicity cims:M:1..1;
  cim:unitMultiplier cim:UnitMultiplier.k;
  cim:unitSymbol cim:UnitSymbol.V;
  qudt:hasQuantityKind cim:Voltage;
  qudt:hasUnit unit:KiloV .

cim:VsPpccControlKind a owl:Class;
  rdfs:comment "Types applicable to the control of real power and/or DC voltage by voltage source converter."@en;
  rdfs:label "VsPpccControlKind" .

cim:VsQpccControlKind a owl:Class;
  rdfs:comment "Kind of reactive power control at point of common coupling for a voltage source converter."@en;
  rdfs:label "VsQpccControlKind" .

cim:WindGenUnitKind a owl:Class;
  rdfs:comment "Kind of wind generating unit."@en;
  rdfs:label "WindGenUnitKind" .

cim:WindLookupTableFunctionKind a owl:Class;
  rdfs:comment "Function of the lookup table."@en;
  rdfs:label "WindLookupTableFunctionKind" .

cim:WindPlantQcontrolModeKind a owl:Class;
  rdfs:comment "Reactive power/voltage controller mode."@en;
  rdfs:label "WindPlantQcontrolModeKind" .

cim:WindQcontrolModeKind a owl:Class;
  rdfs:comment "General wind turbine Q control modes <i>M</i><i><sub>qG</sub></i><i>.</i>"@en;
  rdfs:label "WindQcontrolModeKind" .

cim:WindUVRTQcontrolModeKind a owl:Class;
  rdfs:comment "UVRT Q control modes <i>M</i><i><sub>qUVRT</sub></i><i>.</i>"@en;
  rdfs:label "WindUVRTQcontrolModeKind" .

cim:WindingConnection a owl:Class;
  rdfs:comment "Winding connection type."@en;
  rdfs:label "WindingConnection" .

cim:WindingConnection.Y a cim:WindingConnection;
  rdfs:comment "Wye."@en;
  rdfs:label "Y" .

cim:WindingConnection.Zn a cim:WindingConnection;
  rdfs:comment "ZigZag, with neutral brought out for grounding."@en;
  rdfs:label "Zn" .

cim:WireInfo a owl:Class;
  rdfs:comment "Wire data that can be specified per line segment phase, or for the line segment as a whole in case its phases all have the same wire characteristics."@en;
  rdfs:subClassOf cim:AssetInfo;
  rdfs:label "WireInfo" .

cim:WireInfo.gmr a owl:ObjectProperty, owl:FunctionalProperty;
  rdfs:comment "Geometric mean radius. If we replace the conductor by a thin walled tube of radius GMR, then its reactance is identical to the reactance of the actual conductor."@en;
  rdfs:domain cim:WireInfo;
  rdfs:label "gmr";
  cims:multiplicity cims:M:0..1;
  cims:dataType cim:Length .

cim:WireInfo.insulated a owl:ObjectProperty, owl:FunctionalProperty;
  rdfs:comment "True if conductor is insulated."@en;
  rdfs:domain cim:WireInfo;
  rdfs:label "insulated";
  cims:multiplicity cims:M:0..1;
  cims:dataType cim:Boolean .

cim:WireInfo.insulationMaterial a owl:ObjectProperty, owl:FunctionalProperty;
  rdfs:comment "(if insulated conductor) Material used for insulation."@en;
  rdfs:domain cim:WireInfo;
  rdfs:range cim:WireInsulationKind;
  rdfs:label "insulationMaterial";
  cims:multiplicity cims:M:0..1 .

cim:WireInfo.rAC25 a owl:ObjectProperty, owl:FunctionalProperty;
  rdfs:comment "AC resistance per unit length of the conductor at 25 °C."@en;
  rdfs:domain cim:WireInfo;
  rdfs:label "rAC25";
  cims:multiplicity cims:M:0..1;
  cims:dataType cim:ResistancePerLength .

cim:WireInfo.rAC75 a owl:ObjectProperty, owl:FunctionalProperty;
  rdfs:comment "AC resistance per unit length of the conductor at 75 °C."@en;
  rdfs:domain cim:WireInfo;
  rdfs:label "rAC75";
  cims:multiplicity cims:M:0..1;
  cims:dataType cim:ResistancePerLength .

cim:WireInfo.radius a owl:ObjectProperty, owl:FunctionalProperty;
  rdfs:comment "Outside radius of the wire."@en;
  rdfs:domain cim:WireInfo;
  rdfs:label "radius";
  cims:multiplicity cims:M:0..1;
  cims:dataType cim:Length .

cim:WireInfo.ratedCurrent a owl:ObjectProperty, owl:FunctionalProperty;
  rdfs:comment "Current carrying capacity of the wire under stated thermal conditions."@en;
  rdfs:domain cim:WireInfo;
  rdfs:label "ratedCurrent";
  cims:multiplicity cims:M:0..1;
  cims:dataType cim:CurrentFlow .

cim:WireInsulationKind a owl:Class;
  rdfs:comment "Kind of wire insulation."@en;
  rdfs:label "WireInsulationKind" .

cim:WireInsulationKind.other a cim:WireInsulationKind;
  rdfs:comment "Other kind of wire insulation."@en;
  rdfs:label "other" .

cim:WireInsulationKind.treeRetardantCrosslinkedPolyethylene a cim:WireInsulationKind;
  rdfs:comment "Tree retardant crosslinked polyethylene wire insulation."@en;
  rdfs:label "treeRetardantCrosslinkedPolyethylene" .

cim:WireUsageKind a owl:Class;
  rdfs:comment "Kind of wire usage."@en;
  rdfs:label "WireUsageKind" .

eu:BoundaryPoint a owl:Class;
  rdfs:comment "Designates a connection point at which one or more model authority sets shall connect to. The location of the connection point as well as other properties are agreed between organisations responsible for the interconnection, hence all attributes of the class represent this agreement.  It is primarily used in a boundary model authority set which can contain one or many BoundaryPoint-s among other Equipment-s and their connections."@en;
  rdfs:subClassOf cim:PowerSystemResource;
  rdfs:label "BoundaryPoint" .

eu:BoundaryPoint.ConnectivityNode a owl:ObjectProperty, owl:InverseFunctionalProperty,
    owl:FunctionalProperty;
  rdfs:comment "The connectivity node that is designated as a boundary point."@en;
  rdfs:domain eu:BoundaryPoint;
  rdfs:range cim:ConnectivityNode;
  rdfs:label "ConnectivityNode";
  cims:multiplicity cims:M:1..1;
  owl:inverseOf eu:ConnectivityNode.BoundaryPoint .

eu:BoundaryPoint.fromEndIsoCode a owl:FunctionalProperty, owl:DatatypeProperty;
  rdfs:comment """The ISO code of the region which the \"From\" side of the Boundary point belongs to or it is connected to.
The ISO code is a two-character country code as defined by ISO 3166 (http://www.iso.org/iso/country_codes). The length of the string is 2 characters maximum."""@en;
  rdfs:domain eu:BoundaryPoint;
  rdfs:range xsd:string;
  rdfs:label "fromEndIsoCode";
  cims:multiplicity cims:M:1..1 .

eu:BoundaryPoint.fromEndName a owl:FunctionalProperty, owl:DatatypeProperty;
  rdfs:comment """A human readable name with length of the string 64 characters maximum. It covers the following two cases:
-if the Boundary point is placed on a tie-line, it is the name (IdentifiedObject.name) of the substation at which the \"From\" side of the tie-line is connected to.
-if the Boundary point is placed in a substation, it is the name (IdentifiedObject.name) of the element (e.g. PowerTransformer, ACLineSegment, Switch, etc.) at which the \"From\" side of the Boundary point is connected to."""@en;
  rdfs:domain eu:BoundaryPoint;
  rdfs:range xsd:string;
  rdfs:label "fromEndName";
  cims:multiplicity cims:M:1..1 .

eu:BoundaryPoint.fromEndNameTso a owl:FunctionalProperty, owl:DatatypeProperty;
  rdfs:comment "Identifies the name of the transmission system operator, distribution system operator or other entity at which the \"From\" side of the interconnection is connected to. The length of the string is 64 characters maximum."@en;
  rdfs:domain eu:BoundaryPoint;
  rdfs:range xsd:string;
  rdfs:label "fromEndNameTso";
  cims:multiplicity cims:M:1..1 .

eu:BoundaryPoint.toEndIsoCode a owl:FunctionalProperty, owl:DatatypeProperty;
  rdfs:comment """The ISO code of the region which the \"To\" side of the Boundary point belongs to or is connected to.
The ISO code is a two-character country code as defined by ISO 3166 (http://www.iso.org/iso/country_codes). The length of the string is 2 characters maximum."""@en;
  rdfs:domain eu:BoundaryPoint;
  rdfs:range xsd:string;
  rdfs:label "toEndIsoCode";
  cims:multiplicity cims:M:1..1 .

eu:BoundaryPoint.toEndName a owl:FunctionalProperty, owl:DatatypeProperty;
  rdfs:comment """A human readable name with length of the string 64 characters maximum. It covers the following two cases:
-if the Boundary point is placed on a tie-line, it is the name (IdentifiedObject.name) of the substation at which the \"To\" side of the tie-line is connected to.
-if the Boundary point is placed in a substation, it is the name (IdentifiedObject.name) of the element (e.g. PowerTransformer, ACLineSegment, Switch, etc.) at which the \"To\" side of the Boundary point is connected to."""@en;
  rdfs:domain eu:BoundaryPoint;
  rdfs:range xsd:string;
  rdfs:label "toEndName";
  cims:multiplicity cims:M:1..1 .

eu:BoundaryPoint.toEndNameTso a owl:FunctionalProperty, owl:DatatypeProperty;
  rdfs:comment "Identifies the name of the transmission system operator, distribution system operator or other entity at which the \"To\" side of the interconnection is connected to. The length of the string is 64 characters maximum."@en;
  rdfs:domain eu:BoundaryPoint;
  rdfs:range xsd:string;
  rdfs:label "toEndNameTso";
  cims:multiplicity cims:M:1..1 .

eu:ConnectivityNode.BoundaryPoint a owl:ObjectProperty, owl:InverseFunctionalProperty,
    owl:FunctionalProperty;
  rdfs:comment "The boundary point associated with the connectivity node."@en;
  rdfs:domain cim:ConnectivityNode;
  rdfs:range eu:BoundaryPoint;
  rdfs:label "BoundaryPoint";
  cims:multiplicity cims:M:0..1;
  owl:inverseOf eu:BoundaryPoint.ConnectivityNode .

eu:IdentifiedObject.energyIdentCodeEic a owl:FunctionalProperty, owl:DatatypeProperty;
  rdfs:comment "The attribute is used for an exchange of the EIC code (Energy identification Code). The length of the string is 16 characters as defined by the EIC code. For details on EIC scheme please refer to ENTSO-E web site."@en;
  rdfs:domain cim:IdentifiedObject;
  rdfs:range xsd:string;
  rdfs:label "energyIdentCodeEic";
  cims:multiplicity cims:M:0..1;
  owl:deprecated true .

eu:LimitKind a owl:Class;
  rdfs:comment "Limit kinds."@en;
  rdfs:label "LimitKind" .

eu:LimitKind.highVoltage a eu:LimitKind;
  rdfs:comment """Referring to the rating of the equipments, a voltage too high can lead to accelerated ageing or the destruction of the equipment. 
This limit type may or may not have duration."""@en;
  rdfs:label "highVoltage" .

eu:LimitKind.lowVoltage a eu:LimitKind;
  rdfs:comment """A too low voltage can disturb the normal operation of some protections and transformer equipped with on-load tap changers, electronic power devices or can affect the behaviour of the auxiliaries of generation units.
This limit type may or may not have duration."""@en;
  rdfs:label "lowVoltage" .

eu:LimitKind.patl a eu:LimitKind;
  rdfs:comment """The Permanent Admissible Transmission Loading (PATL) is the loading in amperes, MVA or MW that can be accepted by a network branch for an unlimited duration without any risk for the material.
The OperationnalLimitType.isInfiniteDuration is set to true. There shall be only one OperationalLimitType of kind PATL per OperationalLimitSet if the PATL is ApparentPowerLimit, ActivePowerLimit, or CurrentLimit for a given Terminal or Equipment."""@en;
  rdfs:label "patl" .

eu:LimitKind.stability a eu:LimitKind;
  rdfs:comment "Stability."@en;
  rdfs:label "stability" .

eu:LimitKind.tatl a eu:LimitKind;
  rdfs:comment """Temporarily Admissible Transmission Loading (TATL) which is the loading in amperes, MVA or MW that can be accepted by a branch for a certain limited duration. The TATL can be defined in different ways: <ul> 	<li>as a fixed percentage of the PATL for a given time (for example, 115% of the PATL that can be accepted during 15 minutes),</li> </ul> <ul> 	<li>pairs of TATL type and Duration calculated for each line taking into account its particular configuration and conditions of functioning (for example,"""@en;
  rdfs:label "tatl" .

eu:OperationalLimitType.kind a owl:ObjectProperty, owl:FunctionalProperty;
  rdfs:comment "Types of limits defined in the ENTSO-E Operational Handbook Policy 3."@en;
  rdfs:domain cim:OperationalLimitType;
  rdfs:range eu:LimitKind;
  rdfs:label "kind";
  cims:multiplicity cims:M:1..1 .

cimr:Equipment.Terminals a owl:ObjectProperty;
  rdfs:comment "Terminals of the equipment";
  rdfs:domain cim:Equipment;
  rdfs:range cim:Terminal;
  rdfs:label "terminals";
  owl:inverseOf cimr:Terminal.Equipment .

cimr:EquipmentOrContainer a owl:Class;
  rdfs:comment "Union (superclass) of Equipment and ConnectivityNodeContainer";
  rdfs:subClassOf cim:PowerSystemResource;
  rdfs:label "Equipment or Container" .

cimr:Measurement.isInCognite a owl:DatatypeProperty;
  rdfs:comment "Flag indicating if a cim:Analog measurement represents to a Cognite timeseries";
  rdfs:domain cim:Analog;
  rdfs:range xsd:boolean;
  rdfs:label "Measurement is in Cognite";
  cims:pragmatics "Use the mRID of this measurement to query a timeseries in the Cognite API by \"external_id\" " .

cimr:Terminal.Equipment a owl:ObjectProperty;
  rdfs:comment "The equipment of the terminal. Disjunction of the props listed in skos:example";
  rdfs:domain cim:Terminal;
  rdfs:range cim:Equipment;
  rdfs:label "equipment";
  owl:inverseOf cimr:Equipment.Terminals;
  skos:example cim:Terminal.ConductingEquipment, cim:Terminal.AuxiliaryEquipment .

cimr:connectedThroughPart a owl:SymmetricProperty, owl:ObjectProperty;
  rdfs:comment "Equipment or EquipmentContainer is connected to Equipment or EquipmentContainer through some of its transitive parts, and their terminals and a common ConnectivityNode";
  rdfs:domain cimr:EquipmentOrContainer;
  rdfs:range cimr:EquipmentOrContainer;
  rdfs:label "connected through part" .

cimr:connectedTo a owl:SymmetricProperty, owl:ObjectProperty;
  rdfs:comment "Equipment is connected to Equipment through some of their terminals and a common ConnectivityNode";
  rdfs:domain cim:Equipment;
  rdfs:range cim:Equipment;
  rdfs:label "connected to" .

cimr:hasPart a owl:ObjectProperty;
  rdfs:comment "Equipment or Container has part. Disjunction of the props listed in skos:example";
  rdfs:subPropertyOf cimr:hasPartTransitive;
  rdfs:domain cimr:EquipmentOrContainer;
  rdfs:range cimr:EquipmentOrContainer;
  rdfs:label "has part";
  owl:inverseOf cimr:isPart;
  skos:example cim:VoltageLevel.Bays, cim:EquipmentContainer.Equipments, cim:Substation.VoltageLevels .

cimr:hasPartTransitive a owl:ObjectProperty;
  rdfs:comment "EquipmentContainer and its subcontainers have part Equipment. Transitive closure of cimr:hasPart";
  rdfs:domain cimr:EquipmentOrContainer;
  rdfs:range cimr:EquipmentOrContainer;
  rdfs:label "has part transitive";
  owl:inverseOf cimr:isPartTransitive;
  psys:transitiveOver cimr:hasPart .

cimr:isPart a owl:ObjectProperty;
  rdfs:comment "Equipment is part of EquipmentContainer. Disjunction of the props listed in skos:example";
  rdfs:domain cimr:EquipmentOrContainer;
  rdfs:range cimr:EquipmentOrContainer;
  rdfs:label "is part";
  owl:inverseOf cimr:hasPart;
  skos:example cim:Bay.VoltageLevel, cim:Equipment.EquipmentContainer, cim:VoltageLevel.Substation .

cimr:isPartTransitive a owl:ObjectProperty;
  rdfs:comment "Equipment is part of EquipmentContainer and its super-containers. Transitive closure of cimr:isPart";
  rdfs:domain cimr:EquipmentOrContainer;
  rdfs:range cimr:EquipmentOrContainer;
  rdfs:label "is part transitive";
  owl:inverseOf cimr:hasPartTransitive .

cimr:mridSignificantPart a owl:DatatypeProperty;
  rdfs:comment "CIM UUIDs vary in the first component and confuse some indexers. This property isolates only the significant part if the id for easier indexing";
  rdfs:domain cim:IdentifiedObject;
  rdfs:range xsd:string;
  rdfs:label "MRID significant part" .

nc:AmbientTemperatureDependencyCurve a owl:Class;
  rdfs:comment "A curve or functional relationship between the ambient temperature independent variable (X-axis) and relative temperature dependent (Y-axis) variables."@en;
  rdfs:subClassOf nc:LimitDependencyCurve;
  rdfs:label "AmbientTemperatureDependencyCurve" .

nc:AutoReclosingKind a owl:Class;
  rdfs:comment """The type of autoreclosing that occurred with the trip.

If high-speed automatic reclosing is successful at one end of a line, but the line needs to be reclosed manually at the other end, choose manual reclosing.

In this document, high-speed automatic reclosing refers to automatic reclosing after less than 2 seconds."""@en;
  rdfs:label "AutoReclosingKind" .

nc:AvailabilityFunctionKind a owl:Class;
  rdfs:comment "Kind of availability that is affecting the function."@en;
  rdfs:label "AvailabilityFunctionKind" .

nc:AvailabilityScheduleCauseKind a owl:Class;
  rdfs:comment "The kinds of cause of the (un)availability schedule."@en;
  rdfs:label "AvailabilityScheduleCauseKind" .

nc:BaseTimeSeries a owl:Class;
  rdfs:comment "Time series of values at points in time."@en;
  rdfs:subClassOf cim:IdentifiedObject;
  rdfs:label "BaseTimeSeries" .

nc:BaseTimeSeries.generatedAtTime a owl:FunctionalProperty, owl:DatatypeProperty;
  rdfs:comment "The time this time series (entity) come to existents and available for use."@en;
  rdfs:domain nc:BaseTimeSeries;
  rdfs:range xsd:dateTime;
  rdfs:label "generatedAtTime";
  cims:multiplicity cims:M:0..1 .

nc:BaseTimeSeries.interpolationKind a owl:ObjectProperty, owl:FunctionalProperty;
  rdfs:comment "Kind of interpolation done between time point."@en;
  rdfs:domain nc:BaseTimeSeries;
  rdfs:range nc:TimeSeriesInterpolationKind;
  rdfs:label "interpolationKind";
  cims:multiplicity cims:M:1..1 .

nc:BaseTimeSeries.kind a owl:ObjectProperty, owl:FunctionalProperty;
  rdfs:comment "Kind of base time series."@en;
  rdfs:domain nc:BaseTimeSeries;
  rdfs:range nc:BaseTimeSeriesKind;
  rdfs:label "kind";
  cims:multiplicity cims:M:1..1 .

nc:BaseTimeSeries.percentile a owl:FunctionalProperty, owl:DatatypeProperty;
  rdfs:comment "The percentile is a number where a certain percentage of scores/ranking/values of a sample fall below that number. This is a way for expressing uncertainty in the number provided."@en;
  rdfs:domain nc:BaseTimeSeries;
  rdfs:range xsd:integer;
  rdfs:label "percentile";
  cims:multiplicity cims:M:0..1 .

nc:BaseTimeSeriesKind a owl:Class;
  rdfs:comment "Kind of time series."@en;
  rdfs:label "BaseTimeSeriesKind" .

nc:BaseTimeSeriesKind.forecast a nc:BaseTimeSeriesKind;
  rdfs:comment "Time series is forecast data. The values represent the result of scientific predictions based on historical time stamped data."@en;
  rdfs:label "forecast" .

nc:BidDirectionKind a owl:Class;
  rdfs:comment "Kind of direction of the bid."@en;
  rdfs:label "BidDirectionKind" .

nc:BiddingZone a owl:Class;
  rdfs:comment "A bidding zone is a market-based method for handling power transmission congestion. It consists of scheduling areas that include the relevant production (supply) and consumption (demand) to form an electrical area with the same market price without capacity allocation."@en;
  rdfs:subClassOf cim:PowerSystemResource;
  rdfs:label "BiddingZone" .

nc:BiddingZone.BiddingZoneBorderOne a owl:ObjectProperty, owl:InverseFunctionalProperty;
  rdfs:comment "The primary side of the border."@en;
  rdfs:domain nc:BiddingZone;
  rdfs:range nc:BiddingZoneBorder;
  rdfs:label "BiddingZoneBorderOne";
  cims:multiplicity cims:M:0..n;
  owl:inverseOf nc:BiddingZoneBorder.BiddingZoneOne .

nc:BiddingZone.BiddingZoneBorderTwo a owl:ObjectProperty, owl:InverseFunctionalProperty;
  rdfs:comment "The secondary side of the border."@en;
  rdfs:domain nc:BiddingZone;
  rdfs:range nc:BiddingZoneBorder;
  rdfs:label "BiddingZoneBorderTwo";
  cims:multiplicity cims:M:0..n;
  owl:inverseOf nc:BiddingZoneBorder.BiddingZoneTwo .

nc:BiddingZone.SchedulingArea a owl:ObjectProperty, owl:InverseFunctionalProperty;
  rdfs:comment "The scheduling area that has bidding zone."@en;
  rdfs:domain nc:BiddingZone;
  rdfs:range nc:SchedulingArea;
  rdfs:label "SchedulingArea";
  cims:multiplicity cims:M:1..n;
  owl:inverseOf nc:SchedulingArea.BiddingZone .

nc:BiddingZone.isTradeEnabled a owl:FunctionalProperty, owl:DatatypeProperty;
  rdfs:comment "Identifies the mechanism for determining the energy price for a given bidding zone. If true, the bid and the offer is expected to be provided for the bidding zone to create the market price. If false,  other mechanism determines the price of energy for a given bidding zone, e.g. virtual bidding zone."@en;
  rdfs:domain nc:BiddingZone;
  rdfs:range xsd:boolean;
  rdfs:label "isTradeEnabled";
  cims:multiplicity cims:M:1..1 .

nc:BiddingZoneBorder a owl:Class;
  rdfs:comment "Defines the aggregated connection capacity between two Bidding Zones."@en;
  rdfs:subClassOf cim:PowerSystemResource;
  rdfs:label "BiddingZoneBorder" .

nc:BiddingZoneBorder.BiddingZoneOne a owl:ObjectProperty, owl:FunctionalProperty;
  rdfs:comment "The bidding zone for the primary side."@en;
  rdfs:domain nc:BiddingZoneBorder;
  rdfs:range nc:BiddingZone;
  rdfs:label "BiddingZoneOne";
  cims:multiplicity cims:M:1..1;
  owl:inverseOf nc:BiddingZone.BiddingZoneBorderOne .

nc:BiddingZoneBorder.BiddingZoneTwo a owl:ObjectProperty, owl:FunctionalProperty;
  rdfs:comment "The bidding zone for the secondary side."@en;
  rdfs:domain nc:BiddingZoneBorder;
  rdfs:range nc:BiddingZone;
  rdfs:label "BiddingZoneTwo";
  cims:multiplicity cims:M:1..1;
  owl:inverseOf nc:BiddingZone.BiddingZoneBorderTwo .

nc:CalculationKind a owl:Class;
  rdfs:comment "Kind of calculation operation that can be done to Measurement."@en;
  rdfs:label "CalculationKind" .

nc:CapacityCalculationRegion a owl:Class;
  rdfs:comment "Capacity calculation region is a coherent part of the interconnected system that is used for calculating the transmission capacity for a bidding zone or between bidding zones."@en;
  rdfs:subClassOf nc:Region;
  rdfs:label "CapacityCalculationRegion" .

nc:CertaintyLevelKind a owl:Class;
  rdfs:comment "High certainty level is used when the cause of a fault is 100 % certain or when the cause is the most probable cause and potentially determined by an expert."@en;
  rdfs:label "CertaintyLevelKind" .

nc:Circuit a owl:Class;
  rdfs:comment "A circuit is a collection of equipment in a network graph that provide common stability limits. The relevant equipment is in general given by the identifying terminal. A software application that can do topology processing shall calculate the equipment belonging to the circuit, if there are no stability limits associated to it. In case of stability limits, the containment reflects the equipments that were used in the calculation/analysis."@en;
  rdfs:subClassOf cim:PowerSystemResource;
  rdfs:label "Circuit" .

nc:Circuit.CircuitShare a owl:ObjectProperty, owl:InverseFunctionalProperty;
  rdfs:comment "The circuit share of the given power transfer corridor."@en;
  rdfs:domain nc:Circuit;
  rdfs:range nc:CircuitShare;
  rdfs:label "CircuitShare";
  cims:multiplicity cims:M:0..n;
  owl:inverseOf nc:CircuitShare.Circuit .

nc:Circuit.IdentifyingTerminal a owl:ObjectProperty, owl:InverseFunctionalProperty,
    owl:FunctionalProperty;
  rdfs:comment "Terminal that identifies the circuit."@en;
  rdfs:domain nc:Circuit;
  rdfs:range cim:Terminal;
  rdfs:label "IdentifyingTerminal";
  cims:multiplicity cims:M:0..1;
  owl:inverseOf nc:Terminal.Circuit .

nc:Circuit.positiveFlowIn a owl:FunctionalProperty, owl:DatatypeProperty;
  rdfs:comment "True, if the positive value on the terminal shall be considered flow into the circuit. False, if the positive value on the terminal shall be considered flow out of the circuit."@en;
  rdfs:domain nc:Circuit;
  rdfs:range xsd:boolean;
  rdfs:label "positiveFlowIn";
  cims:multiplicity cims:M:1..1 .

nc:CircuitShare a owl:Class;
  rdfs:comment "Defines the share of the circuit which is part of an associated power transfer corridor."@en;
  rdfs:subClassOf cim:IdentifiedObject;
  rdfs:label "CircuitShare" .

nc:CircuitShare.Circuit a owl:ObjectProperty, owl:FunctionalProperty;
  rdfs:comment "The circuit that has a share of the power system corridor."@en;
  rdfs:domain nc:CircuitShare;
  rdfs:range nc:Circuit;
  rdfs:label "Circuit";
  cims:multiplicity cims:M:1..1;
  owl:inverseOf nc:Circuit.CircuitShare .

nc:CircuitShare.PowerTransferCorridor a owl:ObjectProperty, owl:FunctionalProperty;
  rdfs:comment "The power transfer corridor that has this circuit share."@en;
  rdfs:domain nc:CircuitShare;
  rdfs:range nc:PowerTransferCorridor;
  rdfs:label "PowerTransferCorridor";
  cims:multiplicity cims:M:1..1;
  owl:inverseOf nc:PowerTransferCorridor.CircuitShare .

nc:CircuitShare.contributionFactor a owl:FunctionalProperty, owl:DatatypeProperty;
  rdfs:comment """Contribution factor for the circuit which is part of a power transfer corridor.
The allowed value range is [0,100]."""@en;
  rdfs:domain nc:CircuitShare;
  rdfs:range xsd:float;
  rdfs:label "contributionFactor";
  cims:multiplicity cims:M:1..1;
  cim:unitMultiplier cim:UnitMultiplier.none;
  cim:unitSymbol cim:UnitSymbol.none;
  qudt:hasQuantityKind cim:PerCent;
  qudt:hasUnit unit:PERCENT .

nc:CircuitShare.normalContributionFactor a owl:FunctionalProperty, owl:DatatypeProperty;
  rdfs:comment """Normal contribution factor for the circuit which is part of a power transfer corridor.
The allowed value range is [0,100]."""@en;
  rdfs:domain nc:CircuitShare;
  rdfs:range xsd:float;
  rdfs:label "normalContributionFactor";
  cims:multiplicity cims:M:0..1;
  cim:unitMultiplier cim:UnitMultiplier.none;
  cim:unitSymbol cim:UnitSymbol.none;
  qudt:hasQuantityKind cim:PerCent;
  qudt:hasUnit unit:PERCENT .

nc:CompensatorControlModeKind a owl:Class;
  rdfs:comment "Kind of compensator controller mode."@en;
  rdfs:label "CompensatorControlModeKind" .

nc:Contingency.EquipmentOperator a owl:ObjectProperty, owl:FunctionalProperty;
  rdfs:comment "System operator that is operating the equipment that is being run a contingency on."@en;
  rdfs:domain cim:Contingency;
  rdfs:range nc:SystemOperator;
  rdfs:label "EquipmentOperator";
  cims:multiplicity cims:M:0..1;
  owl:inverseOf nc:SystemOperator.Contingency .

nc:Contingency.normalMustStudy a owl:FunctionalProperty, owl:DatatypeProperty;
  rdfs:comment "Specifies the requirement of study the contingency under normal operating conditions. True means the contingency must be study in a normal scenario. False means that the contingency does not need to be included in the scenario. This is the default value if mustStudy is missing."@en;
  rdfs:domain cim:Contingency;
  rdfs:range xsd:boolean;
  rdfs:label "normalMustStudy";
  cims:multiplicity cims:M:1..1 .

nc:Contingency.normalProbability a owl:FunctionalProperty, owl:DatatypeProperty;
  rdfs:comment """Normal probability of the occurrence of the contingency based on normal operational condition. The value is used as the default if the probability is missing.
The allowed value range is [0,100]."""@en;
  rdfs:domain cim:Contingency;
  rdfs:range xsd:float;
  rdfs:label "normalProbability";
  cims:multiplicity cims:M:0..1;
  cim:unitMultiplier cim:UnitMultiplier.none;
  cim:unitSymbol cim:UnitSymbol.none;
  qudt:hasQuantityKind cim:PerCent;
  qudt:hasUnit unit:PERCENT .

nc:Contingency.probability a owl:FunctionalProperty, owl:DatatypeProperty;
  rdfs:comment """The forecasted probability of the occurrence of the contingency based on the given operational condition, status of the equipment and the forecasted environment condition.
The allowed value range is [0,100]."""@en;
  rdfs:domain cim:Contingency;
  rdfs:range xsd:float;
  rdfs:label "probability";
  cims:multiplicity cims:M:0..1;
  cim:unitMultiplier cim:UnitMultiplier.none;
  cim:unitSymbol cim:UnitSymbol.none;
  qudt:hasQuantityKind cim:PerCent;
  qudt:hasUnit unit:PERCENT .

nc:ContingencyConditionKind a owl:Class;
  rdfs:comment "Kinds of occurrence criteria of application."@en;
  rdfs:label "ContingencyConditionKind" .

nc:ControlArea.SchedulingArea a owl:ObjectProperty, owl:InverseFunctionalProperty;
  rdfs:comment "The scheduling area related to a control area."@en;
  rdfs:domain cim:ControlArea;
  rdfs:range nc:SchedulingArea;
  rdfs:label "SchedulingArea";
  cims:multiplicity cims:M:1..n;
  owl:inverseOf nc:SchedulingArea.ControlArea .

nc:CoordinatedCapacityCalculator a owl:Class;
  rdfs:comment "A role that coordinates and executes the task of calculating transmission capacity."@en;
  rdfs:subClassOf nc:SystemOperationCoordinator;
  rdfs:label "CoordinatedCapacityCalculator" .

nc:CostSettledKind a owl:Class;
  rdfs:comment "Kind describing how settled the cost is in regards to changes."@en;
  rdfs:label "CostSettledKind" .

nc:CriticalElementContingencyKind a owl:Class;
  rdfs:comment "The kind of critical element contingency."@en;
  rdfs:label "CriticalElementContingencyKind" .

nc:DCControlModeKind a owl:Class;
  rdfs:comment "Kind of DC control mode."@en;
  rdfs:label "DCControlModeKind" .

nc:DCSystemDirectionKind a owl:Class;
  rdfs:comment "Direction kinds of the DC system."@en;
  rdfs:label "DCSystemDirectionKind" .

nc:DCSystemTransmissionKind a owl:Class;
  rdfs:comment "DC system transmission kind."@en;
  rdfs:label "DCSystemTransmissionKind" .

nc:DayOfWeekKind a owl:Class;
  rdfs:comment "The kind of day to be included in a regular schedule."@en;
  rdfs:label "DayOfWeekKind" .

nc:DistributionSystemOperator a owl:Class;
  rdfs:comment "A system operator that is responsible for operating of energy distribution network from transmission level down to low voltage levels including the connection to household."@en;
  rdfs:subClassOf nc:SystemOperator;
  rdfs:label "DistributionSystemOperator" .

nc:ElementCombinationConstraintKind a owl:Class;
  rdfs:comment "Kind of constraint for an element combination."@en;
  rdfs:label "ElementCombinationConstraintKind" .

nc:EnergyConsumer.LoadAction a owl:ObjectProperty, owl:InverseFunctionalProperty;
  rdfs:comment "The action appled to an EnergyConsumer."@en;
  rdfs:domain cim:EnergyConsumer;
  rdfs:range nc:LoadAction;
  rdfs:label "LoadAction";
  cims:multiplicity cims:M:0..n;
  owl:inverseOf nc:LoadAction.EnergyConsumer .

nc:EnergyDemandKind a owl:Class;
  rdfs:comment "Kind of energy demand."@en;
  rdfs:label "EnergyDemandKind" .

nc:EnergyKind a owl:Class;
  rdfs:comment "Categories of energy used for energy groups."@en;
  rdfs:label "EnergyKind" .

nc:Equipment.InServiceAction a owl:ObjectProperty, owl:InverseFunctionalProperty;
  rdfs:comment "Action that is applied to an equipment."@en;
  rdfs:domain cim:Equipment;
  rdfs:range nc:InServiceAction;
  rdfs:label "InServiceAction";
  cims:multiplicity cims:M:0..n;
  owl:inverseOf nc:InServiceAction.Equipment .

nc:Equipment.PinEquipment a owl:ObjectProperty, owl:InverseFunctionalProperty;
  rdfs:comment "The pin that uses this input."@en;
  rdfs:domain cim:Equipment;
  rdfs:range nc:PinEquipment;
  rdfs:label "PinEquipment";
  cims:multiplicity cims:M:0..n;
  owl:inverseOf nc:PinEquipment.Equipment .

nc:Equipment.PinEquipmentTripping a owl:ObjectProperty, owl:InverseFunctionalProperty;
  rdfs:comment "Pin equipment that is used as gate input."@en;
  rdfs:domain cim:Equipment;
  rdfs:range nc:PinEquipmentTripping;
  rdfs:label "PinEquipmentTripping";
  cims:multiplicity cims:M:0..n;
  owl:inverseOf nc:PinEquipmentTripping.Equipment .

nc:FaultCategoryKind a owl:Class;
  rdfs:comment "Available kinds of fault categories."@en;
  rdfs:label "FaultCategoryKind" .

nc:FaultKind a owl:Class;
  rdfs:comment """One fault can consist of several fault types. If a fault consists of several fault types, the most significant fault type is used.

In case of developing faults, that is in faults changing from one type to another, the final type is given."""@en;
  rdfs:label "FaultKind" .

nc:FunctionInputVariable a owl:Class;
  rdfs:comment "Functional input variable defines the domain of the function."@en;
  rdfs:subClassOf cim:IdentifiedObject;
  rdfs:label "FunctionInputVariable" .

nc:Gate a owl:Class;
  rdfs:comment "Logical gate that supports a logical operation based on the input."@en;
  rdfs:subClassOf cim:IdentifiedObject;
  rdfs:label "Gate" .

nc:Gate.GateInputPin a owl:ObjectProperty, owl:InverseFunctionalProperty;
  rdfs:comment "This is the input to the gate."@en;
  rdfs:domain nc:Gate;
  rdfs:range nc:GateInputPin;
  rdfs:label "GateInputPin";
  cims:multiplicity cims:M:1..n;
  owl:inverseOf nc:GateInputPin.Gate .

nc:Gate.PinGate a owl:ObjectProperty, owl:InverseFunctionalProperty;
  rdfs:comment "The pin for this gate output."@en;
  rdfs:domain nc:Gate;
  rdfs:range nc:PinGate;
  rdfs:label "PinGate";
  cims:multiplicity cims:M:0..n;
  owl:inverseOf nc:PinGate.GateOutput .

nc:Gate.StageTrigger a owl:ObjectProperty, owl:InverseFunctionalProperty;
  rdfs:comment "The stage trigger associated with the gate trigger."@en;
  rdfs:domain nc:Gate;
  rdfs:range nc:StageTrigger;
  rdfs:label "StageTrigger";
  cims:multiplicity cims:M:0..n;
  owl:inverseOf nc:StageTrigger.GateTrigger .

nc:Gate.kind a owl:ObjectProperty, owl:FunctionalProperty;
  rdfs:comment "The logical operation of the gate."@en;
  rdfs:domain nc:Gate;
  rdfs:range nc:GateLogicKind;
  rdfs:label "kind";
  cims:multiplicity cims:M:1..1 .

nc:GateInputPin a owl:Class;
  rdfs:comment "Input pin for a logical gate. The condition described in the input pin gives a logical true or false. The result from measurement and calculation are converted to a true or false."@en;
  rdfs:subClassOf nc:FunctionInputVariable;
  rdfs:label "GateInputPin" .

nc:GateInputPin.Gate a owl:ObjectProperty, owl:FunctionalProperty;
  rdfs:comment "The Gate that has this input."@en;
  rdfs:domain nc:GateInputPin;
  rdfs:range nc:Gate;
  rdfs:label "Gate";
  cims:multiplicity cims:M:1..1;
  owl:inverseOf nc:Gate.GateInputPin .

nc:GateInputPin.logicKind a owl:ObjectProperty, owl:FunctionalProperty;
  rdfs:comment "The logical operator kind used for comparison."@en;
  rdfs:domain nc:GateInputPin;
  rdfs:range nc:LogicalOperatorsKind;
  rdfs:label "logicKind";
  cims:multiplicity cims:M:0..1, cims:M:1..1 .

nc:GateInputPin.negate a owl:FunctionalProperty, owl:DatatypeProperty;
  rdfs:comment "Invert/negate the result of the comparison."@en;
  rdfs:domain nc:GateInputPin;
  rdfs:range xsd:boolean;
  rdfs:label "negate";
  cims:multiplicity cims:M:0..1, cims:M:1..1 .

nc:GateInputPin.thresholdPercentage a owl:FunctionalProperty, owl:DatatypeProperty;
  rdfs:comment """The threshold percentage that should be used for compare with the percentage change between input value and threshold value.
The allowed value range is [0,100]."""@en;
  rdfs:domain nc:GateInputPin;
  rdfs:range xsd:float;
  rdfs:label "thresholdPercentage";
  cims:multiplicity cims:M:0..1;
  cim:unitMultiplier cim:UnitMultiplier.none;
  cim:unitSymbol cim:UnitSymbol.none;
  qudt:hasQuantityKind cim:PerCent;
  qudt:hasUnit unit:PERCENT .

nc:GateInputPin.thresholdValue a owl:FunctionalProperty, owl:DatatypeProperty;
  rdfs:comment "The threshold value that should be used for compare with the input value."@en;
  rdfs:domain nc:GateInputPin;
  rdfs:range xsd:float;
  rdfs:label "thresholdValue";
  cims:multiplicity cims:M:0..1 .

nc:GateLogicKind a owl:Class;
  rdfs:comment "Define the different logical operations."@en;
  rdfs:label "GateLogicKind" .

nc:GateLogicKind.and a nc:GateLogicKind;
  rdfs:comment "A logical AND operation. True when all inputs are true."@en;
  rdfs:label "and" .

nc:GateLogicKind.or a nc:GateLogicKind;
  rdfs:comment "A logical OR operation. True when one or more inputs are true."@en;
  rdfs:label "or" .

nc:GeneratingUnit.ScheduleResource a owl:ObjectProperty, owl:FunctionalProperty;
  rdfs:comment "The schedule resource that has this generating unit."@en;
  rdfs:domain cim:GeneratingUnit;
  rdfs:range nc:ScheduleResource;
  rdfs:label "ScheduleResource";
  cims:multiplicity cims:M:0..1;
  owl:inverseOf nc:ScheduleResource.GeneratingUnit .

nc:GeothermalUnitKind a owl:Class;
  rdfs:comment "Kind of geothermal."@en;
  rdfs:label "GeothermalUnitKind" .

nc:GridStateAlteration a owl:Class;
  rdfs:comment "Grid state alteration is a change of values describing state (operating point) of one element in the grid model compared to the base case."@en;
  rdfs:subClassOf cim:IdentifiedObject;
  rdfs:label "GridStateAlteration" .

nc:GridStateAlteration.GridStateAlterationCollection a owl:ObjectProperty, owl:FunctionalProperty;
  rdfs:comment "The collection that has a GridStateAlteration."@en;
  rdfs:domain nc:GridStateAlteration;
  rdfs:range nc:GridStateAlterationCollection;
  rdfs:label "GridStateAlterationCollection";
  cims:multiplicity cims:M:0..1;
  owl:inverseOf nc:GridStateAlterationCollection.GridStateAlteration .

nc:GridStateAlteration.PropertyReference a owl:ObjectProperty, owl:FunctionalProperty;
  rdfs:comment "The property reference for this grid state alteration."@en;
  rdfs:domain nc:GridStateAlteration;
  rdfs:range nc:PropertyReference;
  rdfs:label "PropertyReference";
  cims:multiplicity cims:M:1..1;
  owl:inverseOf nc:PropertyReference.GridStateAlteration .

nc:GridStateAlteration.RangeConstraint a owl:ObjectProperty, owl:InverseFunctionalProperty;
  rdfs:comment "The range constraint associated with a given GridStateAlteration."@en;
  rdfs:domain nc:GridStateAlteration;
  rdfs:range nc:RangeConstraint;
  rdfs:label "RangeConstraint";
  cims:multiplicity cims:M:0..n;
  owl:inverseOf nc:RangeConstraint.GridStateAlteration .

nc:GridStateAlteration.enabled a owl:FunctionalProperty, owl:DatatypeProperty;
  rdfs:comment "The status of the GridStateAlteration set by an operation or by a signal resulting from a control action."@en;
  rdfs:domain nc:GridStateAlteration;
  rdfs:range xsd:boolean;
  rdfs:label "enabled";
  cims:multiplicity cims:M:1..1 .

nc:GridStateAlteration.normalEnabled a owl:FunctionalProperty, owl:DatatypeProperty;
  rdfs:comment "The default/normal value used when other active signal/values are missing."@en;
  rdfs:domain nc:GridStateAlteration;
  rdfs:range xsd:boolean;
  rdfs:label "normalEnabled";
  cims:multiplicity cims:M:0..1 .

nc:GridStateAlterationCollection a owl:Class;
  rdfs:comment "A collection of grid state alterations."@en;
  rdfs:subClassOf cim:IdentifiedObject;
  rdfs:label "GridStateAlterationCollection" .

nc:GridStateAlterationCollection.GridStateAlteration a owl:ObjectProperty, owl:InverseFunctionalProperty;
  rdfs:comment "The GridStateAlteration that belongs to the collection."@en;
  rdfs:domain nc:GridStateAlterationCollection;
  rdfs:range nc:GridStateAlteration;
  rdfs:label "GridStateAlteration";
  cims:multiplicity cims:M:0..n;
  owl:inverseOf nc:GridStateAlteration.GridStateAlterationCollection .

nc:GridStateAlterationCollection.StageAction a owl:ObjectProperty, owl:InverseFunctionalProperty;
  rdfs:comment "The stage action related to this GridStateAlterationCollection."@en;
  rdfs:domain nc:GridStateAlterationCollection;
  rdfs:range nc:Stage;
  rdfs:label "StageAction";
  cims:multiplicity cims:M:0..n;
  owl:inverseOf nc:Stage.GridStateAlterationCollection .

nc:ImpactAgreementKind a owl:Class;
  rdfs:comment "The impact agreement for the remedial action."@en;
  rdfs:label "ImpactAgreementKind" .

nc:InServiceAction a owl:Class;
  rdfs:comment "In service action represents a change of the status of the equipment in the grid model compared to the base case."@en;
  rdfs:subClassOf nc:GridStateAlteration;
  rdfs:label "InServiceAction" .

nc:InServiceAction.Equipment a owl:ObjectProperty, owl:FunctionalProperty;
  rdfs:comment "Equipment that has a in service action associated."@en;
  rdfs:domain nc:InServiceAction;
  rdfs:range cim:Equipment;
  rdfs:label "Equipment";
  cims:multiplicity cims:M:1..1;
  owl:inverseOf nc:Equipment.InServiceAction .

nc:InjectionControlModeKind a owl:Class;
  rdfs:comment "Kind of injection controller mode."@en;
  rdfs:label "InjectionControlModeKind" .

nc:LimitDependencyCurve a owl:Class;
  rdfs:comment "A curve or functional relationship between an independent variable (X-axis) and limiting dependent (Y-axis) variables."@en;
  rdfs:subClassOf cim:Curve;
  rdfs:label "LimitDependencyCurve" .

nc:LineCircuit a owl:Class;
  rdfs:comment "A line circuit is a circuit that has at least one ACLineSegment and may or may not include related switching and/or auxiliary equipment."@en;
  rdfs:subClassOf nc:Circuit;
  rdfs:label "LineCircuit" .

nc:LoadAction a owl:Class;
  rdfs:comment "Load action."@en;
  rdfs:subClassOf nc:SetPointAction;
  rdfs:label "LoadAction" .

nc:LoadAction.EnergyConsumer a owl:ObjectProperty, owl:FunctionalProperty;
  rdfs:comment "The EnergyConsumer that is associated with a load action."@en;
  rdfs:domain nc:LoadAction;
  rdfs:range cim:EnergyConsumer;
  rdfs:label "EnergyConsumer";
  cims:multiplicity cims:M:1..1;
  owl:inverseOf nc:EnergyConsumer.LoadAction .

nc:LogicalOperatorsKind a owl:Class;
  rdfs:comment "Kinds of logical operators for comparison."@en;
  rdfs:label "LogicalOperatorsKind" .

nc:MarineUnitKind a owl:Class;
  rdfs:comment "Kind of marine energy capture."@en;
  rdfs:label "MarineUnitKind" .

nc:NuclearReactorKind a owl:Class;
  rdfs:comment "Kind of nuclear reactor."@en;
  rdfs:label "NuclearReactorKind" .

nc:ObservableQuantityKind a owl:Class;
  rdfs:comment "Kind of observable quantity."@en;
  rdfs:label "ObservableQuantityKind" .

nc:OperationalLimit.PinOperationallLimit a owl:ObjectProperty, owl:InverseFunctionalProperty;
  rdfs:comment "The operational limit pin pin that uses this operational limit."@en;
  rdfs:domain cim:OperationalLimit;
  rdfs:range nc:PinOperationalLimit;
  rdfs:label "PinOperationallLimit";
  cims:multiplicity cims:M:0..n;
  owl:inverseOf nc:PinOperationalLimit.OperationalLimit .

nc:OperationalLimitSet.PowerTransferCorridor a owl:ObjectProperty, owl:FunctionalProperty;
  rdfs:comment "The power transfer corridor that has this operational limit set."@en;
  rdfs:domain cim:OperationalLimitSet;
  rdfs:range nc:PowerTransferCorridor;
  rdfs:label "PowerTransferCorridor";
  cims:multiplicity cims:M:0..1;
  owl:inverseOf nc:PowerTransferCorridor.OperationalLimitSet .

nc:OrdinaryContingency a owl:Class;
  rdfs:comment "Ordinary contingency means the occurrence of a contingency of a single branch or injection."@en;
  rdfs:subClassOf cim:Contingency;
  rdfs:label "OrdinaryContingency" .

nc:OrdinaryPowerTransferCorridor a owl:Class;
  rdfs:comment "Power transfer corridor defined for normal operating network."@en;
  rdfs:subClassOf nc:PowerTransferCorridor;
  rdfs:label "OrdinaryPowerTransferCorridor" .

nc:OutcomeImpactAssessmentKind a owl:Class;
  rdfs:comment "Outcome impact assessments kinds."@en;
  rdfs:label "OutcomeImpactAssessmentKind" .

nc:PeakKind a owl:Class;
  rdfs:comment "Kind of time period with similar intensity."@en;
  rdfs:label "PeakKind" .

nc:PinDCTerminalKind a owl:Class;
  rdfs:comment "The kind of quantities that can serve as an input value for the DCTerminal pin."@en;
  rdfs:label "PinDCTerminalKind" .

nc:PinEquipment a owl:Class;
  rdfs:comment "Input pin associated with an Equipment. It is used for the comparison."@en;
  rdfs:subClassOf nc:GateInputPin;
  rdfs:label "PinEquipment" .

nc:PinEquipment.Equipment a owl:ObjectProperty, owl:FunctionalProperty;
  rdfs:comment "The Equipment that is used in the input pin."@en;
  rdfs:domain nc:PinEquipment;
  rdfs:range cim:Equipment;
  rdfs:label "Equipment";
  cims:multiplicity cims:M:1..1;
  owl:inverseOf nc:Equipment.PinEquipment .

nc:PinEquipment.PropertyReference a owl:ObjectProperty, owl:FunctionalProperty;
  rdfs:comment "The property reference for this pin equipment."@en;
  rdfs:domain nc:PinEquipment;
  rdfs:range nc:PropertyReference;
  rdfs:label "PropertyReference";
  cims:multiplicity cims:M:1..1;
  owl:inverseOf nc:PropertyReference.PinEquipment .

nc:PinEquipmentTripping a owl:Class;
  rdfs:comment "Input pin associated with an Equipment. It is used to determine if the equipment is tripped between two consecutive stages, i.e. the equipment is in service at pre-fault stage and it is out of service at post-fault stage."@en;
  rdfs:subClassOf nc:GateInputPin;
  rdfs:label "PinEquipmentTripping" .

nc:PinEquipmentTripping.Equipment a owl:ObjectProperty, owl:FunctionalProperty;
  rdfs:comment "Equipment that is tripped."@en;
  rdfs:domain nc:PinEquipmentTripping;
  rdfs:range cim:Equipment;
  rdfs:label "Equipment";
  cims:multiplicity cims:M:1..1;
  owl:inverseOf nc:Equipment.PinEquipmentTripping .

nc:PinGate a owl:Class;
  rdfs:comment "An output from one gate represents an input to another gate."@en;
  rdfs:subClassOf nc:GateInputPin;
  rdfs:label "PinGate" .

nc:PinGate.GateOutput a owl:ObjectProperty, owl:FunctionalProperty;
  rdfs:comment "The output of the gate."@en;
  rdfs:domain nc:PinGate;
  rdfs:range nc:Gate;
  rdfs:label "GateOutput";
  cims:multiplicity cims:M:1..1;
  owl:inverseOf nc:Gate.PinGate .

nc:PinOperationalLimit a owl:Class;
  rdfs:comment "Input pin associated with the limits of a Terminal. It is used for comparison."@en;
  rdfs:subClassOf nc:GateInputPin;
  rdfs:label "PinOperationalLimit" .

nc:PinOperationalLimit.OperationalLimit a owl:ObjectProperty, owl:FunctionalProperty;
  rdfs:comment "The operational limit that is used in the input pin."@en;
  rdfs:domain nc:PinOperationalLimit;
  rdfs:range cim:OperationalLimit;
  rdfs:label "OperationalLimit";
  cims:multiplicity cims:M:1..1;
  owl:inverseOf nc:OperationalLimit.PinOperationallLimit .

nc:PinPowerTransferCorridorKind a owl:Class;
  rdfs:comment "The kind of quantities that can serve as an input value for the PowerTransferCorridor pin."@en;
  rdfs:label "PinPowerTransferCorridorKind" .

nc:PinTerminal a owl:Class;
  rdfs:comment "Input pin associated with a Terminal. It is used for comparison."@en;
  rdfs:subClassOf nc:GateInputPin;
  rdfs:label "PinTerminal" .

nc:PinTerminal.Terminal a owl:ObjectProperty, owl:FunctionalProperty;
  rdfs:comment "The Terminal that is used in the input pin."@en;
  rdfs:domain nc:PinTerminal;
  rdfs:range cim:Terminal;
  rdfs:label "Terminal";
  cims:multiplicity cims:M:1..1;
  owl:inverseOf nc:Terminal.PinTerminal .

nc:PinTerminal.kind a owl:ObjectProperty, owl:FunctionalProperty;
  rdfs:comment "The kind of quantity which is used as an input value."@en;
  rdfs:domain nc:PinTerminal;
  rdfs:range nc:PinTerminalKind;
  rdfs:label "kind";
  cims:multiplicity cims:M:1..1 .

nc:PinTerminalKind a owl:Class;
  rdfs:comment "The kind of quantities that can serve as an input value for the pin."@en;
  rdfs:label "PinTerminalKind" .

nc:PinTerminalKind.activePower a nc:PinTerminalKind;
  rdfs:comment "Active power on the Terminal."@en;
  rdfs:label "activePower" .

nc:PinTerminalKind.voltageMagnitude a nc:PinTerminalKind;
  rdfs:comment "Voltage magnitude on the Terminal."@en;
  rdfs:label "voltageMagnitude" .

nc:PowerBidDependencyKind a owl:Class;
  rdfs:comment "Kind of power bid dependency."@en;
  rdfs:label "PowerBidDependencyKind" .

nc:PowerBlockKind a owl:Class;
  rdfs:comment "Power block kind describes the increase and/or decrease of power."@en;
  rdfs:label "PowerBlockKind" .

nc:PowerElectricalChemicalUnitKind a owl:Class;
  rdfs:comment "Kind of power electrical chemical unit."@en;
  rdfs:label "PowerElectricalChemicalUnitKind" .

nc:PowerFrequencyControlKind a owl:Class;
  rdfs:comment "Kinds of power frequency control modes."@en;
  rdfs:label "PowerFrequencyControlKind" .

nc:PowerScheduleKind a owl:Class;
  rdfs:comment "Kind of power schedule."@en;
  rdfs:label "PowerScheduleKind" .

nc:PowerShiftKeyKind a owl:Class;
  rdfs:comment "Kind of generating and load shift keys strategy."@en;
  rdfs:label "PowerShiftKeyKind" .

nc:PowerSystemOrganisationRole a owl:Class;
  rdfs:comment "A role that is responsible for the functional operational of a power system resource."@en;
  rdfs:subClassOf cim:OrganisationRole;
  rdfs:label "PowerSystemOrganisationRole" .

nc:PowerTransferCorridor a owl:Class;
  rdfs:comment "A power transfer corridor is defined as a set of circuits (transmission lines or transformers) separating two portions of the power system, or a subset of circuits exposed to a substantial portion of the transmission exchange between two parts of the system."@en;
  rdfs:subClassOf cim:PowerSystemResource;
  rdfs:label "PowerTransferCorridor" .

nc:PowerTransferCorridor.CircuitShare a owl:ObjectProperty, owl:InverseFunctionalProperty;
  rdfs:comment "The circuit share for this power transfer corridor."@en;
  rdfs:domain nc:PowerTransferCorridor;
  rdfs:range nc:CircuitShare;
  rdfs:label "CircuitShare";
  cims:multiplicity cims:M:0..n;
  owl:inverseOf nc:CircuitShare.PowerTransferCorridor .

nc:PowerTransferCorridor.OperationalLimitSet a owl:ObjectProperty, owl:InverseFunctionalProperty;
  rdfs:comment "The operational limit set relevant for this power transfer corridor."@en;
  rdfs:domain nc:PowerTransferCorridor;
  rdfs:range cim:OperationalLimitSet;
  rdfs:label "OperationalLimitSet";
  cims:multiplicity cims:M:0..n;
  owl:inverseOf nc:OperationalLimitSet.PowerTransferCorridor .

nc:PowerTransferCorridor.enabled a owl:FunctionalProperty, owl:DatatypeProperty;
  rdfs:comment "It enables/disables the monitoring/assessment of a power transfer corridor. True means that the monitoring of the power transfer corridor is assessed. False means the power transfer corridor is not assessed."@en;
  rdfs:domain nc:PowerTransferCorridor;
  rdfs:range xsd:boolean;
  rdfs:label "enabled";
  cims:multiplicity cims:M:1..1 .

nc:PowerTransferCorridor.normalEnabled a owl:FunctionalProperty, owl:DatatypeProperty;
  rdfs:comment "It is the normal enable/disable the monitoring/assessment of a power transfer corridor. True means that the monitoring of the power transfer corridor is assessed. False means the power transfer corridor is not assessed."@en;
  rdfs:domain nc:PowerTransferCorridor;
  rdfs:range xsd:boolean;
  rdfs:label "normalEnabled";
  cims:multiplicity cims:M:0..1 .

nc:PropertyReference a owl:Class;
  rdfs:comment "The reference to a class and one of its properties."@en;
  rdfs:label "PropertyReference" .

nc:PropertyReference.GridStateAlteration a owl:ObjectProperty, owl:InverseFunctionalProperty;
  rdfs:comment "The grid state alteration for this property reference."@en;
  rdfs:domain nc:PropertyReference;
  rdfs:range nc:GridStateAlteration;
  rdfs:label "GridStateAlteration";
  cims:multiplicity cims:M:0..n;
  owl:inverseOf nc:GridStateAlteration.PropertyReference .

nc:PropertyReference.PinEquipment a owl:ObjectProperty, owl:InverseFunctionalProperty;
  rdfs:comment "The pin equipment that has this property reference."@en;
  rdfs:domain nc:PropertyReference;
  rdfs:range nc:PinEquipment;
  rdfs:label "PinEquipment";
  cims:multiplicity cims:M:0..n;
  owl:inverseOf nc:PinEquipment.PropertyReference .

nc:PropertyReference.StaticPropertyRange a owl:ObjectProperty, owl:InverseFunctionalProperty;
  rdfs:comment "Static property range that has this property reference."@en;
  rdfs:domain nc:PropertyReference;
  rdfs:range nc:StaticPropertyRange;
  rdfs:label "StaticPropertyRange";
  cims:multiplicity cims:M:0..n;
  owl:inverseOf nc:StaticPropertyRange.PropertyReference .

nc:RampingPrincipleKind a owl:Class;
  rdfs:comment "Kind of ramping principle."@en;
  rdfs:label "RampingPrincipleKind" .

nc:RangeConstraint a owl:Class;
  rdfs:comment "Defines the rage constraint."@en;
  rdfs:subClassOf cim:IdentifiedObject;
  rdfs:label "RangeConstraint" .

nc:RangeConstraint.GridStateAlteration a owl:ObjectProperty, owl:FunctionalProperty;
  rdfs:comment "The grid state alteration which has static range."@en;
  rdfs:domain nc:RangeConstraint;
  rdfs:range nc:GridStateAlteration;
  rdfs:label "GridStateAlteration";
  cims:multiplicity cims:M:1..1;
  owl:inverseOf nc:GridStateAlteration.RangeConstraint .

nc:RangeConstraint.direction a owl:ObjectProperty, owl:FunctionalProperty;
  rdfs:comment "Defines the direction of the attribute value referenced by the PropertyReference."@en;
  rdfs:domain nc:RangeConstraint;
  rdfs:range nc:RelativeDirectionKind;
  rdfs:label "direction";
  cims:multiplicity cims:M:1..1 .

nc:RangeConstraint.normalValue a owl:FunctionalProperty, owl:DatatypeProperty;
  rdfs:comment """The normal (initial) value. The meaning of the value is defined by the attribute referenced by the PropertyReference. The value can be integer, float or boolean. In case of boolean 1 equals true and 0 equals false.
If the valueKind is incremental or incrementalPercentage, then the value shall be positive (greater than zero).
If the valueKind is incrementalPercentage, then the value shall be in the range [0, 100]."""@en;
  rdfs:domain nc:RangeConstraint;
  rdfs:range xsd:float;
  rdfs:label "normalValue";
  cims:multiplicity cims:M:0..1 .

nc:RangeConstraint.value a owl:FunctionalProperty, owl:DatatypeProperty;
  rdfs:comment """The value at the time. The meaning of the value is defined by the attribute referenced by the PropertyReference. The value can be integer, float or boolean. In case of boolean 1 equals true and 0 equals false. 
If the valueKind is incremental or incrementalPercentage, then the value shall be positive (greater than zero).
If the valueKind is incrementalPercentage, then the value shall be in the range [0, 100]."""@en;
  rdfs:domain nc:RangeConstraint;
  rdfs:range xsd:float;
  rdfs:label "value";
  cims:multiplicity cims:M:1..1 .

nc:RangeConstraint.valueKind a owl:ObjectProperty, owl:FunctionalProperty;
  rdfs:comment "Kind of value offset for the range that applies to the attribute referenced by the PropertyReference."@en;
  rdfs:domain nc:RangeConstraint;
  rdfs:range nc:ValueOffsetKind;
  rdfs:label "valueKind";
  cims:multiplicity cims:M:0..1 .

nc:Region a owl:Class;
  rdfs:comment "A region where the system operator belongs to."@en;
  rdfs:subClassOf cim:PowerSystemResource;
  rdfs:label "Region" .

nc:RelativeDirectionKind a owl:Class;
  rdfs:comment "Kind of direction for the changes."@en;
  rdfs:label "RelativeDirectionKind" .

nc:RelativeDirectionKind.down a nc:RelativeDirectionKind;
  rdfs:comment "Down signifies that the changes are decreasing from the current status."@en;
  rdfs:label "down" .

nc:RemedialActionDependencyKind a owl:Class;
  rdfs:comment "Kind of dependency between remedial actions."@en;
  rdfs:label "RemedialActionDependencyKind" .

nc:RemedialActionKind a owl:Class;
  rdfs:comment "The different kinds for a remedial action."@en;
  rdfs:label "RemedialActionKind" .

nc:RemedialActionScheduleAcceptanceKind a owl:Class;
  rdfs:comment "The kind of acceptance for a remedial action schedule."@en;
  rdfs:label "RemedialActionScheduleAcceptanceKind" .

nc:RemedialActionScheduleDependencyKind a owl:Class;
  rdfs:comment "Kind of dependency between remedial action schedules."@en;
  rdfs:label "RemedialActionScheduleDependencyKind" .

nc:RemedialActionScheduleStatusKind a owl:Class;
  rdfs:comment "Remedial action schedule status kinds."@en;
  rdfs:label "RemedialActionScheduleStatusKind" .

nc:RemedialActionScheme a owl:Class;
  rdfs:comment """Remedial Action Scheme (RAS), Special Protection Schemes (SPS), System Protection Schemes (SPS) or System Integrity Protection Schemes (SIPS).
A Remedial Action Scheme consists of one or more stages that can trigger and execute a protection action."""@en;
  rdfs:subClassOf cim:PowerSystemResource;
  rdfs:label "RemedialActionScheme" .

nc:RemedialActionScheme.Stage a owl:ObjectProperty, owl:InverseFunctionalProperty;
  rdfs:comment "The stage for this remedial action scheme."@en;
  rdfs:domain nc:RemedialActionScheme;
  rdfs:range nc:Stage;
  rdfs:label "Stage";
  cims:multiplicity cims:M:1..n;
  owl:inverseOf nc:Stage.RemedialActionScheme .

nc:RemedialActionScheme.armed a owl:FunctionalProperty, owl:DatatypeProperty;
  rdfs:comment "Defines the arming status of the remedial action scheme. It is set by operation or by signal."@en;
  rdfs:domain nc:RemedialActionScheme;
  rdfs:range xsd:boolean;
  rdfs:label "armed";
  cims:multiplicity cims:M:1..1 .

nc:RemedialActionScheme.inService a owl:FunctionalProperty, owl:DatatypeProperty;
  rdfs:comment "Specifies the availability of the Remedial Action Scheme (RAS). If true, the RAS is available for contingency processing. If false, the RAS is treated by contingency processing as if it is not in the model."@en;
  rdfs:domain nc:RemedialActionScheme;
  rdfs:range xsd:boolean;
  rdfs:label "inService";
  cims:multiplicity cims:M:1..1 .

nc:RemedialActionScheme.kind a owl:ObjectProperty, owl:FunctionalProperty;
  rdfs:comment "Kind of Remedial Action Scheme."@en;
  rdfs:domain nc:RemedialActionScheme;
  rdfs:range nc:RemedialActionSchemeKind;
  rdfs:label "kind";
  cims:multiplicity cims:M:1..1 .

nc:RemedialActionScheme.normalArmed a owl:FunctionalProperty, owl:DatatypeProperty;
  rdfs:comment "Defines the normal arming status of the remedial action scheme."@en;
  rdfs:domain nc:RemedialActionScheme;
  rdfs:range xsd:boolean;
  rdfs:label "normalArmed";
  cims:multiplicity cims:M:1..1 .

nc:RemedialActionSchemeKind a owl:Class;
  rdfs:comment "Classification of Remedial Action Scheme."@en;
  rdfs:label "RemedialActionSchemeKind" .

nc:RemedialActionSchemeKind.sips a nc:RemedialActionSchemeKind;
  rdfs:comment "System Integrity Protection Scheme (SIPS). The triggering conditions are met through field measurements."@en;
  rdfs:label "sips" .

nc:RotatingMachine.RotatingMachineAction a owl:ObjectProperty, owl:InverseFunctionalProperty;
  rdfs:comment "The action applied to a rotating machine."@en;
  rdfs:domain cim:RotatingMachine;
  rdfs:range nc:RotatingMachineAction;
  rdfs:label "RotatingMachineAction";
  cims:multiplicity cims:M:0..n;
  owl:inverseOf nc:RotatingMachineAction.RotatingMachine .

nc:RotatingMachineAction a owl:Class;
  rdfs:comment "Rotating machine action."@en;
  rdfs:subClassOf nc:SetPointAction;
  rdfs:label "RotatingMachineAction" .

nc:RotatingMachineAction.RotatingMachine a owl:ObjectProperty, owl:FunctionalProperty;
  rdfs:comment "The rotating machine that has an action."@en;
  rdfs:domain nc:RotatingMachineAction;
  rdfs:range cim:RotatingMachine;
  rdfs:label "RotatingMachine";
  cims:multiplicity cims:M:1..1;
  owl:inverseOf nc:RotatingMachine.RotatingMachineAction .

nc:RotatingMachineControlModeKind a owl:Class;
  rdfs:comment "Kind of rotating machine controller mode."@en;
  rdfs:label "RotatingMachineControlModeKind" .

nc:SSSCControlModeKind a owl:Class;
  rdfs:comment "Control modes of the Static Synchronous Series Compensator (SSSC)."@en;
  rdfs:label "SSSCControlModeKind" .

nc:ScheduleResource a owl:Class;
  rdfs:comment "A schedule resource is a market-based method for handling participation of small units, particularly located on the lower voltage level that is controlled by a Distributed System Operator (DSO). It is a collection of units that can operate in the market by providing bids, offers and a resulting committed operational schedule for the collection."@en;
  rdfs:subClassOf cim:PowerSystemResource;
  rdfs:label "ScheduleResource" .

nc:ScheduleResource.GeneratingUnit a owl:ObjectProperty, owl:InverseFunctionalProperty;
  rdfs:comment "The generating unit that relates to this schedule resource."@en;
  rdfs:domain nc:ScheduleResource;
  rdfs:range cim:GeneratingUnit;
  rdfs:label "GeneratingUnit";
  cims:multiplicity cims:M:0..n;
  owl:inverseOf nc:GeneratingUnit.ScheduleResource .

nc:SchedulingArea a owl:Class;
  rdfs:comment "An area where production and/or consumption of energy can be forecasted, scheduled and measured. The area is operated by only one system operator, typically a Transmission System Operator (TSO). The area can consist of a sub area, which has the same definition as the main area, but it can be operated by another system operator (typically Distributed System Operator (DSO) or a Closed Distributed System Operator (CDSO)). This includes microgrid concept. A substation is the smallest grouping that can"@en;
  rdfs:subClassOf cim:PowerSystemResource;
  rdfs:label "SchedulingArea" .

nc:SchedulingArea.BiddingZone a owl:ObjectProperty, owl:FunctionalProperty;
  rdfs:comment "The bidding zone related to this scheduling area."@en;
  rdfs:domain nc:SchedulingArea;
  rdfs:range nc:BiddingZone;
  rdfs:label "BiddingZone";
  cims:multiplicity cims:M:1..1;
  owl:inverseOf nc:BiddingZone.SchedulingArea .

nc:SchedulingArea.ControlArea a owl:ObjectProperty, owl:FunctionalProperty;
  rdfs:comment "The control area for this scheduling area."@en;
  rdfs:domain nc:SchedulingArea;
  rdfs:range cim:ControlArea;
  rdfs:label "ControlArea";
  cims:multiplicity cims:M:0..1;
  owl:inverseOf nc:ControlArea.SchedulingArea .

nc:SchedulingArea.SynchronousArea a owl:ObjectProperty, owl:FunctionalProperty;
  rdfs:comment "The synchronous are that has this scheduling area."@en;
  rdfs:domain nc:SchedulingArea;
  rdfs:range nc:SynchronousArea;
  rdfs:label "SynchronousArea";
  cims:multiplicity cims:M:0..1;
  owl:inverseOf nc:SynchronousArea.SchedulingArea .

nc:SchedulingArea.normalParticipationFactor a owl:FunctionalProperty, owl:DatatypeProperty;
  rdfs:comment "Normal participation factor describing the entity part of the active power provided by a collection of entities (e.g. an active power forecast to a collection of entities is divided to each of the member entity according to the participation factor). Must be a positive value. In the case of a sharing strategy, the distribution is following entities value (V) equals aggregated value (T) divided by sum of participation factors (PF), i.e. V=T/sum(PF).  In the case of priority strategy, the item with"@en;
  rdfs:domain nc:SchedulingArea;
  rdfs:range xsd:float;
  rdfs:label "normalParticipationFactor";
  cims:multiplicity cims:M:0..1 .

nc:SchedulingArea.participationFactor a owl:FunctionalProperty, owl:DatatypeProperty;
  rdfs:comment "Participation factor describing the entity part of the active power provided by a collection of entities (e.g. an active power forecast to a collection of entities is divided to each of the member entity according to the participation factor). Must be a positive value. In the case of a sharing strategy, the distribution is following entities value (V) equals aggregated value (T) divided by sum of participation factors (PF), i.e. V=T/sum(PF).  In the case of priority strategy, the item with the lowest"@en;
  rdfs:domain nc:SchedulingArea;
  rdfs:range xsd:float;
  rdfs:label "participationFactor";
  cims:multiplicity cims:M:0..1 .

nc:SecuredExclusionReasonKind a owl:Class;
  rdfs:comment "The kind of secured exclusion reason."@en;
  rdfs:label "SecuredExclusionReasonKind" .

nc:SecurityCoordinator a owl:Class;
  rdfs:comment "A role that coordinates the relevant remedial actions and their optimisation to ensure efficient use to achieve required operational security of the power system."@en;
  rdfs:subClassOf nc:SystemOperationCoordinator;
  rdfs:label "SecurityCoordinator" .

nc:SensitivityMatrixKind a owl:Class;
  rdfs:comment "Kinds of sensitivity matrix."@en;
  rdfs:label "SensitivityMatrixKind" .

nc:SetPointAction a owl:Class;
  rdfs:comment "Setpoint action."@en;
  rdfs:subClassOf nc:GridStateAlteration;
  rdfs:label "SetPointAction" .

nc:ShiftMethodKind a owl:Class;
  rdfs:comment "Kind of shift method. Describes the way a power schedule should be distributed amongst production and consumption. e.g. Type of generating and load shift key."@en;
  rdfs:label "ShiftMethodKind" .

nc:Stage a owl:Class;
  rdfs:comment "Stage of a remedial action scheme."@en;
  rdfs:subClassOf cim:IdentifiedObject;
  rdfs:label "Stage" .

nc:Stage.GridStateAlterationCollection a owl:ObjectProperty, owl:FunctionalProperty;
  rdfs:comment "The GridStateAlterationCollection which belongs to the Stage."@en;
  rdfs:domain nc:Stage;
  rdfs:range nc:GridStateAlterationCollection;
  rdfs:label "GridStateAlterationCollection";
  cims:multiplicity cims:M:0..1;
  owl:inverseOf nc:GridStateAlterationCollection.StageAction .

nc:Stage.RemedialActionScheme a owl:ObjectProperty, owl:FunctionalProperty;
  rdfs:comment "The remedial action scheme that has a stage."@en;
  rdfs:domain nc:Stage;
  rdfs:range nc:RemedialActionScheme;
  rdfs:label "RemedialActionScheme";
  cims:multiplicity cims:M:1..1;
  owl:inverseOf nc:RemedialActionScheme.Stage .

nc:Stage.StageTrigger a owl:ObjectProperty, owl:InverseFunctionalProperty;
  rdfs:comment "The state trigger that is part of this stage."@en;
  rdfs:domain nc:Stage;
  rdfs:range nc:StageTrigger;
  rdfs:label "StageTrigger";
  cims:multiplicity cims:M:1..n;
  owl:inverseOf nc:StageTrigger.Stage .

nc:Stage.priority a owl:FunctionalProperty, owl:DatatypeProperty;
  rdfs:comment "The priority of the stage.   0 = do not care (default) 1 = highest priority. 2 is less than 1 and so on. A stage with higher priority needs be activated before a lower stage can be activated."@en;
  rdfs:domain nc:Stage;
  rdfs:range xsd:integer;
  rdfs:label "priority";
  cims:multiplicity cims:M:1..1 .

nc:StageTrigger a owl:Class;
  rdfs:comment "Stage that is triggered either by TriggerCondition or by gate condition within a stage."@en;
  rdfs:subClassOf cim:PowerSystemResource;
  rdfs:label "StageTrigger" .

nc:StageTrigger.GateTrigger a owl:ObjectProperty, owl:FunctionalProperty;
  rdfs:comment "The gate that is the input pin which triggers the protective reactions."@en;
  rdfs:domain nc:StageTrigger;
  rdfs:range nc:Gate;
  rdfs:label "GateTrigger";
  cims:multiplicity cims:M:0..1;
  owl:inverseOf nc:Gate.StageTrigger .

nc:StageTrigger.Stage a owl:ObjectProperty, owl:FunctionalProperty;
  rdfs:comment "The stage that has this stage trigger."@en;
  rdfs:domain nc:StageTrigger;
  rdfs:range nc:Stage;
  rdfs:label "Stage";
  cims:multiplicity cims:M:1..1;
  owl:inverseOf nc:Stage.StageTrigger .

nc:StageTrigger.armed a owl:FunctionalProperty, owl:DatatypeProperty;
  rdfs:comment "The status of the class set by operation or by signal. Optional field that will override other status fields."@en;
  rdfs:domain nc:StageTrigger;
  rdfs:range xsd:boolean;
  rdfs:label "armed";
  cims:multiplicity cims:M:1..1 .

nc:StageTrigger.inService a owl:FunctionalProperty, owl:DatatypeProperty;
  rdfs:comment "Indicates if the stage trigger is in service."@en;
  rdfs:domain nc:StageTrigger;
  rdfs:range xsd:boolean;
  rdfs:label "inService";
  cims:multiplicity cims:M:1..1 .

nc:StageTrigger.normalArmed a owl:FunctionalProperty, owl:DatatypeProperty;
  rdfs:comment "The default/normal value used when other active signal/values are missing."@en;
  rdfs:domain nc:StageTrigger;
  rdfs:range xsd:boolean;
  rdfs:label "normalArmed";
  cims:multiplicity cims:M:1..1 .

nc:StageTrigger.priority a owl:FunctionalProperty, owl:DatatypeProperty;
  rdfs:comment "Priority of trigger. 0 = don t care (default) 1 = highest priority. 2 is less than 1 and so on. A trigger with the highest priority will trigger first."@en;
  rdfs:domain nc:StageTrigger;
  rdfs:range xsd:integer;
  rdfs:label "priority";
  cims:multiplicity cims:M:1..1 .

nc:StaticPropertyRange a owl:Class;
  rdfs:comment "Defines the static range, which means that this is the minimum and/or maximum of an attribute value. The value provided by the schedule replaces the value of the attribute to which the schedule refers to. In case that the PropertyReference refers to Boolean type attributes, RangeConstraint.direction shall be none or upAndDown and the RangeConstraint.valueKind shall be absolute. If the direction is none then optimization of the attribute referenced by the PropertyReference is not possible if the current"@en;
  rdfs:subClassOf nc:RangeConstraint;
  rdfs:label "StaticPropertyRange" .

nc:StaticPropertyRange.PropertyReference a owl:ObjectProperty, owl:FunctionalProperty;
  rdfs:comment "Property reference for this static property range."@en;
  rdfs:domain nc:StaticPropertyRange;
  rdfs:range nc:PropertyReference;
  rdfs:label "PropertyReference";
  cims:multiplicity cims:M:1..1;
  owl:inverseOf nc:PropertyReference.StaticPropertyRange .

nc:SubstationControllerModeKind a owl:Class;
  rdfs:comment "Kind of substation controller mode."@en;
  rdfs:label "SubstationControllerModeKind" .

nc:Switch.TopologyAction a owl:ObjectProperty, owl:InverseFunctionalProperty;
  rdfs:comment "The action assigned to a switch."@en;
  rdfs:domain cim:Switch;
  rdfs:range nc:TopologyAction;
  rdfs:label "TopologyAction";
  cims:multiplicity cims:M:0..n;
  owl:inverseOf nc:TopologyAction.Switch .

nc:SynchronousArea a owl:Class;
  rdfs:comment "A synchronous area is an electrical area covered by interconnect with a common system frequency in a steady-state."@en;
  rdfs:subClassOf cim:PowerSystemResource;
  rdfs:label "SynchronousArea" .

nc:SynchronousArea.SchedulingArea a owl:ObjectProperty, owl:InverseFunctionalProperty;
  rdfs:comment "The scheduling area that is part of this synchronous area."@en;
  rdfs:domain nc:SynchronousArea;
  rdfs:range nc:SchedulingArea;
  rdfs:label "SchedulingArea";
  cims:multiplicity cims:M:0..n;
  owl:inverseOf nc:SchedulingArea.SynchronousArea .

nc:SynchronousArea.nominalFrequency a owl:FunctionalProperty, owl:DatatypeProperty;
  rdfs:comment "The nominal frequency for the Synchronous Area, e.g. 50 Hz for Europe."@en;
  rdfs:domain nc:SynchronousArea;
  rdfs:range xsd:float;
  rdfs:label "nominalFrequency";
  cims:multiplicity cims:M:1..1;
  cim:unitMultiplier cim:UnitMultiplier.none;
  cim:unitSymbol cim:UnitSymbol.Hz;
  qudt:hasQuantityKind cim:Frequency;
  qudt:hasUnit unit:HZ .

nc:SystemOperationCoordinator a owl:Class;
  rdfs:comment "A role that coordinates relevant information and impact in regards to operating the power system."@en;
  rdfs:subClassOf nc:PowerSystemOrganisationRole;
  rdfs:label "SystemOperationCoordinator" .

nc:SystemOperator a owl:Class;
  rdfs:comment "System operator."@en;
  rdfs:subClassOf nc:PowerSystemOrganisationRole;
  rdfs:label "SystemOperator" .

nc:SystemOperator.Contingency a owl:ObjectProperty, owl:InverseFunctionalProperty;
  rdfs:comment "Contingency for the equipment that is operated by the system operator."@en;
  rdfs:domain nc:SystemOperator;
  rdfs:range cim:Contingency;
  rdfs:label "Contingency";
  cims:multiplicity cims:M:0..n;
  owl:inverseOf nc:Contingency.EquipmentOperator .

nc:SystemUnitKind a owl:Class;
  rdfs:comment "A system unit is defined as:  A group of components which are delimited by one or more circuit breakers.  Note 1: the system unit concept has been defined to simplify the calculation of availability. While a system unit is always delimited by circuit breakers, an individual component may not always be. A system unit may therefore contain more than one component.   Note 2: the circuit breakers are not included in the system unit.   Note 3: a tripped element is synonymous to a tripped system unit."@en;
  rdfs:label "SystemUnitKind" .

nc:TCSCControlModeKind a owl:Class;
  rdfs:comment "Kind of TCSC control mode."@en;
  rdfs:label "TCSCControlModeKind" .

nc:Terminal.Circuit a owl:ObjectProperty, owl:InverseFunctionalProperty, owl:FunctionalProperty;
  rdfs:comment "Circuit that is identified by the given Terminal."@en;
  rdfs:domain cim:Terminal;
  rdfs:range nc:Circuit;
  rdfs:label "Circuit";
  cims:multiplicity cims:M:0..1;
  owl:inverseOf nc:Circuit.IdentifyingTerminal .

nc:Terminal.PinTerminal a owl:ObjectProperty, owl:InverseFunctionalProperty;
  rdfs:comment "The pin that uses this input."@en;
  rdfs:domain cim:Terminal;
  rdfs:range nc:PinTerminal;
  rdfs:label "PinTerminal";
  cims:multiplicity cims:M:0..n;
  owl:inverseOf nc:PinTerminal.Terminal .

nc:TimeSeriesInterpolationKind a owl:Class;
  rdfs:comment "Kinds of interpolation of values between two time point."@en;
  rdfs:label "TimeSeriesInterpolationKind" .

nc:TimeSeriesInterpolationKind.previous a nc:TimeSeriesInterpolationKind;
  rdfs:comment "The value between two time points is set to previous value."@en;
  rdfs:label "previous" .

nc:TopologyAction a owl:Class;
  rdfs:comment "Topology action means the connection or disconnection of a switch in the grid model compared to the base case."@en;
  rdfs:subClassOf nc:GridStateAlteration;
  rdfs:label "TopologyAction" .

nc:TopologyAction.Switch a owl:ObjectProperty, owl:FunctionalProperty;
  rdfs:comment "The switch that has a topology action associated."@en;
  rdfs:domain nc:TopologyAction;
  rdfs:range cim:Switch;
  rdfs:label "Switch";
  cims:multiplicity cims:M:1..1;
  owl:inverseOf nc:Switch.TopologyAction .

nc:TransmissionSystemOperator a owl:Class;
  rdfs:comment "A system operator role that is responsible for operating of an energy transmission network."@en;
  rdfs:subClassOf nc:SystemOperator;
  rdfs:label "TransmissionSystemOperator" .

nc:TripKind a owl:Class;
  rdfs:comment """Whether the type of the trip due to the outage was automatic, automatic with successful automatic reclosing or manual.

In case of a fault in the reclosing automatics resulting in lack of reclosing, automatic should be chosen as an alternative."""@en;
  rdfs:label "TripKind" .

nc:ValueOffsetKind a owl:Class;
  rdfs:comment "The kind of the value offset."@en;
  rdfs:label "ValueOffsetKind" .

nc:ValueOffsetKind.incremental a nc:ValueOffsetKind;
  rdfs:comment "Value of the range constraint is incrementing the attribute value referenced by the PropertyReference in a determined operational scenario."@en;
  rdfs:label "incremental" .
