@prefix cimr: <https://cim.ucaiug.io/rules#> .
@prefix entsoe2: <http://entsoe.eu/CIM/SchemaExtension/3/2#> .
@prefix cim:     <https://cim.ucaiug.io/ns#> .
@prefix cims:    <http://iec.ch/TC57/1999/rdf-schema-extensions-19990926#> .

@prefix dcat: <http://www.w3.org/ns/dcat#> .
@prefix dct:  <http://purl.org/dc/terms/> .
@prefix owl:  <http://www.w3.org/2002/07/owl#> .
@prefix psys: <http://proton.semanticweb.org/protonsys#> .
@prefix pti: <http://www.pti-us.com/PTI_CIM-schema-cim16#> .
@prefix rdf:  <http://www.w3.org/1999/02/22-rdf-syntax-ns#> .
@prefix rdfs: <http://www.w3.org/2000/01/rdf-schema#> .
@prefix skos: <http://www.w3.org/2004/02/skos/core#> .
@prefix sesame: <http://www.openrdf.org/schema/sesame#>.
@prefix vann: <http://purl.org/vocab/vann/> .
@prefix xsd:  <http://www.w3.org/2001/XMLSchema#> .

cimr: a owl:Ontology;
  rdfs:label "CIM Inferred Extension Ontology" ;
  rdfs:comment "Inferred properties for electrical CIM/CGMES";
  vann:preferredNamespacePrefix "cimr";
  vann:preferredNamespaceUri "https://cim.ucaiug.io/rules#"^^xsd:anyURI ;
  dct:creator "Vladimir Alexiev", "Nikola Tulechki" ;
  dct:publisher <https://graphwise.ai>;
  dct:created  "2025-02-14"^^xsd:date ;
  dct:modified "2025-06-27"^^xsd:date ;
  dct:publisher "ENTSO-E" ;
  owl:versionInfo "1.1";
  rdfs:seeAlso <https://github.com/statnett/Talk2PowerSystem/issues/16>, <https://github.com/statnett/Talk2PowerSystem/issues/31>;
  dcat:keyword "CIM", "CGMES", "reasoning", "inference", "derived relations", "connectivity", "containment";
  skos:note """Additional Reasoning (counts given about the Nordic44 sample dataset):
The basic CIM ontologies use RDFS subclass, OWL inverse; CIM requires subclass but not inverse; but we used both.
- triples: 63.5k explicit, 17.6k inferred, 81.2k total: 1.28x expansion
The cimr ontology uses RDFS subclass and subproperty, OWL inverse, transitive, propertyChainAxiom (requires owl-rl2-optimized reasoning).
- triples: 63.5k explicit, 60.4k inferred, 124k  total: 1.95x expansion
""".

# TODO: add domain/range?

cimr:hasPart a owl:ObjectProperty;
  rdfs:label "has part";
  rdfs:comment "EquipmentContainer (or Equipment) has part. Disjunction of the props listed in skos:example";
  owl:inverseOf cimr:isPart;
  skos:example cim:EquipmentContainer.Equipments, cim:Substation.VoltageLevels, cim:VoltageLevel.Bays;
  rdfs:subPropertyOf cimr:hasPartTransitive ;
  rdfs:isDefinedBy cimr: .

cim:EquipmentContainer.Equipments rdfs:subPropertyOf cimr:hasPart.
cim:Substation.VoltageLevels      rdfs:subPropertyOf cimr:hasPart.
cim:VoltageLevel.Bays             rdfs:subPropertyOf cimr:hasPart.

cimr:isPart a owl:ObjectProperty;
  rdfs:label "is part";
  rdfs:comment "Equipment is part of EquipmentContainer. Disjunction of the props listed in skos:example";
  owl:inverseOf cimr:hasPart;
  skos:example cim:Equipment.EquipmentContainer, cim:VoltageLevel.Substation, cim:Bay.VoltageLevel;
  rdfs:isDefinedBy cimr: .

cimr:hasPartTransitive a owl:ObjectProperty;
  rdfs:label "has part transitive";
  rdfs:comment "EquipmentContainer and its subcontainers have part Equipment. Transitive closure of cimr:hasPart";
  owl:inverseOf cimr:isPartTransitive;
  psys:transitiveOver cimr:hasPart ;
  rdfs:isDefinedBy cimr: .

cimr:isPartTransitive a owl:ObjectProperty;
  rdfs:label "is part transitive";
  rdfs:comment "Equipment is part of EquipmentContainer and its super-containers. Transitive closure of cimr:isPart";
  owl:inverseOf cimr:hasPartTransitive;
  rdfs:isDefinedBy cimr: .

cimr:Terminal.Equipment a owl:ObjectProperty;
  rdfs:label "equipment";
  rdfs:comment "The equipment of the terminal. Disjunction of the props listed in skos:example";
  owl:inverseOf cimr:Equipment.Terminals;
  skos:example cim:Terminal.ConductingEquipment, cim:Terminal.AuxiliaryEquipment;
  rdfs:isDefinedBy cimr: .

cim:Terminal.ConductingEquipment rdfs:subPropertyOf cimr:Terminal.Equipment.
cim:Terminal.AuxiliaryEquipment  rdfs:subPropertyOf cimr:Terminal.Equipment.

cimr:Equipment.Terminals a owl:ObjectProperty;
  rdfs:label "terminals";
  rdfs:comment "Terminals of the equipment";
  owl:inverseOf cimr:Terminal.Equipment;
  rdfs:isDefinedBy cimr: .

cimr:connectedTo a owl:ObjectProperty, owl:SymmetricProperty;
  rdfs:label "connected to";
  rdfs:comment "Equipment is connected to Equipment through some of their terminals and a common ConnectivityNode";
  rdfs:isDefinedBy cimr: .

cimr:connectedTo owl:propertyChainAxiom
  (cimr:Equipment.Terminals cim:Terminal.ConnectivityNode cim:ConnectivityNode.Terminals cimr:Terminal.Equipment).

cimr:connectedThroughPart a owl:ObjectProperty, owl:SymmetricProperty;
  rdfs:label "connected through part";
  rdfs:comment "Equipment is connected to Equipment through some of its transitive parts, and their terminals and a common ConnectivityNode";
  rdfs:isDefinedBy cimr: .

cimr:connectedThroughPart owl:propertyChainAxiom
  (cimr:hasPartTransitive cimr:connectedTo cimr:isPartTransitive).

cimr:mridSignificantPart a owl:DatatypeProperty ;
   rdfs:label "MRID significant part";
   rdfs:comment "CIM UUIDs vary in the first component and confuse some indexers. This property isolates only the significant part if the id for easier indexing";
   rdfs:isDefinedBy cimr: .

cimr:Measurement.isInCognite a owl:DatatypeProperty ;
   rdfs:label "Measurement is in Cognite";
   rdfs:comment "Flag indicating if a cim:Analog measurement represents to a Cognite timeseries";
   rdfs:domain cim:Analog ;
   rdfs:range xsd:boolean ;
   cims:pragmatics """Use the mRID of this measurement to query a timeseries in the Cognite API by "external_id" """;
   rdfs:isDefinedBy cimr: .

### Pragmatics

cims:pragmatics a owl:DatatypeProperty ;
  rdfs:label "LLM Pragmatics";
  rdfs:comment "Specific SPARQL guidance and important practical information for an LLM. Applies to Classes and Properties.";
  rdfs:range xsd:string  ;
  rdfs:isDefinedBy cimr: .

sesame:directType cims:pragmatics "Use this to find leaf-level (concrete) type of a resource".

cim:Line cims:pragmatics "This means only AC Line (not DC)".

cim:ConductingEquipment cims:pragmatics  "This means only AC Conducting Equipment (not DC)".

cim:Measurement.measurementType
  skos:example "CurrencyExchange-Actual", "Price-Actual", "ThreePhaseActivePower", "ThreePhaseActivePower-Flow-Estimated";
  cims:pragmatics "Possible values: CurrencyExchange-Actual, Price-Actual, ThreePhaseActivePower, ThreePhaseActivePower-Flow-Estimated".

cim:Analog.positiveFlowIn cims:pragmatics """For BiddingZoneBorder,
"true" means the flow is from BiddingZoneOne to BiddingZoneTwo.
"false" means the flow is in the opposite direction""".

pti:Measurement.uncefactUnitCode cims:pragmatics "Uses UNCEFACT Rec21 unit codes".

pti:Diagram.type
  skos:example "Worldview", "Substation";
  cims:pragmatics "Possible values: Worldview, Substation".


#### Patch to add some entsoe2 terms

#entsoe2:EnergyCongestionZone a rdfs:Class;
#  rdfs:label "EnergyCongestionZone"@en;
#  rdfs:comment "Energy congestion zone"@en;
#  rdfs:subClassOf cim:PowerSystemResource;
#  rdfs:isDefinedBy cimr: .
#
#entsoe2:EnergyCongestionZone.netDCInterchange a rdf:Property;
#  rdfs:label "netDCInterchange"@en;
#  rdfs:comment "Net DC interchange"@en;
#  rdfs:domain entsoe2:EnergyCongestionZone;
#  cims:dataType cim:Float;
#  rdfs:isDefinedBy cimr: .
#
#entsoe2:EnergyCongestionZone.netACInterchangeTolerance a rdf:Property;
#  rdfs:label "netDCInterchangeTolerance"@en;
#  rdfs:comment "Net DC interchange tolerance"@en;
#  rdfs:domain entsoe2:EnergyCongestionZone;
#  cims:dataType cim:Float;
#  rdfs:isDefinedBy cimr: .
#
#entsoe2:EnergyCongestionZone.netACInterchange a rdf:Property;
#  rdfs:label "netACInterchange"@en;
#  rdfs:comment "Net AC interchange"@en;
#  rdfs:domain entsoe2:EnergyCongestionZone;
#  cims:dataType cim:Float;
#  rdfs:isDefinedBy cimr: .
