@prefix cimd: <https://cim.ucaiug.io/diagrams#> .
@prefix cim:  <https://cim.ucaiug.io/ns#> .
@prefix cims: <http://iec.ch/TC57/1999/rdf-schema-extensions-19990926#> .
@prefix dcat: <http://www.w3.org/ns/dcat#> .
@prefix dct:  <http://purl.org/dc/terms/> .
@prefix owl:  <http://www.w3.org/2002/07/owl#> .
@prefix rdf:  <http://www.w3.org/1999/02/22-rdf-syntax-ns#> .
@prefix rdfs: <http://www.w3.org/2000/01/rdf-schema#> .
@prefix skos: <http://www.w3.org/2004/02/skos/core#> .
@prefix vann: <http://purl.org/vocab/vann/> .
@prefix xsd:  <http://www.w3.org/2001/XMLSchema#> .
@prefix uml:  <http://iec.ch/TC57/NonStandard/UML#> .

cimd: a owl:Ontology;
  rdfs:label "CIM Diagrams Ontology";
  dct:title  "CIM Diagrams Ontology";
  rdfs:comment    "Various CIM/CGMES diagrams: electrical (generated with PowSyBl), geospatial, GraphDB VizGraph";
  dct:description "Various CIM/CGMES diagrams: electrical (generated with PowSyBl), geospatial, GraphDB VizGraph";
  vann:preferredNamespacePrefix "cimd";
  vann:preferredNamespaceUri "https://cim.ucaiug.io/diagrams#"^^xsd:anyURI ;
  dct:creator <https://graphwise.ai> ;
  dct:created  "2025-12-05"^^xsd:date ;
  dct:modified "2025-12-05"^^xsd:date ;
  dct:issued   "2025-12-05"^^xsd:date ;
  owl:versionInfo "1.0";
  rdfs:seeAlso <https://github.com/statnett/Talk2PowerSystem/wiki/Electrical-Diagrams>, <https://github.com/statnett/Talk2PowerSystem/tree/main/diagram>;
  dcat:keyword "CIM", "CGMES", "diagrams", "PowSyBl", "Network-Area-Diagram", "Single-Line-Diagram", "Visual Graph".

cimd:Diagram a owl:Class ;
  rdfs:label "Diagram" ;
  rdfs:comment """Diagram represented as an image (SVG, PNG) or web app (the MIME type is indicated by dct:format).
Unlike cim:Diagram, cimd:Diagram doesn't have DiagramObjects and DiagramObjectPoints.""" ;
  cims:stereotype uml:concrete ;
  rdfs:subClassOf cim:IdentifiedObject;
  cims:pragmatics "In this knowledge graph, cimd:Diagram instances can be displayed by the diagram tool; cim:Diagram instances cannot be displayed";
  cims:belongsToCategory cimd: ;
  rdfs:isDefinedBy cimd: .

cim:Diagram cims:pragmatics "In this knowledge graph, cimd:Diagram instances can be displayed by the diagram tool; cim:Diagram instances cannot be displayed".

cimd:DiagramKind a owl:Class ;
  rdfs:label "DiagramKind" ;
  rdfs:comment "Diagram kind reflecting the technology (e.g. PowSyBl vs VizGraph) and subkind." ;
  cims:stereotype uml:enumeration ;
  cims:belongsToCategory cimd: ;
  rdfs:isDefinedBy cimd: .

cimd:DiagramKind.PowSyBl-NetworkAreaDiagram a cimd:DiagramKind;
  rdfs:label "PowSyBl-NetworkAreaDiagram";
  rdfs:comment """PowSyBl Network-Area-Diagram. Shows voltage levels as nodes, and the lines and transformers between voltage levels as edges.
Can display the whole grid, one or several voltage levels, and the neighborhood of one or several voltage levels up to a given depth""";
  cims:stereotype "enum" ;
  rdfs:isDefinedBy cimd: .

cimd:DiagramKind.PowSyBl-SingleLineDiagram a cimd:DiagramKind;
  rdfs:label "PowSyBl-SingleLineDiagram";
  rdfs:comment """PowSyBl Single-Line-Diagram. Shows equipment (switches, disconnectors, busbars, voltage levels, power transformers, loads, generators), adjacent lines, voltages and input/output flows.
Can display one or several substations, voltage levels or areas.""";
  cims:stereotype "enum" ;
  rdfs:isDefinedBy cimd: .
  
cimd:DiagramKind.PowSyBl-SingleLineDiagram-Multi a cimd:DiagramKind;
  rdfs:label "PowSyBl-SingleLineDiagram-Multi";
  rdfs:comment """PowSyBl Single-Line-Diagram (Multi). Shows equipment in several substations (switches, disconnectors, busbars, voltage levels, power transformers, loads, generators), adjacent lines, voltages and input/output flows.""";
  cims:stereotype "enum" ;
  rdfs:isDefinedBy cimd: .
  
cimd:Diagram.kind a owl:ObjectProperty, owl:FunctionalProperty;
  cims:multiplicity cims:M:1..1 ;
  rdfs:label "kind";
  rdfs:comment "Kind of diagram";
  rdfs:domain cimd:Diagram;
  rdfs:range cimd:DiagramKind.

cimd:Diagram.PowerSystemResource a owl:Property;
  cims:multiplicity cims:M:0..n ;
  rdfs:label "PowerSystemResource";
  rdfs:comment "Power System Resource(s) shown on the diagram. This lists major resources (eg SubGeographicalArea, LoadArea) but doesn't list the individual VoltageLevels compare to cimd:Diagram.mRIDs)";
  rdfs:domain cimd:Diagram;
  rdfs:range cim:PowerSystemResource.

cimd:Diagram.link a owl:Property, owl:FunctionalProperty;
  cims:multiplicity cims:M:1..1 ;
  rdfs:label "link";
  rdfs:comment "Image file or web app link. For reasons of portability between servers, it is a relative URL (does not include the base).";
  rdfs:domain cimd:Diagram;
  rdfs:range xsd:string.

cimd:Diagram.mRIDs a owl:Property, owl:FunctionalProperty;
  cims:multiplicity cims:M:0..1 ;
  rdfs:label "mRIDs";
  rdfs:comment "mRIDs of the lower-level PSRs (Substations or VoltageLevels) shown on the diagram, as a string suitable for passing to PowSyBl Python version. Compare to cimd:Diagram.PowerSystemResource.";
  skos:example
    'Single substation or voltage level: "mrid1"',
    'Two substations listed left-to-right (west-to-east): [["mrid1","mrid2"]]',
    'Multiple voltage levels: ("mrid1","mrid2"..."mridN")';
  rdfs:domain cimd:Diagram;
  rdfs:range xsd:string.

# TODO: add DiagramKind.VizGraph* and DiagramConfiguration
